@prefix classifier: <http://anzsoil.org/def/soil/au/edu/fed-uni/classifier/colour/> .
@prefix dc: <http://purl.org/dc/elements/1.1/> .
@prefix dcat: <http://www.w3.org/ns/dcat#> .
@prefix dct: <http://purl.org/dc/terms/> .
@prefix euvoc: <http://publications.europa.eu/ontology/euvoc#> .
@prefix foaf: <http://xmlns.com/foaf/0.1/> .
@prefix fu: <http://anzsoil.org/def/soil/au/edu/fed-uni/> .
@prefix ldp: <http://www.w3.org/ns/ldp#> .
@prefix lismore-soil-series: <http://anzsoil.org/def/soil/au/edu/fed-uni/classifier/name/lismore/> .
@prefix name: <http://anzsoil.org/def/soil/au/edu/fed-uni/classifier/name/> .
@prefix object: <http://anzsoil.org/def/soil/au/edu/fed-uni/object/> .
@prefix org: <http://www.w3.org/ns/org#> .
@prefix owl: <http://www.w3.org/2002/07/owl#> .
@prefix procedure: <http://anzsoil.org/def/soil/au/edu/fed-uni/procedure/> .
@prefix property: <http://anzsoil.org/def/soil/au/edu/fed-uni/property/> .
@prefix prov: <http://www.w3.org/ns/prov#> .
@prefix qb: <http://purl.org/linked-data/cube#> .
@prefix rdf: <http://www.w3.org/1999/02/22-rdf-syntax-ns#> .
@prefix rdfs: <http://www.w3.org/2000/01/rdf-schema#> .
@prefix schema: <http://schema.org/> .
@prefix sdo: <https://schema.org/> .
@prefix sh: <http://www.w3.org/ns/shacl#> .
@prefix skos: <http://www.w3.org/2004/02/skos/core#> .
@prefix skosthes: <http://purl.org/iso25964/skos-thes#> .
@prefix skosxl: <http://www.w3.org/2008/05/skos-xl#> .
@prefix sosa: <http://www.w3.org/ns/sosa/> .
@prefix structure-pedality-type: <http://anzsoil.org/def/soil/au/edu/fed-uni/classifier/structure-pedality-type/> .
@prefix texture-grade: <http://anzsoil.org/def/soil/au/edu/fed-uni/classifier/texture-grade/> .
@prefix ui: <http://purl.org/linked-data/registry-ui#> .
@prefix xsd: <http://www.w3.org/2001/XMLSchema#> .

<http://anzoil.org/def/soil/au/edu/fed-uni> a skos:ConceptScheme;
  dct:accrualPeriodicity <http://purl.org/cld/freq/completelyIrregular>;
  dct:contributor <https://orcid.org/0000-0002-3884-3420\u0020,\u0020https://orcid.org/0000-0002-9722-4697\u0020,\u0020Bruce\u0020Simons>;
  dct:created "2021-12-24"^^xsd:date;
  dct:creator <https://orcid.org/0000-0002-2991-2308>;
  dct:description "<p>A machine representation of concepts used in the description of soil data and information. Maintained by Federation University, Centre for eResearch and Digital Innovation (CeRDI). </p>"^^rdf:HTML,
    "<p>Controlled-Vocabularies used in the description of soil data and information by Centre of eResearch and Digital Innovation, Federation University.</p>"^^rdf:HTML;
  dct:identifier "http://anzsoil.org/def/soil/au/edu/fed-uni"^^xsd:anyURI;
  dct:license <https://creativecommons.org/publicdomain/zero/1.0/>;
  dct:source "From data providers' desciptions of their data, including from data headers, reports, soil testing laborarory result sheets, and publically available soil testing laboratory information sheets. Some of the terms are derivatives, extensions and or machine encodings of Australian Soil Standards URN:ISBN:978-0-909605-68-1 , URN:ISBN:978-0-643-10218-7 and URN:ISBN:978-0-64309-395-9"@en;
  dct:title "Federation University soil controlled-vocabularies"@en;
  ui:hierarchyChildProperty skos:member;
  ui:hierarchyRootProperty ui:topMemberOf;
  owl:VersionInfo "001"@en;
  skos:hasTopConcept procedure:12A1-CU, procedure:12A1-FE, procedure:12A1-MN, procedure:12A1-ZN,
    procedure:12B1-CO, procedure:12B1-CU, procedure:12B1-ZN, procedure:12C, procedure:12D1-CU,
    procedure:12D1-FE, procedure:12D1-MN, procedure:12D1-ZN, procedure:13A1-FE, procedure:15D2-MG,
    procedure:15D2-NA, procedure:15D3-15G1-ECEC, procedure:15D3-15G1-ECEC-CA, procedure:15D3-15G1-ECEC-K,
    procedure:15D3-15G1-ECEC-MG, procedure:15D3-15G1-ECEC-NA, procedure:15D3-CA, procedure:15D3-CEC-CA,
    procedure:15D3-CEC-K, procedure:15D3-CEC-MG, procedure:15D3-CEC-NA, procedure:15D3-ECR,
    procedure:15D3-GTRI, procedure:15D3-K, procedure:15D3-MG, procedure:15D3-NA, procedure:15E1-AL,
    procedure:15E1-CA, procedure:15E1-K, procedure:15E1-MG, procedure:15E1-NA, procedure:15D1-BACL-H,
    procedure:15D1-BACL-K, procedure:15D1-BACL-MG, procedure:15D1-BACL-NA, procedure:15D1-CA,
    procedure:15D1-K, procedure:15D1-MG, procedure:15D1-NA, procedure:15E2-CA, procedure:15E2-K,
    procedure:15E2-MG, procedure:15E2-NA, procedure:15G1-15D3-ECEC-AL, procedure:15G1-15D3-ECEC-H,
    procedure:15G1-AL, procedure:15G1-H, procedure:15M1-CMR, procedure:15M1-PMR, procedure:3A1-TDS,
    procedure:6C1HUMa, procedure:6C1POCa, procedure:6C1RECa, procedure:7C2a-NH4, procedure:7C2a-NO3,
    procedure:7C2b-NH4, procedure:7C2b-NO3, procedure:9I2, procedure:AA-S, procedure:AD-TOT-P,
    procedure:ADJ-CEC, procedure:ADJ-EXCH-H, procedure:AODE-AVL-MO, procedure:AVL-CA,
    procedure:AVL-K, procedure:AVL-MG, procedure:AVL-NA, procedure:AVL-ZN, procedure:AW-TOT-C,
    procedure:B, procedure:BACL-EXCH-H, procedure:AL, procedure:BCI, procedure:BROMF-AL,
    procedure:BRU-N, procedure:CA, procedure:CACL2-AL, procedure:CACL2-PH, procedure:18F1-S,
    procedure:CACL2a-SI, procedure:CEC, procedure:CEC-AL, procedure:CEC-NA, procedure:CL,
    procedure:15M1-CNR, procedure:6A1-MOD, procedure:CMR, procedure:CO, procedure:CO2-MA,
    procedure:CO2-MBR, procedure:CO2-MIN-N, procedure:CO2-MIN-P, procedure:CO2-SBR-C,
    procedure:CO2-SMB, procedure:CU, procedure:DGT-P, procedure:EC, procedure:ECEC, procedure:ECEC-NA,
    procedure:ECSE-SP, procedure:EXCH-AL, procedure:EXCH-CA, procedure:15D1-BACL-CA, procedure:EXCH-H,
    procedure:9K1, procedure:EXCH-K, procedure:EXCH-MG, procedure:EXCH-NA, procedure:FE,
    procedure:GTRI, procedure:15D-CA, procedure:H2O-PH, procedure:HWS-B, procedure:HWS-ICP-B,
    procedure:ICP-TOT-CA, procedure:ICP-TOT-CO, procedure:ICP-TOT-CU, procedure:ICP-TOT-FE,
    procedure:ICP-TOT-K, procedure:ICP-TOT-MG, procedure:ICP-TOT-MN, procedure:ICP-TOT-NA,
    procedure:ICP-TOT-P, procedure:ICP-TOT-ZN, procedure:K, procedure:MG, procedure:MIK-AVL-FE,
    procedure:MIK-AVL-MN, procedure:MIR, procedure:MN, procedure:MO, procedure:NA, object:POC,
    object:HUM, object:REC, classifier:grey, classifier:brown, classifier:orange-yellow,
    classifier:grey-brown, classifier:brown-grey, classifier:dark-grey, classifier:light-grey,
    classifier:grey-yellow, classifier:dark-brown, classifier:light-brown, classifier:brown-yellow,
    classifier:red, classifier:grey-black, classifier:brown-black, classifier:brown-orange,
    classifier:brown-white, classifier:yellow, classifier:brown-red, classifier:grey-white,
    classifier:yellow-brown, classifier:dark-yellow-brown, classifier:black, classifier:dark-grey-brown,
    classifier:red-brown, classifier:very-dark-grey, classifier:light-olive-brown, classifier:very-dark-grey-brown,
    classifier:very-dark-brown, classifier:light-yellow-brown, classifier:light-grey-brown,
    classifier:very-dusky-red, classifier:dusky-red, classifier:olive-grey, procedure:NACL2,
    procedure:CSBP-CA, procedure:CSBP-MG, procedure:CSBP-K, procedure:CSBP-NA, procedure:15G,
    procedure:15G-AL, procedure:15G-H, procedure:15D-MG, procedure:15D-K, procedure:15D-NA,
    lismore-soil-series:mundy-gully-black-clays, lismore-soil-series:buckshot-clays, lismore-soil-series:lismore-grey-clays,
    lismore-soil-series:nowra-red-clays, lismore-soil-series:lunette-clays, lismore-soil-series:granitic-sandy-loam,
    texture-grade:C, texture-grade:CSBP-S, texture-grade:CSBP-LS, texture-grade:CSBP-L,
    texture-grade:CSBP-CL, texture-grade:CSBP-C, texture-grade:CSBP-HC, texture-grade:L,
    texture-grade:SL, texture-grade:CL, texture-grade:SCL, texture-grade:SC, texture-grade:S,
    texture-grade:LS, procedure:NH4, structure-pedality-type:B, procedure:NH4-NO3, procedure:NO3,
    procedure:OC-TN, procedure:P, procedure:P6-LP, procedure:PAW, procedure:PBI, procedure:PERI,
    procedure:PH, procedure:PLFA-DR, procedure:PLFA-DRR, procedure:PLFA-FB, procedure:PLFA-MBAL,
    procedure:PLFA-MD, procedure:PLFA-MF-B, procedure:PLFA-NA-VAM, procedure:PLFA-NCR,
    procedure:PLFA-NSR, procedure:PLFA-PB, procedure:PLFA-RB, procedure:PLFA-TAB, procedure:PLFA-TBB,
    procedure:PLFA-TFB, procedure:PLFA-TMB, procedure:PRI-AJ, procedure:PSR, procedure:R-FE,
    procedure:RCH-N, procedure:S, procedure:S10-CA, procedure:S10-K, procedure:S10-MG,
    procedure:S10-P, procedure:SC-30-NETP, procedure:SC-30-NFIX, procedure:SC-30-NMIN,
    procedure:SC-30-NR, procedure:SC-7-PFERT, procedure:SC-7-PREL, procedure:SE, procedure:SI,
    procedure:SOC, procedure:SOM, procedure:TAE-AL, procedure:TAE-B, procedure:TAE-CA,
    procedure:TAE-CO, procedure:TAE-CU, procedure:TAE-FE, procedure:TAE-K, procedure:TAE-MG,
    procedure:TAE-MN, procedure:TAE-MO, procedure:TAE-NA, procedure:TAE-P, procedure:TAE-S,
    procedure:TAE-SE, procedure:TAE-SI, procedure:TAE-ZN, procedure:TC-KJE, procedure:TOC-TN,
    procedure:TOT-C, procedure:TOT-N, procedure:WB-MOD-2-TOC, procedure:WB-MOD-TOC, procedure:WB-N,
    procedure:WB-OM, procedure:WE-CN, procedure:WE-OC, procedure:WE-OC-ON, procedure:WE-ON,
    procedure:WP-P, procedure:ZN, procedure:bouyoucos-1936, procedure:bray-2, procedure:bulk-density-soil,
    procedure:field-soil-texture, procedure:field-soil-texture-organic, procedure:gravel-1,
    procedure:gravel-2, procedure:soil-texture, property:HUM-concentration, property:POC-concentration,
    property:REC-concentration, property:SOM-concentration, property:calcium-magnesium-ratio,
    property:clay-content, property:evc-vic, property:exchangeable-cation-ratio, property:grass-tetany-risk-index,
    property:lower-depth-boundary, property:phosphorus-environmental-risk-index, property:phosphorus-retention-index,
    property:phosphorus-saturation-ratio, property:potassium-magnesium-ratio, property:potassium-sodium-ratio,
    property:sand-content, property:silt-content, property:upper-depth-boundary;
  sdo:codeRepository <https://github.com/FedUni-CeRDI/def-au-edu-feduni> .

fu:procedure a "reg:Register"@en, ldp:Container;
  dct:description "A collection of some procedures used to describe the measurement of soil observable properties"@en;
  dct:identifier "http://anzsoil.org/def/soil/au/edu/fed-uni/procedure"^^xsd:anyURI;
  ui:topMemberOf <http://anzsoil.org/def/soil/au/edu/fed-uni>;
  rdfs:label "Procedures"@en;
  skos:definition "A collection of some procedures used to make an observation related to soil"@en;
  skos:member procedure:12A1-CU, procedure:12A1-FE, procedure:12A1-MN, procedure:12A1-ZN,
    procedure:12B1-CO, procedure:12B1-CU, procedure:12B1-ZN, procedure:12C, procedure:12D1-CU,
    procedure:12D1-FE, procedure:12D1-MN, procedure:12D1-ZN, procedure:13A1-FE, procedure:15D2-MG,
    procedure:15D2-NA, procedure:15D3-15G1-ECEC, procedure:15D3-15G1-ECEC-CA, procedure:15D3-15G1-ECEC-K,
    procedure:15D3-15G1-ECEC-MG, procedure:15D3-15G1-ECEC-NA, procedure:15D3-CA, procedure:15D3-CEC-CA,
    procedure:15D3-CEC-K, procedure:15D3-CEC-MG, procedure:15D3-CEC-NA, procedure:15D3-ECR,
    procedure:15D3-GTRI, procedure:15D3-K, procedure:15D3-MG, procedure:15D3-NA, procedure:15E1-AL,
    procedure:15E1-CA, procedure:15E1-K, procedure:15E1-MG, procedure:15E1-NA, procedure:15D1-BACL-H,
    procedure:15D1-BACL-K, procedure:15D1-BACL-MG, procedure:15D1-BACL-NA, procedure:15D1-CA,
    procedure:15D1-K, procedure:15D1-MG, procedure:15D1-NA, procedure:15E2-CA, procedure:15E2-K,
    procedure:15E2-MG, procedure:15E2-NA, procedure:15G1-15D3-ECEC-AL, procedure:15G1-15D3-ECEC-H,
    procedure:15G1-AL, procedure:15G1-H, procedure:15M1-CMR, procedure:15M1-PMR, procedure:3A1-TDS,
    procedure:6C1HUMa, procedure:6C1POCa, procedure:6C1RECa, procedure:7C2a-NH4, procedure:7C2a-NO3,
    procedure:7C2b-NH4, procedure:7C2b-NO3, procedure:9I2, procedure:AA-S, procedure:AD-TOT-P,
    procedure:ADJ-CEC, procedure:ADJ-EXCH-H, procedure:AODE-AVL-MO, procedure:AVL-CA,
    procedure:AVL-K, procedure:AVL-MG, procedure:AVL-NA, procedure:AVL-ZN, procedure:AW-TOT-C,
    procedure:B, procedure:BACL-EXCH-H, procedure:AL, procedure:BCI, procedure:BROMF-AL,
    procedure:BRU-N, procedure:CA, procedure:CACL2-AL, procedure:CACL2-PH, procedure:18F1-S,
    procedure:CACL2a-SI, procedure:CEC, procedure:CEC-AL, procedure:CEC-NA, procedure:CL,
    procedure:15M1-CNR, procedure:6A1-MOD, procedure:CMR, procedure:CO, procedure:CO2-MA,
    procedure:CO2-MBR, procedure:CO2-MIN-N, procedure:CO2-MIN-P, procedure:CO2-SBR-C,
    procedure:CO2-SMB, procedure:CU, procedure:DGT-P, procedure:EC, procedure:ECEC, procedure:ECEC-NA,
    procedure:ECSE-SP, procedure:EXCH-AL, procedure:EXCH-CA, procedure:15D1-BACL-CA, procedure:EXCH-H,
    procedure:9K1, procedure:EXCH-K, procedure:EXCH-MG, procedure:EXCH-NA, procedure:FE,
    procedure:GTRI, procedure:15D-CA, procedure:H2O-PH, procedure:HWS-B, procedure:HWS-ICP-B,
    procedure:ICP-TOT-CA, procedure:CSBP-CA, procedure:CSBP-MG, procedure:CSBP-K, procedure:CSBP-NA,
    procedure:15G, procedure:15G-AL, procedure:15G-H, procedure:15D-MG, procedure:15D-K,
    procedure:15D-NA, procedure:ICP-TOT-CO, procedure:ICP-TOT-CU, procedure:ICP-TOT-FE,
    procedure:ICP-TOT-K, procedure:ICP-TOT-MG, procedure:ICP-TOT-MN, procedure:ICP-TOT-NA,
    procedure:ICP-TOT-P, procedure:ICP-TOT-ZN, procedure:K, procedure:MG, procedure:MIK-AVL-FE,
    procedure:MIK-AVL-MN, procedure:MIR, procedure:MN, procedure:MO, procedure:NA, procedure:NACL2,
    procedure:NH4, procedure:NH4-NO3, procedure:NO3, procedure:OC-TN, procedure:P, procedure:P6-LP,
    procedure:PAW, procedure:PBI, procedure:PERI, procedure:PH, procedure:PLFA-DR, procedure:PLFA-DRR,
    procedure:PLFA-FB, procedure:PLFA-MBAL, procedure:PLFA-MD, procedure:PLFA-MF-B, procedure:PLFA-NA-VAM,
    procedure:PLFA-NCR, procedure:PLFA-NSR, procedure:PLFA-PB, procedure:PLFA-RB, procedure:PLFA-TAB,
    procedure:PLFA-TBB, procedure:PLFA-TFB, procedure:PLFA-TMB, procedure:PRI-AJ, procedure:PSR,
    procedure:R-FE, procedure:RCH-N, procedure:S, procedure:S10-CA, procedure:S10-K, procedure:S10-MG,
    procedure:S10-P, procedure:SC-30-NETP, procedure:SC-30-NFIX, procedure:SC-30-NMIN,
    procedure:SC-30-NR, procedure:SC-7-PFERT, procedure:SC-7-PREL, procedure:SE, procedure:SI,
    procedure:SOC, procedure:SOM, procedure:TAE-AL, procedure:TAE-B, procedure:TAE-CA,
    procedure:TAE-CO, procedure:TAE-CU, procedure:TAE-FE, procedure:TAE-K, procedure:TAE-MG,
    procedure:TAE-MN, procedure:TAE-MO, procedure:TAE-NA, procedure:TAE-P, procedure:TAE-S,
    procedure:TAE-SE, procedure:TAE-SI, procedure:TAE-ZN, procedure:TC-KJE, procedure:TOC-TN,
    procedure:TOT-C, procedure:TOT-N, procedure:WB-MOD-2-TOC, procedure:WB-MOD-TOC, procedure:WB-N,
    procedure:WB-OM, procedure:WE-CN, procedure:WE-OC, procedure:WE-OC-ON, procedure:WE-ON,
    procedure:WP-P, procedure:ZN, procedure:bouyoucos-1936, procedure:bray-2, procedure:bulk-density-soil,
    procedure:field-soil-texture, procedure:field-soil-texture-organic, procedure:gravel-1,
    procedure:gravel-2, procedure:soil-texture;
  skos:prefLabel "Procedures"@en .

fu:property a "reg:Register"@en, ldp:Container;
  dct:description "A register of soil observable properties used in the desciption of soils"@en;
  dct:identifier "http://anzsoil.org/def/soil/au/edu/fed-uni/property"^^xsd:anyURI;
  ui:topMemberOf <http://anzsoil.org/def/soil/au/edu/fed-uni>;
  rdfs:label "Properties"@en;
  skos:definition "A collection of soil observable properties related to soil"@en;
  skos:member property:HUM-concentration, property:POC-concentration, property:REC-concentration,
    property:SOM-concentration, property:calcium-magnesium-ratio, property:clay-content,
    property:evc-vic, property:exchangeable-cation-ratio, property:grass-tetany-risk-index,
    property:lower-depth-boundary, property:phosphorus-environmental-risk-index, property:phosphorus-retention-index,
    property:phosphorus-saturation-ratio, property:potassium-magnesium-ratio, property:potassium-sodium-ratio,
    property:sand-content, property:silt-content, property:upper-depth-boundary;
  skos:prefLabel "Properties"@en .

fu:object a "reg:Register"@en, ldp:Container;
  dct:description "A collection of objects, substances and taxa which may appear as the subject (identified object) of soil observable properties"@en;
  dct:identifier "http://anzsoil.org/def/soil/au/edu/fed-uni/object"^^xsd:anyURI;
  ui:topMemberOf <http://anzsoil.org/def/soil/au/edu/fed-uni>;
  rdfs:label "Objects"@en;
  skos:definition "A collection of objects, substances and taxa which may appear as the subject (identified object) of soil observable relating to soil"@en;
  skos:member object:HUM, object:POC, object:REC;
  skos:prefLabel "Objects"@en .

fu:classifier a "reg:Register"@en, ldp:Container;
  dct:description "A collection of soil classifiers. These classifiers fall outside of the codes and vocabularies from National Committee on Soil and Terrain (2009), Australian soil and land survey field handbook (3rd edn). (© CSIRO Publishing: Melbourne)"@en;
  dct:identifier "http://anzsoil.org/def/soil/au/edu/fed-uni/classifier"^^xsd:anyURI;
  ui:topMemberOf <http://anzsoil.org/def/soil/au/edu/fed-uni>;
  rdfs:label "Classifiers"@en;
  skos:definition "A collection of soil classifiers that are the results of observations relating to soil. These classifiers fall outside of the codes and vocabularies from National Committee on Soil and Terrain (2009), Australian soil and land survey field handbook (3rd edn). ISBN: 9780643093959"@en;
  skos:member classifier:name, classifier:structure-pedality-type;
  skos:prefLabel "Classifiers"@en .

classifier:colour a "reg:Register"@en, ldp:Container;
  dct:description "A register of soil colour classifiers. These classifiers fall outside the colour descriptions of the Australian Soil and Land Survey Field Handbook (3rd edn). ISBN: 9780643093959"@en;
  dct:identifier "http://anzsoil.org/def/soil/au/edu/fed-uni/classifier/colour"^^xsd:anyURI;
  rdfs:label "Colours"@en;
  skos:definition "Soil colour classifiers. These classifiers fall outside the colour descriptions of the Australian Soil and Land Survey Field Handbook (3rd edn). ISBN: 9780643093959"@en;
  skos:member classifier:black, classifier:brown, classifier:brown-black, classifier:brown-grey,
    classifier:brown-orange, classifier:brown-red, classifier:brown-white, classifier:brown-yellow,
    classifier:dark-brown, classifier:dark-grey, classifier:dark-grey-brown, classifier:dark-yellow-brown,
    classifier:dusky-red, classifier:grey, classifier:grey-black, classifier:grey-brown,
    classifier:grey-white, classifier:grey-yellow, classifier:light-brown, classifier:light-grey,
    classifier:light-grey-brown, classifier:light-olive-brown, classifier:light-yellow-brown,
    classifier:olive-grey, classifier:orange-yellow, classifier:red, classifier:red-brown,
    classifier:very-dark-brown, classifier:very-dark-grey, classifier:very-dark-grey-brown,
    classifier:very-dusky-red, classifier:yellow, classifier:yellow-brown;
  skos:prefLabel "Colours"@en .

fu:clasifier skos:member classifier:colour, classifier:texture-grade .

classifier:texture-grade a "reg:Register"@en, ldp:Container;
  dct:description "A register of soil texture grades that fall outside the mineral soils field texture grades described in Australian Soil and Land Survey Field Handbook (3rd edn). ISBN: 9780643093959"@en;
  dct:identifier "http://anzsoil.org/def/soil/au/edu/fed-uni/classifier/texture-grade"^^xsd:anyURI;
  rdfs:label "Texture Grades"@en;
  skos:definition "Soil texture classifiers. These grades fall outside the mineral soils field texture grades described in Australian Soil and Land Survey Field Handbook (3rd edn). ISBN: 9780643093959"@en;
  skos:member texture-grade:C, texture-grade:CL, texture-grade:CSBP-C, texture-grade:CSBP-CL,
    texture-grade:CSBP-HC, texture-grade:CSBP-L, texture-grade:CSBP-LS, texture-grade:CSBP-S,
    texture-grade:L, texture-grade:LS, texture-grade:S, texture-grade:SC, texture-grade:SCL,
    texture-grade:SL;
  skos:prefLabel "Texture Grades"@en .

procedure:12A1-CU a skos:Concept, sosa:Procedure;
  dct:description "A procedure for measuring Extractable Copper DTPA"@en;
  dct:identifier "http://anzsoil.org/def/soil/au/edu/fed-uni/procedure/12A1-CU"^^xsd:anyURI;
  rdfs:label "DTPA - Extractable Copper procedure"@en;
  skos:definition "A procedure for measuring Extractable Copper DTPA"@en;
  skos:inScheme <http://anzoil.org/def/soil/au/edu/fed-uni>;
  skos:notation "12A1-CU";
  skos:prefLabel "DTPA - Extractable Copper procedure"@en;
  skos:topConceptOf <http://anzoil.org/def/soil/au/edu/fed-uni> .

procedure:12A1-FE a skos:Concept, sosa:Procedure;
  dct:description "A procedure for measuring Extractable Iron DTPA"@en;
  dct:identifier "http://anzsoil.org/def/soil/au/edu/fed-uni/procedure/12A1-FE"^^xsd:anyURI;
  rdfs:label "DTPA - Extractable Iron procedure"@en;
  skos:definition "A procedure for measuring Extractable Iron DTPA"@en;
  skos:inScheme <http://anzoil.org/def/soil/au/edu/fed-uni>;
  skos:notation "12A1-FE";
  skos:prefLabel "DTPA - Extractable Iron procedure"@en;
  skos:topConceptOf <http://anzoil.org/def/soil/au/edu/fed-uni> .

procedure:12A1-MN a skos:Concept, sosa:Procedure;
  dct:description "A procedure for measuring Extractable Manganese"@en;
  dct:identifier "http://anzsoil.org/def/soil/au/edu/fed-uni/procedure/12A1-MN"^^xsd:anyURI;
  rdfs:label "DTPA - Extractable Manganese procedure"@en;
  skos:definition "A procedure for measuring Extractable Manganese"@en;
  skos:inScheme <http://anzoil.org/def/soil/au/edu/fed-uni>;
  skos:notation "12A1-MN";
  skos:prefLabel "DTPA - Extractable Manganese procedure"@en;
  skos:topConceptOf <http://anzoil.org/def/soil/au/edu/fed-uni> .

procedure:12A1-ZN a skos:Concept, sosa:Procedure;
  dct:description "A procedure for measuring Extractable Zinc DTPA"@en;
  dct:identifier "http://anzsoil.org/def/soil/au/edu/fed-uni/procedure/12A1-ZN"^^xsd:anyURI;
  rdfs:label "DTPA - Extractable Zinc procedure"@en;
  skos:definition "A procedure for measuring Extractable Zinc DTPA"@en;
  skos:inScheme <http://anzoil.org/def/soil/au/edu/fed-uni>;
  skos:notation "12A1-ZN";
  skos:prefLabel "DTPA - Extractable Zinc procedure"@en;
  skos:topConceptOf <http://anzoil.org/def/soil/au/edu/fed-uni> .

procedure:12B1-CO a skos:Concept, sosa:Procedure;
  dct:description "A procedure for measuring Extractable Copper Ammonium bicarbonate/EDTA"@en;
  dct:identifier "http://anzsoil.org/def/soil/au/edu/fed-uni/procedure/12B1-CO"^^xsd:anyURI;
  rdfs:label "Extractable Copper procedure - Ammonium bicarbonate/EDTA"@en;
  skos:definition "A procedure for measuring Extractable Copper Ammonium bicarbonate/EDTA"@en;
  skos:inScheme <http://anzoil.org/def/soil/au/edu/fed-uni>;
  skos:notation "12B1-CO";
  skos:prefLabel "Extractable Copper procedure - Ammonium bicarbonate/EDTA"@en;
  skos:topConceptOf <http://anzoil.org/def/soil/au/edu/fed-uni> .

procedure:12B1-CU a skos:Concept, sosa:Procedure;
  dct:description "A procedure for measuring Extractable Copper Ammonium Bicarbonate/EDTA"@en;
  dct:identifier "http://anzsoil.org/def/soil/au/edu/fed-uni/procedure/12B1-CU"^^xsd:anyURI;
  rdfs:label "Ammonium bicarbonate/EDTA - Extractable Copper procedure"@en;
  skos:definition "A procedure for measuring Extractable Copper Ammonium Bicarbonate/EDTA"@en;
  skos:inScheme <http://anzoil.org/def/soil/au/edu/fed-uni>;
  skos:notation "12B1-CU";
  skos:prefLabel "Ammonium bicarbonate/EDTA - Extractable Copper procedure"@en;
  skos:topConceptOf <http://anzoil.org/def/soil/au/edu/fed-uni> .

procedure:12B1-ZN a skos:Concept, sosa:Procedure;
  dct:description "A procedure for measuring Extractable Zinc Ammonium Bicarbonate/EDTA"@en;
  dct:identifier "http://anzsoil.org/def/soil/au/edu/fed-uni/procedure/12B1-ZN"^^xsd:anyURI;
  rdfs:label "Ammonium bicarbonate/EDTA - Extractable Zinc procedure"@en;
  skos:definition "A procedure for measuring Extractable Zinc Ammonium Bicarbonate/EDTA"@en;
  skos:inScheme <http://anzoil.org/def/soil/au/edu/fed-uni>;
  skos:notation "12B1-ZN";
  skos:prefLabel "Ammonium bicarbonate/EDTA - Extractable Zinc procedure"@en;
  skos:topConceptOf <http://anzoil.org/def/soil/au/edu/fed-uni> .

procedure:12C a skos:Concept, sosa:Procedure;
  dct:description "A procedure for measuring Extractable Boron - Calcium chloride-extractable"@en;
  dct:identifier "http://anzsoil.org/def/soil/au/edu/fed-uni/procedure/12C"^^xsd:anyURI;
  rdfs:label "Extractable Boron - Calcium chloride procedure"@en;
  skos:definition "A procedure for measuring Extractable Boron - Calcium chloride-extractable"@en;
  skos:inScheme <http://anzoil.org/def/soil/au/edu/fed-uni>;
  skos:notation "12C";
  skos:prefLabel "Extractable Boron - Calcium chloride procedure"@en;
  skos:topConceptOf <http://anzoil.org/def/soil/au/edu/fed-uni> .

procedure:12D1-CU a skos:Concept, sosa:Procedure;
  dct:description "A procedure for measuring Extractable Copper 0.1 M HCl-extractable"@en;
  dct:identifier "http://anzsoil.org/def/soil/au/edu/fed-uni/procedure/12D1-CU"^^xsd:anyURI;
  rdfs:label "0.1 M HCl-extractable Cu procedure"@en;
  skos:definition "A procedure for measuring Extractable Copper 0.1 M HCl-extractable"@en;
  skos:inScheme <http://anzoil.org/def/soil/au/edu/fed-uni>;
  skos:notation "12D1-CU";
  skos:prefLabel "0.1 M HCl-extractable Cu procedure"@en;
  skos:topConceptOf <http://anzoil.org/def/soil/au/edu/fed-uni> .

procedure:12D1-FE a skos:Concept, sosa:Procedure;
  dct:description "A procedure for measuring Extractable Iron - 0.1 M HCl-extractable"@en;
  dct:identifier "http://anzsoil.org/def/soil/au/edu/fed-uni/procedure/12D1-FE"^^xsd:anyURI;
  rdfs:label "0.1 M HCl-extractable Fe procedure"@en;
  skos:definition "A procedure for measuring Extractable Iron - 0.1 M HCl-extractable"@en;
  skos:inScheme <http://anzoil.org/def/soil/au/edu/fed-uni>;
  skos:notation "12D1-FE";
  skos:prefLabel "0.1 M HCl-extractable Fe procedure"@en;
  skos:topConceptOf <http://anzoil.org/def/soil/au/edu/fed-uni> .

procedure:12D1-MN a skos:Concept, sosa:Procedure;
  dct:description "A procedure for measuring Extractable Manganese 0.1 M HCl-extractable"@en;
  dct:identifier "http://anzsoil.org/def/soil/au/edu/fed-uni/procedure/12D1-MN"^^xsd:anyURI;
  rdfs:label "0.1 M HCl-extractable Mn procedure"@en;
  skos:definition "A procedure for measuring Extractable Manganese 0.1 M HCl-extractable"@en;
  skos:inScheme <http://anzoil.org/def/soil/au/edu/fed-uni>;
  skos:notation "12D1-MN";
  skos:prefLabel "0.1 M HCl-extractable Mn procedure"@en;
  skos:topConceptOf <http://anzoil.org/def/soil/au/edu/fed-uni> .

procedure:12D1-ZN a skos:Concept, sosa:Procedure;
  dct:description "A procedure for measuring Extractable Zinc - 0.1 M HCl-extractable"@en;
  dct:identifier "http://anzsoil.org/def/soil/au/edu/fed-uni/procedure/12D1-ZN"^^xsd:anyURI;
  rdfs:label "0.1 M HCl-extractable Zn procedure"@en;
  skos:definition "A procedure for measuring Extractable Zinc - 0.1 M HCl-extractable"@en;
  skos:inScheme <http://anzoil.org/def/soil/au/edu/fed-uni>;
  skos:notation "12D1-ZN";
  skos:prefLabel "0.1 M HCl-extractable Zn procedure"@en;
  skos:topConceptOf <http://anzoil.org/def/soil/au/edu/fed-uni> .

procedure:13A1-FE a skos:Concept, sosa:Procedure;
  dct:description "A procedure for measuing Iron by oxalate-extraction"@en;
  dct:identifier "http://anzsoil.org/def/soil/au/edu/fed-uni/procedure/13A1-FE"^^xsd:anyURI;
  rdfs:label "Iron procedure - oxalate-extraction"@en;
  skos:definition "A procedure for measuing Iron by oxalate-extraction"@en;
  skos:inScheme <http://anzoil.org/def/soil/au/edu/fed-uni>;
  skos:notation "13A1-FE";
  skos:prefLabel "Iron procedure - oxalate-extraction"@en;
  skos:topConceptOf <http://anzoil.org/def/soil/au/edu/fed-uni> .

procedure:15D2-MG a skos:Concept, sosa:Procedure;
  dct:description "A procedure for measuring Exchangeable Magnesium (Mg2+) 1M ammonium acetate at pH 7.0, pretreatment for soluble salts; automati"@en;
  dct:identifier "http://anzsoil.org/def/soil/au/edu/fed-uni/procedure/15D2-MG"^^xsd:anyURI;
  rdfs:label "Exchangeable Magnesium Mg2+ procedure - 1M ammonium acetate at pH 7.0, pretreatment for soluble salts; automatic extractor"@en;
  skos:definition "A procedure for measuring Exchangeable Magnesium (Mg2+) 1M ammonium acetate at pH 7.0, pretreatment for soluble salts; automati"@en;
  skos:inScheme <http://anzoil.org/def/soil/au/edu/fed-uni>;
  skos:notation "15D2-MG";
  skos:prefLabel "Exchangeable Magnesium Mg2+ procedure - 1M ammonium acetate at pH 7.0, pretreatment for soluble salts; automatic extractor"@en;
  skos:topConceptOf <http://anzoil.org/def/soil/au/edu/fed-uni> .

procedure:15D2-NA a skos:Concept, sosa:Procedure;
  dct:description "A procedure for measuring Exchangeable Sodium (Na+) 1M ammonium acetate at pH 7.0, pretreatment for soluble salts; automatic"@en;
  dct:identifier "http://anzsoil.org/def/soil/au/edu/fed-uni/procedure/15D2-NA"^^xsd:anyURI;
  rdfs:label "Exchangeable Sodium Na+ procedure - 1M ammonium acetate at pH 7.0, pretreatment for soluble salts; automatic extractor"@en;
  skos:definition "A procedure for measuring Exchangeable Sodium (Na+) 1M ammonium acetate at pH 7.0, pretreatment for soluble salts; automatic"@en;
  skos:inScheme <http://anzoil.org/def/soil/au/edu/fed-uni>;
  skos:notation "15D2-NA";
  skos:prefLabel "Exchangeable Sodium Na+ procedure - 1M ammonium acetate at pH 7.0, pretreatment for soluble salts; automatic extractor"@en;
  skos:topConceptOf <http://anzoil.org/def/soil/au/edu/fed-uni> .

procedure:15D3-15G1-ECEC a skos:Concept, sosa:Procedure;
  dct:description "A procedure for measuring Effective Cation Exchange Capacity, (ECEC) where effective cation exchange capacity equals Exchangeable bases and CEC - 1 M ammonium acetate at pH 7.0, rapid method with no pre-treatment for soluble salts plus Exchange acidity (H+ + Al3+) 1 M potassium chloride."@en;
  dct:identifier "http://anzsoil.org/def/soil/au/edu/fed-uni/procedure/15D3-15G1-ECEC"^^xsd:anyURI;
  rdfs:label "Effective Cation Exchange Capacity procedure - ammonium acetate and KCl"@en;
  skos:definition "A procedure for measuring Effective Cation Exchange Capacity, (ECEC) where effective cation exchange capacity equals Exchangeable bases and CEC - 1 M ammonium acetate at pH 7.0, rapid method with no pre-treatment for soluble salts plus Exchange acidity (H+ + Al3+) 1 M potassium chloride."@en;
  skos:inScheme <http://anzoil.org/def/soil/au/edu/fed-uni>;
  skos:notation "15D3-15G1-ECEC";
  skos:prefLabel "Effective Cation Exchange Capacity procedure - ammonium acetate and KCl"@en;
  skos:topConceptOf <http://anzoil.org/def/soil/au/edu/fed-uni> .

procedure:15D3-15G1-ECEC-CA a skos:Concept, sosa:Procedure;
  dct:description "A procedure for measuring Calcium as a percentage of Effective Cation Exchange Capacity, where Effective Cation Exchange Capacity equals exchangeable bases and CEC - 1 M ammonium acetate at pH 7.0, rapid method with no pre-treatment for soluble salts plus Exchange acidity (H+ + Al3+) 1 M potassium chloride"@en;
  dct:identifier "http://anzsoil.org/def/soil/au/edu/fed-uni/procedure/15D3-15G1-ECEC-CA"^^xsd:anyURI;
  rdfs:label "Calcium as a percentage of Effective Cation Exchange Capacity procedure"@en;
  skos:definition "A procedure for measuring Calcium as a percentage of Effective Cation Exchange Capacity, where Effective Cation Exchange Capacity equals exchangeable bases and CEC - 1 M ammonium acetate at pH 7.0, rapid method with no pre-treatment for soluble salts plus Exchange acidity (H+ + Al3+) 1 M potassium chloride"@en;
  skos:inScheme <http://anzoil.org/def/soil/au/edu/fed-uni>;
  skos:notation "15D3-15G1-ECEC-CA";
  skos:prefLabel "Calcium as a percentage of Effective Cation Exchange Capacity procedure"@en;
  skos:topConceptOf <http://anzoil.org/def/soil/au/edu/fed-uni> .

procedure:15D3-15G1-ECEC-K a skos:Concept, sosa:Procedure;
  dct:description "A procedure for measuring Potassium as a percentage of Effective Cation Exchange Capacity, where Effective Cation Exchange Capacity equals exchangeable bases and CEC- 1 M ammonium acetate at pH 7.0, rapid method with no pre-treatment for soluble salts plus Exchange acidity (H+ + Al3+) 1 M potassium chloride."@en;
  dct:identifier "http://anzsoil.org/def/soil/au/edu/fed-uni/procedure/15D3-15G1-ECEC-K"^^xsd:anyURI;
  rdfs:label "Potassium as a percentage of Effective Cation Exchange Capacity procedure"@en;
  skos:definition "A procedure for measuring Potassium as a percentage of Effective Cation Exchange Capacity, where Effective Cation Exchange Capacity equals exchangeable bases and CEC- 1 M ammonium acetate at pH 7.0, rapid method with no pre-treatment for soluble salts plus Exchange acidity (H+ + Al3+) 1 M potassium chloride."@en;
  skos:inScheme <http://anzoil.org/def/soil/au/edu/fed-uni>;
  skos:notation "15D3-15G1-ECEC-K";
  skos:prefLabel "Potassium as a percentage of Effective Cation Exchange Capacity procedure"@en;
  skos:topConceptOf <http://anzoil.org/def/soil/au/edu/fed-uni> .

procedure:15D3-15G1-ECEC-MG a skos:Concept, sosa:Procedure;
  dct:description "A procedure for measuring Magnesium as a percentage of Effective Cation Exchange Capacity, where Effective Cation Exchange Capacity equals exchangeable bases and CEC - 1 M ammonium acetate at pH 7.0, rapid method with no pre-treatment for soluble salts plus Exchange acidity (H+ + Al3+) 1 M potassium chloride."@en;
  dct:identifier "http://anzsoil.org/def/soil/au/edu/fed-uni/procedure/15D3-15G1-ECEC-MG"^^xsd:anyURI;
  rdfs:label "Magnesium as a percentage of Effective Cation Exchange Capacity procedure"@en;
  skos:definition "A procedure for measuring Magnesium as a percentage of Effective Cation Exchange Capacity, where Effective Cation Exchange Capacity equals exchangeable bases and CEC - 1 M ammonium acetate at pH 7.0, rapid method with no pre-treatment for soluble salts plus Exchange acidity (H+ + Al3+) 1 M potassium chloride."@en;
  skos:inScheme <http://anzoil.org/def/soil/au/edu/fed-uni>;
  skos:notation "15D3-15G1-ECEC-MG";
  skos:prefLabel "Magnesium as a percentage of Effective Cation Exchange Capacity procedure"@en;
  skos:topConceptOf <http://anzoil.org/def/soil/au/edu/fed-uni> .

procedure:15D3-15G1-ECEC-NA a skos:Concept, sosa:Procedure;
  dct:description "A procedure for measuring Sodium as a percentage of Effective Cation Exchange Capacity, where Effective Cation Exchange Capacity equals exchangeable bases and CEC - 1 M ammonium acetate at pH 7.0, rapid method with no pre-treatment for soluble salts plus Exchange acidity (H+ + Al3+) 1 M potassium chloride."@en;
  dct:identifier "http://anzsoil.org/def/soil/au/edu/fed-uni/procedure/15D3-15G1-ECEC-NA"^^xsd:anyURI;
  rdfs:label "Sodium as a percentage of Effective Cation Exchange Capacity procedure"@en;
  skos:definition "A procedure for measuring Sodium as a percentage of Effective Cation Exchange Capacity, where Effective Cation Exchange Capacity equals exchangeable bases and CEC - 1 M ammonium acetate at pH 7.0, rapid method with no pre-treatment for soluble salts plus Exchange acidity (H+ + Al3+) 1 M potassium chloride."@en;
  skos:inScheme <http://anzoil.org/def/soil/au/edu/fed-uni>;
  skos:notation "15D3-15G1-ECEC-NA";
  skos:prefLabel "Sodium as a percentage of Effective Cation Exchange Capacity procedure"@en;
  skos:topConceptOf <http://anzoil.org/def/soil/au/edu/fed-uni> .

procedure:15D3-CA a skos:Concept, sosa:Procedure;
  dct:description "A procedure for measuring Exchangeable Calcium (Ca2+) 1M ammonium acetate at pH 7.0, rapid method with no pretreatment for soluble salts"@en;
  dct:identifier "http://anzsoil.org/def/soil/au/edu/fed-uni/procedure/15D3-CA"^^xsd:anyURI;
  rdfs:label "Exchangeable Calcium Ca2+ procedure - 1M ammonium acetate at pH 7.0, rapid method with no pretreatment for soluble salts"@en;
  skos:definition "A procedure for measuring Exchangeable Calcium (Ca2+) 1M ammonium acetate at pH 7.0, rapid method with no pretreatment for soluble salts"@en;
  skos:inScheme <http://anzoil.org/def/soil/au/edu/fed-uni>;
  skos:notation "15D3-CA";
  skos:prefLabel "Exchangeable Calcium Ca2+ procedure - 1M ammonium acetate at pH 7.0, rapid method with no pretreatment for soluble salts"@en;
  skos:topConceptOf <http://anzoil.org/def/soil/au/edu/fed-uni> .

procedure:15D3-CEC-CA a skos:Concept, sosa:Procedure;
  dct:description "A procedure for measuring Exchangeable calcium as % of Cation Exhange Capacity (CEC) 1 M ammonium acetate at pH 7.0, rapid method with no pre-treatment for soluble salts"@en;
  dct:identifier "http://anzsoil.org/def/soil/au/edu/fed-uni/procedure/15D3-CEC-CA"^^xsd:anyURI;
  rdfs:label "Exchangeable Calcium as % of cation exhange capacity (CEC) procedure - 1 M ammonium acetate at pH 7.0, rapid method with no pre-treatment for soluble salts"@en;
  skos:definition "A procedure for measuring Exchangeable calcium as % of Cation Exhange Capacity (CEC) 1 M ammonium acetate at pH 7.0, rapid method with no pre-treatment for soluble salts"@en;
  skos:inScheme <http://anzoil.org/def/soil/au/edu/fed-uni>;
  skos:notation "15D3-CEC-CA";
  skos:prefLabel "Exchangeable Calcium as % of cation exhange capacity (CEC) procedure - 1 M ammonium acetate at pH 7.0, rapid method with no pre-treatment for soluble salts"@en;
  skos:topConceptOf <http://anzoil.org/def/soil/au/edu/fed-uni> .

procedure:15D3-CEC-K a skos:Concept, sosa:Procedure;
  dct:description "A procedure for measuring Exchangeable Potassium as % of Cation Exhange Capacity (CEC) 1 M ammonium acetate at pH 7.0, rapid method with no pre-treatment for soluble salts"@en;
  dct:identifier "http://anzsoil.org/def/soil/au/edu/fed-uni/procedure/15D3-CEC-K"^^xsd:anyURI;
  rdfs:label "Exchangeable Potassium as % of cation exhange capacity (CEC) procedure - 1 M ammonium acetate at pH 7.0, rapid method with no pre-treatment for soluble salts."@en;
  skos:definition "A procedure for measuring Exchangeable Potassium as % of Cation Exhange Capacity (CEC) 1 M ammonium acetate at pH 7.0, rapid method with no pre-treatment for soluble salts"@en;
  skos:inScheme <http://anzoil.org/def/soil/au/edu/fed-uni>;
  skos:notation "15D3-CEC-K";
  skos:prefLabel "Exchangeable Potassium as % of cation exhange capacity (CEC) procedure - 1 M ammonium acetate at pH 7.0, rapid method with no pre-treatment for soluble salts."@en;
  skos:topConceptOf <http://anzoil.org/def/soil/au/edu/fed-uni> .

procedure:15D3-CEC-MG a skos:Concept, sosa:Procedure;
  dct:description "A procedure for measuring Exchangeable magnesium as % of Cation Exhange Capacity (CEC) 1 M ammonium acetate at pH 7.0, rapid method with no pre-treatment for soluble salts"@en;
  dct:identifier "http://anzsoil.org/def/soil/au/edu/fed-uni/procedure/15D3-CEC-MG"^^xsd:anyURI;
  rdfs:label "Exchangeable Magnesium as % of cation exhange capacity (CEC) procedure - 1 M ammonium acetate at pH 7.0, rapid method with no pre-treatment for soluble salts"@en;
  skos:definition "A procedure for measuring Exchangeable magnesium as % of Cation Exhange Capacity (CEC) 1 M ammonium acetate at pH 7.0, rapid method with no pre-treatment for soluble salts"@en;
  skos:inScheme <http://anzoil.org/def/soil/au/edu/fed-uni>;
  skos:notation "15D3-CEC-MG";
  skos:prefLabel "Exchangeable Magnesium as % of cation exhange capacity (CEC) procedure - 1 M ammonium acetate at pH 7.0, rapid method with no pre-treatment for soluble salts"@en;
  skos:topConceptOf <http://anzoil.org/def/soil/au/edu/fed-uni> .

procedure:15D3-CEC-NA a skos:Concept, sosa:Procedure;
  dct:description "A procedure for measuring Exchangeable sodium as % of Cation Exhange Capacity (CEC) 1 M ammonium acetate at pH 7.0, rapid method with no pre-treatment for soluble salts"@en;
  dct:identifier "http://anzsoil.org/def/soil/au/edu/fed-uni/procedure/15D3-CEC-NA"^^xsd:anyURI;
  rdfs:label "Exchangeable Sodium as % of cation exhange capacity (CEC) procedure - 1 M ammonium acetate at pH 7.0, rapid method with no pre-treatment for soluble salts"@en;
  skos:definition "A procedure for measuring Exchangeable sodium as % of Cation Exhange Capacity (CEC) 1 M ammonium acetate at pH 7.0, rapid method with no pre-treatment for soluble salts"@en;
  skos:inScheme <http://anzoil.org/def/soil/au/edu/fed-uni>;
  skos:notation "15D3-CEC-NA";
  skos:prefLabel "Exchangeable Sodium as % of cation exhange capacity (CEC) procedure - 1 M ammonium acetate at pH 7.0, rapid method with no pre-treatment for soluble salts"@en;
  skos:topConceptOf <http://anzoil.org/def/soil/au/edu/fed-uni> .

procedure:15D3-ECR a skos:Concept, sosa:Procedure;
  dct:description "A procedure for measuring Exchangeable Cation Ratio (ECR), where ECR=100*(Na + K)/(Na + K + Ca + Mg)"@en;
  dct:identifier "http://anzsoil.org/def/soil/au/edu/fed-uni/procedure/15D3-ECR"^^xsd:anyURI;
  rdfs:label "Exchangable Cation Ratio procedure"@en;
  skos:definition "A procedure for measuring Exchangeable Cation Ratio (ECR), where ECR=100*(Na + K)/(Na + K + Ca + Mg)"@en;
  skos:inScheme <http://anzoil.org/def/soil/au/edu/fed-uni>;
  skos:notation "15D3-ECR";
  skos:prefLabel "Exchangable Cation Ratio procedure"@en;
  skos:topConceptOf <http://anzoil.org/def/soil/au/edu/fed-uni> .

procedure:15D3-GTRI a skos:Concept, sosa:Procedure;
  dct:description "A procedure for measuring Grass Tetany Risk Index (GTRI) specific for pasture, where GTRI=K/(Ca + Mg) measured using 15D3 [Soil Chemical Methods Australasia 1. (2011), George E Rayment and David J Lyons]"@en;
  dct:identifier "http://anzsoil.org/def/soil/au/edu/fed-uni/procedure/15D3-GTRI"^^xsd:anyURI;
  rdfs:label "15D3 - Grass tetany risk index procedure"@en;
  skos:definition "A procedure for measuring Grass Tetany Risk Index (GTRI) specific for pasture, where GTRI=K/(Ca + Mg) measured using 15D3 [Soil Chemical Methods Australasia 1. (2011), George E Rayment and David J Lyons]"@en;
  skos:inScheme <http://anzoil.org/def/soil/au/edu/fed-uni>;
  skos:notation "15D3-GTRI";
  skos:prefLabel "15D3 - Grass tetany risk index procedure"@en;
  skos:topConceptOf <http://anzoil.org/def/soil/au/edu/fed-uni> .

procedure:15D3-K a skos:Concept, sosa:Procedure;
  dct:description "A procedure for measuring Exchangeable Potassium (K+) 1M ammonium acetate at pH 7.0, rapid method with no pretreatment for soluble salts"@en;
  dct:identifier "http://anzsoil.org/def/soil/au/edu/fed-uni/procedure/15D3-K"^^xsd:anyURI;
  rdfs:label "Exchangeable Potassium K+ procedure - 1M ammonium acetate at pH 7.0, rapid method with no pretreatment for soluble salts"@en;
  skos:definition "A procedure for measuring Exchangeable Potassium (K+) 1M ammonium acetate at pH 7.0, rapid method with no pretreatment for soluble salts"@en;
  skos:inScheme <http://anzoil.org/def/soil/au/edu/fed-uni>;
  skos:notation "15D3-K";
  skos:prefLabel "Exchangeable Potassium K+ procedure - 1M ammonium acetate at pH 7.0, rapid method with no pretreatment for soluble salts"@en;
  skos:topConceptOf <http://anzoil.org/def/soil/au/edu/fed-uni> .

procedure:15D3-MG a skos:Concept, sosa:Procedure;
  dct:description "A procedure for measuring Exchangeable Magnesium (Mg2+) 1M ammonium acetate at pH 7.0, rapid method with no pretreatment for soluble salts"@en;
  dct:identifier "http://anzsoil.org/def/soil/au/edu/fed-uni/procedure/15D3-MG"^^xsd:anyURI;
  rdfs:label "Exchangeable Magnesium Mg2+ procedure - 1M ammonium acetate at pH 7.0, rapid method with no pretreatment for soluble salts"@en;
  skos:definition "A procedure for measuring Exchangeable Magnesium (Mg2+) 1M ammonium acetate at pH 7.0, rapid method with no pretreatment for soluble salts"@en;
  skos:inScheme <http://anzoil.org/def/soil/au/edu/fed-uni>;
  skos:notation "15D3-MG";
  skos:prefLabel "Exchangeable Magnesium Mg2+ procedure - 1M ammonium acetate at pH 7.0, rapid method with no pretreatment for soluble salts"@en;
  skos:topConceptOf <http://anzoil.org/def/soil/au/edu/fed-uni> .

procedure:15D3-NA a skos:Concept, sosa:Procedure;
  dct:description "A procedure for measuring Exchangeable Sodium (Na+) 1M ammonium acetate at pH 7.0, rapid method with no pretreatment for soluble salts"@en;
  dct:identifier "http://anzsoil.org/def/soil/au/edu/fed-uni/procedure/15D3-NA"^^xsd:anyURI;
  rdfs:label "Exchangeable Sodium procedure - 1M ammonium acetate at pH 7.0, rapid method with no pretreatment for soluble salts"@en;
  skos:definition "A procedure for measuring Exchangeable Sodium (Na+) 1M ammonium acetate at pH 7.0, rapid method with no pretreatment for soluble salts"@en;
  skos:inScheme <http://anzoil.org/def/soil/au/edu/fed-uni>;
  skos:notation "15D3-NA";
  skos:prefLabel "Exchangeable Sodium procedure - 1M ammonium acetate at pH 7.0, rapid method with no pretreatment for soluble salts"@en;
  skos:topConceptOf <http://anzoil.org/def/soil/au/edu/fed-uni> .

procedure:15E1-AL a skos:Concept, sosa:Procedure;
  dct:description "A procedure for measuring Exchangeable Aluminium (Al3+) compulsive exchange, no pre-treatment for soluble salts"@en;
  dct:identifier "http://anzsoil.org/def/soil/au/edu/fed-uni/procedure/15E1-AL"^^xsd:anyURI;
  rdfs:label "Exchangeable Aluminium Al3+ procedure - compulsive exchange, no pre-treatment for soluble salts"@en;
  skos:definition "A procedure for measuring Exchangeable Aluminium (Al3+) compulsive exchange, no pre-treatment for soluble salts"@en;
  skos:inScheme <http://anzoil.org/def/soil/au/edu/fed-uni>;
  skos:notation "15E1-AL";
  skos:prefLabel "Exchangeable Aluminium Al3+ procedure - compulsive exchange, no pre-treatment for soluble salts"@en;
  skos:topConceptOf <http://anzoil.org/def/soil/au/edu/fed-uni> .

procedure:15E1-CA a skos:Concept, sosa:Procedure;
  dct:description "A procedure for measuring Exchangeable Calcium (Ca2+) compulsive exchange, no pre-treatment for soluble salts"@en;
  dct:identifier "http://anzsoil.org/def/soil/au/edu/fed-uni/procedure/15E1-CA"^^xsd:anyURI;
  rdfs:label "Exchangeable Calcium Ca2+ procedure - compulsive exchange, no pre-treatment for soluble salts"@en;
  skos:definition "A procedure for measuring Exchangeable Calcium (Ca2+) compulsive exchange, no pre-treatment for soluble salts"@en;
  skos:inScheme <http://anzoil.org/def/soil/au/edu/fed-uni>;
  skos:notation "15E1-CA";
  skos:prefLabel "Exchangeable Calcium Ca2+ procedure - compulsive exchange, no pre-treatment for soluble salts"@en;
  skos:topConceptOf <http://anzoil.org/def/soil/au/edu/fed-uni> .

procedure:15E1-K a skos:Concept, sosa:Procedure;
  dct:description "A procedure for measuring Exchangeable Potassium (K+) compulsive exchange, no pre-treatment for soluble salts"@en;
  dct:identifier "http://anzsoil.org/def/soil/au/edu/fed-uni/procedure/15E1-K"^^xsd:anyURI;
  rdfs:label "Exchangeable Potassium K+ procedure - compulsive exchange, no pre-treatment for soluble salts"@en;
  skos:definition "A procedure for measuring Exchangeable Potassium (K+) compulsive exchange, no pre-treatment for soluble salts"@en;
  skos:inScheme <http://anzoil.org/def/soil/au/edu/fed-uni>;
  skos:notation "15E1-K";
  skos:prefLabel "Exchangeable Potassium K+ procedure - compulsive exchange, no pre-treatment for soluble salts"@en;
  skos:topConceptOf <http://anzoil.org/def/soil/au/edu/fed-uni> .

procedure:15E1-MG a skos:Concept, sosa:Procedure;
  dct:description "A procedure for measuring Exchangeable Magnesium (Mg2+) compulsive exchange, no pre-treatment for soluble salts"@en;
  dct:identifier "http://anzsoil.org/def/soil/au/edu/fed-uni/procedure/15E1-MG"^^xsd:anyURI;
  rdfs:label "Exchangeable Magnesium Mg2+ procedure - compulsive exchange, no pre-treatment for soluble salts"@en;
  skos:definition "A procedure for measuring Exchangeable Magnesium (Mg2+) compulsive exchange, no pre-treatment for soluble salts"@en;
  skos:inScheme <http://anzoil.org/def/soil/au/edu/fed-uni>;
  skos:notation "15E1-MG";
  skos:prefLabel "Exchangeable Magnesium Mg2+ procedure - compulsive exchange, no pre-treatment for soluble salts"@en;
  skos:topConceptOf <http://anzoil.org/def/soil/au/edu/fed-uni> .

procedure:15E1-NA a skos:Concept, sosa:Procedure;
  dct:description "A procedure for measuring Exchangeable Sodium (Na+) compulsive exchange, no pre-treatment for soluble salts"@en;
  dct:identifier "http://anzsoil.org/def/soil/au/edu/fed-uni/procedure/15E1-NA"^^xsd:anyURI;
  rdfs:label "Exchangeable Sodium Na+ procedure - compulsive exchange, no pre-treatment for soluble salts"@en;
  skos:definition "A procedure for measuring Exchangeable Sodium (Na+) compulsive exchange, no pre-treatment for soluble salts"@en;
  skos:inScheme <http://anzoil.org/def/soil/au/edu/fed-uni>;
  skos:notation "15E1-NA";
  skos:prefLabel "Exchangeable Sodium Na+ procedure - compulsive exchange, no pre-treatment for soluble salts"@en;
  skos:topConceptOf <http://anzoil.org/def/soil/au/edu/fed-uni> .

procedure:15E2-CA a skos:Concept, sosa:Procedure;
  dct:description "A procedure for measuring Exchangeable Calcium (Ca2+) compulsive exchange, pretreatment for soluble salts"@en;
  dct:identifier "http://anzsoil.org/def/soil/au/edu/fed-uni/procedure/15E2-CA"^^xsd:anyURI;
  rdfs:label "Exchangeable Calcium Ca2+ procedure - compulsive exchange, pretreatment for soluble salts"@en;
  skos:definition "A procedure for measuring Exchangeable Calcium (Ca2+) compulsive exchange, pretreatment for soluble salts"@en;
  skos:inScheme <http://anzoil.org/def/soil/au/edu/fed-uni>;
  skos:notation "15E2-CA";
  skos:prefLabel "Exchangeable Calcium Ca2+ procedure - compulsive exchange, pretreatment for soluble salts"@en;
  skos:topConceptOf <http://anzoil.org/def/soil/au/edu/fed-uni> .

procedure:15E2-K a skos:Concept, sosa:Procedure;
  dct:description "A procedure for measuring Exchangeable Potassium (K+) compulsive exchange, pretreatment for soluble salts"@en;
  dct:identifier "http://anzsoil.org/def/soil/au/edu/fed-uni/procedure/15E2-K"^^xsd:anyURI;
  rdfs:label "Exchangeable Potassium K+ procedure - compulsive exchange, pretreatment for soluble salts"@en;
  skos:definition "A procedure for measuring Exchangeable Potassium (K+) compulsive exchange, pretreatment for soluble salts"@en;
  skos:inScheme <http://anzoil.org/def/soil/au/edu/fed-uni>;
  skos:notation "15E2-K";
  skos:prefLabel "Exchangeable Potassium K+ procedure - compulsive exchange, pretreatment for soluble salts"@en;
  skos:topConceptOf <http://anzoil.org/def/soil/au/edu/fed-uni> .

procedure:15E2-MG a skos:Concept, sosa:Procedure;
  dct:description "A procedure for measuring Exchangeable Magnesium (Mg2+) compulsive exchange, pretreatment for soluble salts"@en;
  dct:identifier "http://anzsoil.org/def/soil/au/edu/fed-uni/procedure/15E2-MG"^^xsd:anyURI;
  rdfs:label "Exchangeable Magnesium Mg2+ procedure - compulsive exchange, pretreatment for soluble salts"@en;
  skos:definition "A procedure for measuring Exchangeable Magnesium (Mg2+) compulsive exchange, pretreatment for soluble salts"@en;
  skos:inScheme <http://anzoil.org/def/soil/au/edu/fed-uni>;
  skos:notation "15E2-MG";
  skos:prefLabel "Exchangeable Magnesium Mg2+ procedure - compulsive exchange, pretreatment for soluble salts"@en;
  skos:topConceptOf <http://anzoil.org/def/soil/au/edu/fed-uni> .

procedure:15E2-NA a skos:Concept, sosa:Procedure;
  dct:description "A procedure for measuring Exchangeable Sodium (Na+) compulsive exchange, pretreatment for soluble salts"@en;
  dct:identifier "http://anzsoil.org/def/soil/au/edu/fed-uni/procedure/15E2-NA"^^xsd:anyURI;
  rdfs:label "Exchangeable Sodium Na+ procedure - compulsive exchange, pretreatment for soluble salts"@en;
  skos:definition "A procedure for measuring Exchangeable Sodium (Na+) compulsive exchange, pretreatment for soluble salts"@en;
  skos:inScheme <http://anzoil.org/def/soil/au/edu/fed-uni>;
  skos:notation "15E2-NA";
  skos:prefLabel "Exchangeable Sodium Na+ procedure - compulsive exchange, pretreatment for soluble salts"@en;
  skos:topConceptOf <http://anzoil.org/def/soil/au/edu/fed-uni> .

procedure:15G1-15D3-ECEC-AL a skos:Concept, sosa:Procedure;
  dct:description "A procedure for measuring Aluminium as a percentage of Effective Cation Exchange Capacity, where Effective Cation Exchange Capacity equals exchangeable bases and CEC - 1 M ammonium acetate at pH 7.0, rapid method with no pre-treatment for soluble salts plus Exchange acidity (H+ + Al3+) 1 M potassium chloride"@en;
  dct:identifier "http://anzsoil.org/def/soil/au/edu/fed-uni/procedure/15G1-15D3-ECEC-AL"^^xsd:anyURI;
  rdfs:label "Aluminium as a percentage of Effective Cation Exchange Capacity procedure"@en;
  skos:definition "A procedure for measuring Aluminium as a percentage of Effective Cation Exchange Capacity, where Effective Cation Exchange Capacity equals exchangeable bases and CEC - 1 M ammonium acetate at pH 7.0, rapid method with no pre-treatment for soluble salts plus Exchange acidity (H+ + Al3+) 1 M potassium chloride"@en;
  skos:inScheme <http://anzoil.org/def/soil/au/edu/fed-uni>;
  skos:notation "15G1-15D3-ECEC-AL";
  skos:prefLabel "Aluminium as a percentage of Effective Cation Exchange Capacity procedure"@en;
  skos:topConceptOf <http://anzoil.org/def/soil/au/edu/fed-uni> .

procedure:15G1-15D3-ECEC-H a skos:Concept, sosa:Procedure;
  dct:description "A procedure for measuring Hydrogen H+ as a percentage of Effective Cation Exchange Capacity, where Effective Cation Exchange Capacity equals exchangeable bases and CEC - 1 M ammonium acetate at pH 7.0, rapid method with no pre-treatment for soluble salts plus Exchange acidity (H+ + Al3+) 1 M potassium chloride."@en;
  dct:identifier "http://anzsoil.org/def/soil/au/edu/fed-uni/procedure/15G1-15D3-ECEC-H"^^xsd:anyURI;
  rdfs:label "Hydrogen H+ as a percentage of Effective Cation Exchange Capacity procedure"@en;
  skos:definition "A procedure for measuring Hydrogen H+ as a percentage of Effective Cation Exchange Capacity, where Effective Cation Exchange Capacity equals exchangeable bases and CEC - 1 M ammonium acetate at pH 7.0, rapid method with no pre-treatment for soluble salts plus Exchange acidity (H+ + Al3+) 1 M potassium chloride."@en;
  skos:inScheme <http://anzoil.org/def/soil/au/edu/fed-uni>;
  skos:notation "15G1-15D3-ECEC-H";
  skos:prefLabel "Hydrogen H+ as a percentage of Effective Cation Exchange Capacity procedure"@en;
  skos:topConceptOf <http://anzoil.org/def/soil/au/edu/fed-uni> .

procedure:15G1-AL a skos:Concept, sosa:Procedure;
  dct:description "A procedure for measuring Exchangeable Aluminuim (Al3+) 1 M potassium chloride"@en;
  dct:identifier "http://anzsoil.org/def/soil/au/edu/fed-uni/procedure/15G1-AL"^^xsd:anyURI;
  rdfs:label "Exchangeable Al3+ procedure - 1 M potassium chloride"@en;
  skos:definition "A procedure for measuring Exchangeable Aluminuim (Al3+) 1 M potassium chloride"@en;
  skos:inScheme <http://anzoil.org/def/soil/au/edu/fed-uni>;
  skos:notation "15G1-AL";
  skos:prefLabel "Exchangeable Al3+ procedure - 1 M potassium chloride"@en;
  skos:topConceptOf <http://anzoil.org/def/soil/au/edu/fed-uni> .

procedure:15G1-H a skos:Concept, sosa:Procedure;
  dct:description "A procedure for measuring Exchangeable Hydrogen (H+) 1 M potassium chloride"@en;
  dct:identifier "http://anzsoil.org/def/soil/au/edu/fed-uni/procedure/15G1-H"^^xsd:anyURI;
  rdfs:label "Exchangeable H+ procedure - 1 M potassium chloride"@en;
  skos:definition "A procedure for measuring Exchangeable Hydrogen (H+) 1 M potassium chloride"@en;
  skos:inScheme <http://anzoil.org/def/soil/au/edu/fed-uni>;
  skos:notation "15G1-H";
  skos:prefLabel "Exchangeable H+ procedure - 1 M potassium chloride"@en;
  skos:topConceptOf <http://anzoil.org/def/soil/au/edu/fed-uni> .

procedure:15M1-CMR a skos:Concept, sosa:Procedure;
  dct:description "A procedure for measuring Calcium to Magnesium Ratio"@en;
  dct:identifier "http://anzsoil.org/def/soil/au/edu/fed-uni/procedure/15M1-CMR"^^xsd:anyURI;
  rdfs:label "Calcium to Magnesium Ratio procedure"@en;
  skos:definition "A procedure for measuring Calcium to Magnesium Ratio"@en;
  skos:inScheme <http://anzoil.org/def/soil/au/edu/fed-uni>;
  skos:notation "15M1-CA/MG";
  skos:prefLabel "Calcium to Magnesium Ratio procedure"@en;
  skos:topConceptOf <http://anzoil.org/def/soil/au/edu/fed-uni> .

procedure:15M1-PMR a skos:Concept, sosa:Procedure;
  dct:description "A procedure for measuring Potassium to Magnesium Ratio"@en;
  dct:identifier "http://anzsoil.org/def/soil/au/edu/fed-uni/procedure/15M1-PMR"^^xsd:anyURI;
  rdfs:label "Potassium to Magnesium Ratio procedure"@en;
  skos:definition "A procedure for measuring Potassium to Magnesium Ratio"@en;
  skos:inScheme <http://anzoil.org/def/soil/au/edu/fed-uni>;
  skos:notation "15M1-K/MG";
  skos:prefLabel "Potassium to Magnesium Ratio procedure"@en;
  skos:topConceptOf <http://anzoil.org/def/soil/au/edu/fed-uni> .

procedure:3A1-TDS a skos:Concept, sosa:Procedure;
  dct:description "A procedure for measuring TDS - the Electrical Conductivity (EC) of 1:5 soil/water extract multiplied 640, where EC is obtained using method http://www.anzsoil.org/def/au/scma/3A1"@en;
  dct:identifier "http://anzsoil.org/def/soil/au/edu/fed-uni/procedure/3A1-TDS"^^xsd:anyURI;
  rdfs:label "Total dissolved salts procedure"@en;
  skos:definition "A procedure for measuring TDS - the Electrical Conductivity (EC) of 1:5 soil/water extract multiplied 640, where EC is obtained using method http://www.anzsoil.org/def/au/scma/3A1"@en;
  skos:inScheme <http://anzoil.org/def/soil/au/edu/fed-uni>;
  skos:notation "3A1-TDS";
  skos:prefLabel "Total dissolved salts procedure"@en;
  skos:topConceptOf <http://anzoil.org/def/soil/au/edu/fed-uni> .

procedure:6C1HUMa a skos:Concept, sosa:Procedure;
  dct:description "A procedure for measuring Organic Carbon as humus or decomposed materials MIR"@en;
  dct:identifier "http://anzsoil.org/def/soil/au/edu/fed-uni/procedure/6C1HUMa"^^xsd:anyURI;
  rdfs:label "Organic Carbon as humus or decomposed materials procedure - MIR"@en;
  skos:definition "A procedure for measuring Organic Carbon as humus or decomposed materials MIR"@en;
  skos:inScheme <http://anzoil.org/def/soil/au/edu/fed-uni>;
  skos:notation "6C1HUMa";
  skos:prefLabel "Organic Carbon as humus or decomposed materials procedure - MIR"@en;
  skos:topConceptOf <http://anzoil.org/def/soil/au/edu/fed-uni> .

procedure:6C1POCa a skos:Concept, sosa:Procedure;
  dct:description "A procedure for measuring Particulate Organic C (POC) MIR"@en;
  dct:identifier "http://anzsoil.org/def/soil/au/edu/fed-uni/procedure/6C1POCa"^^xsd:anyURI;
  rdfs:label "Particulate Organic C (POC) procedure - MIR"@en;
  skos:definition "A procedure for measuring Particulate Organic C (POC) MIR"@en;
  skos:inScheme <http://anzoil.org/def/soil/au/edu/fed-uni>;
  skos:notation "6C1POCa";
  skos:prefLabel "Particulate Organic C (POC) procedure - MIR"@en;
  skos:topConceptOf <http://anzoil.org/def/soil/au/edu/fed-uni> .

procedure:6C1RECa a skos:Concept, sosa:Procedure;
  dct:description "A procedure for measuring Recalcitrant Organic Carbon MIR"@en;
  dct:identifier "http://anzsoil.org/def/soil/au/edu/fed-uni/procedure/6C1RECa"^^xsd:anyURI;
  rdfs:label "Recalcitrant Organic Carbon procedure - MIR"@en;
  skos:definition "A procedure for measuring Recalcitrant Organic Carbon MIR"@en;
  skos:inScheme <http://anzoil.org/def/soil/au/edu/fed-uni>;
  skos:notation "6C1RECa";
  skos:prefLabel "Recalcitrant Organic Carbon procedure - MIR"@en;
  skos:topConceptOf <http://anzoil.org/def/soil/au/edu/fed-uni> .

procedure:7C2a-NH4 a skos:Concept, sosa:Procedure;
  dct:description "A procedure for measuring Mineral-N (Ammonium) 2 M KCl, automated colour, continuous segmented flow"@en;
  dct:identifier "http://anzsoil.org/def/soil/au/edu/fed-uni/procedure/7C2a-NH4"^^xsd:anyURI;
  rdfs:label "Mineral-N (Ammonium) procedure - 2 M KCl, automated colour, continuous segmented flow"@en;
  skos:definition "A procedure for measuring Mineral-N (Ammonium) 2 M KCl, automated colour, continuous segmented flow"@en;
  skos:inScheme <http://anzoil.org/def/soil/au/edu/fed-uni>;
  skos:notation "7C2a-NH4";
  skos:prefLabel "Mineral-N (Ammonium) procedure - 2 M KCl, automated colour, continuous segmented flow"@en;
  skos:topConceptOf <http://anzoil.org/def/soil/au/edu/fed-uni> .

procedure:7C2a-NO3 a skos:Concept, sosa:Procedure;
  dct:description "A procedure for measuring Mineral-N (Nitrate) 2 M KCl, automated colour, continuous segmented flow"@en;
  dct:identifier "http://anzsoil.org/def/soil/au/edu/fed-uni/procedure/7C2a-NO3"^^xsd:anyURI;
  rdfs:label "Mineral-N (Nitrate) procedure - 2 M KCl, automated colour, continuous segmented flow"@en;
  skos:definition "A procedure for measuring Mineral-N (Nitrate) 2 M KCl, automated colour, continuous segmented flow"@en;
  skos:inScheme <http://anzoil.org/def/soil/au/edu/fed-uni>;
  skos:notation "7C2a-NO3";
  skos:prefLabel "Mineral-N (Nitrate) procedure - 2 M KCl, automated colour, continuous segmented flow"@en;
  skos:topConceptOf <http://anzoil.org/def/soil/au/edu/fed-uni> .

procedure:7C2b-NH4 a skos:Concept, sosa:Procedure;
  dct:description "A procedure for measuring Mineral-N (Ammonium) - 2 M KCl, automated colour, FIA"@en;
  dct:identifier "http://anzsoil.org/def/soil/au/edu/fed-uni/procedure/7C2b-NH4"^^xsd:anyURI;
  rdfs:label "Mineral-N (Ammonium) procedure - 2 M KCl, automated colour, FIA"@en;
  skos:definition "A procedure for measuring Mineral-N (Ammonium) - 2 M KCl, automated colour, FIA"@en;
  skos:inScheme <http://anzoil.org/def/soil/au/edu/fed-uni>;
  skos:notation "7C2b-NH4";
  skos:prefLabel "Mineral-N (Ammonium) procedure - 2 M KCl, automated colour, FIA"@en;
  skos:topConceptOf <http://anzoil.org/def/soil/au/edu/fed-uni> .

procedure:7C2b-NO3 a skos:Concept, sosa:Procedure;
  dct:description "A procedure for measuring Mineral-N (Nitrate) 2 M KCl, automated colour, FIA"@en;
  dct:identifier "http://anzsoil.org/def/soil/au/edu/fed-uni/procedure/7C2b-NO3"^^xsd:anyURI;
  rdfs:label "Mineral-N (Nitrate) procedure - 2 M KCl, automated colour, FIA"@en;
  skos:definition "A procedure for measuring Mineral-N (Nitrate) 2 M KCl, automated colour, FIA"@en;
  skos:inScheme <http://anzoil.org/def/soil/au/edu/fed-uni>;
  skos:notation "7C2b-NO3";
  skos:prefLabel "Mineral-N (Nitrate) procedure - 2 M KCl, automated colour, FIA"@en;
  skos:topConceptOf <http://anzoil.org/def/soil/au/edu/fed-uni> .

procedure:9I2 a skos:Concept, sosa:Procedure;
  dct:description "A procedure for measuring Phosphorus Buffer Index using Colwell P"@en;
  dct:identifier "http://anzsoil.org/def/soil/au/edu/fed-uni/procedure/9I2"^^xsd:anyURI;
  rdfs:label "P Buffer Index - PBI (ColP) procedure"@en;
  skos:definition "A procedure for measuring Phosphorus Buffer Index using Colwell P"@en;
  skos:inScheme <http://anzoil.org/def/soil/au/edu/fed-uni>;
  skos:notation "9I2";
  skos:prefLabel "P Buffer Index - PBI (ColP) procedure"@en;
  skos:topConceptOf <http://anzoil.org/def/soil/au/edu/fed-uni> .

procedure:AA-S a skos:Concept, sosa:Procedure;
  dct:description "A procedure for measuring Available Sulfur - ammonium acetate"@en;
  dct:identifier "http://anzsoil.org/def/soil/au/edu/fed-uni/procedure/AA-S"^^xsd:anyURI;
  rdfs:label "Available Sulfur procedure - ammonium acetate"@en;
  skos:definition "A procedure for measuring Available Sulfur - ammonium acetate"@en;
  skos:inScheme <http://anzoil.org/def/soil/au/edu/fed-uni>;
  skos:notation "AA-S";
  skos:prefLabel "Available Sulfur procedure - ammonium acetate"@en;
  skos:topConceptOf <http://anzoil.org/def/soil/au/edu/fed-uni> .

procedure:ADJ-CEC a skos:Concept, sosa:Procedure;
  dct:description "A procedure for measuring Adjusted Cation Exchange Capacity where Adjusted CEC is calculated by subtracting Adjusted Hydrogen H+ from CEC"@en;
  dct:identifier "http://anzsoil.org/def/soil/au/edu/fed-uni/procedure/ADJ-CEC"^^xsd:anyURI;
  rdfs:label "Cation Exchange Capacity procedure - adjusted"@en;
  skos:definition "A procedure for measuring Adjusted Cation Exchange Capacity where Adjusted CEC is calculated by subtracting Adjusted Hydrogen H+ from CEC"@en;
  skos:inScheme <http://anzoil.org/def/soil/au/edu/fed-uni>;
  skos:notation "ADJ-CEC";
  skos:prefLabel "Cation Exchange Capacity procedure - adjusted"@en;
  skos:topConceptOf <http://anzoil.org/def/soil/au/edu/fed-uni> .

procedure:ADJ-EXCH-H a skos:Concept, sosa:Procedure;
  dct:description "A procedure for measuring Exchangeable Hydrogen H+ - adjusted"@en;
  dct:identifier "http://anzsoil.org/def/soil/au/edu/fed-uni/procedure/ADJ-EXCH-H"^^xsd:anyURI;
  rdfs:label "Exchangeable Hydrogen H+ procedure - adjusted"@en;
  skos:definition "A procedure for measuring Exchangeable Hydrogen H+ - adjusted"@en;
  skos:inScheme <http://anzoil.org/def/soil/au/edu/fed-uni>;
  skos:notation "ADJ-EXCH-H";
  skos:prefLabel "Exchangeable Hydrogen H+ procedure - adjusted"@en;
  skos:topConceptOf <http://anzoil.org/def/soil/au/edu/fed-uni> .

procedure:AD-TOT-P a skos:Concept, sosa:Procedure;
  dct:description "A procedure for measuring Total Phosphorus acid digestion"@en;
  dct:identifier "http://anzsoil.org/def/soil/au/edu/fed-uni/procedure/AD-TOT-P"^^xsd:anyURI;
  rdfs:label "Total Phosphorus procedure - acid digestion"@en;
  skos:definition "A procedure for measuring Total Phosphorus acid digestion"@en;
  skos:inScheme <http://anzoil.org/def/soil/au/edu/fed-uni>;
  skos:notation "AD-TOT-P";
  skos:prefLabel "Total Phosphorus procedure - acid digestion"@en;
  skos:topConceptOf <http://anzoil.org/def/soil/au/edu/fed-uni> .

procedure:AODE-AVL-MO a skos:Concept, sosa:Procedure;
  dct:description "A procedure for measuring Available Molybdenum ammonium oxalate/oxalic acid, diisopropyl ether"@en;
  dct:identifier "http://anzsoil.org/def/soil/au/edu/fed-uni/procedure/AODE-AVL-MO"^^xsd:anyURI;
  rdfs:label "Available Molybdenum procedure - ammonium oxalate/oxalic acid, diisopropyl ether"@en;
  skos:definition "A procedure for measuring Available Molybdenum ammonium oxalate/oxalic acid, diisopropyl ether"@en;
  skos:inScheme <http://anzoil.org/def/soil/au/edu/fed-uni>;
  skos:notation "AODE-AVL-MO";
  skos:prefLabel "Available Molybdenum procedure - ammonium oxalate/oxalic acid, diisopropyl ether"@en;
  skos:topConceptOf <http://anzoil.org/def/soil/au/edu/fed-uni> .

procedure:AVL-CA a skos:Concept, sosa:Procedure;
  dct:description "A procedure for measuring Available Calcium"@en;
  dct:identifier "http://anzsoil.org/def/soil/au/edu/fed-uni/procedure/AVL-CA"^^xsd:anyURI;
  rdfs:label "Available Calcium procedure"@en;
  skos:definition "A procedure for measuring Available Calcium"@en;
  skos:inScheme <http://anzoil.org/def/soil/au/edu/fed-uni>;
  skos:notation "AVL-CA";
  skos:prefLabel "Available Calcium procedure"@en;
  skos:topConceptOf <http://anzoil.org/def/soil/au/edu/fed-uni> .

procedure:AVL-K a skos:Concept, sosa:Procedure;
  dct:description "A procedure for measuring Available Potassium"@en;
  dct:identifier "http://anzsoil.org/def/soil/au/edu/fed-uni/procedure/AVL-K"^^xsd:anyURI;
  rdfs:label "Available Potassium procedure"@en;
  skos:definition "A procedure for measuring Available Potassium"@en;
  skos:inScheme <http://anzoil.org/def/soil/au/edu/fed-uni>;
  skos:notation "AVL-K";
  skos:prefLabel "Available Potassium procedure"@en;
  skos:topConceptOf <http://anzoil.org/def/soil/au/edu/fed-uni> .

procedure:AVL-MG a skos:Concept, sosa:Procedure;
  dct:description "A procedure for measuring Available Magnesium"@en;
  dct:identifier "http://anzsoil.org/def/soil/au/edu/fed-uni/procedure/AVL-MG"^^xsd:anyURI;
  rdfs:label "Available Magnesium procedure"@en;
  skos:definition "A procedure for measuring Available Magnesium"@en;
  skos:inScheme <http://anzoil.org/def/soil/au/edu/fed-uni>;
  skos:notation "AVL-MG";
  skos:prefLabel "Available Magnesium procedure"@en;
  skos:topConceptOf <http://anzoil.org/def/soil/au/edu/fed-uni> .

procedure:AVL-NA a skos:Concept, sosa:Procedure;
  dct:description "A procedure for measuring Available Sodium"@en;
  dct:identifier "http://anzsoil.org/def/soil/au/edu/fed-uni/procedure/AVL-NA"^^xsd:anyURI;
  rdfs:label "Available Sodium procedure"@en;
  skos:definition "A procedure for measuring Available Sodium"@en;
  skos:inScheme <http://anzoil.org/def/soil/au/edu/fed-uni>;
  skos:notation "AVL-NA";
  skos:prefLabel "Available Sodium procedure"@en;
  skos:topConceptOf <http://anzoil.org/def/soil/au/edu/fed-uni> .

procedure:AVL-ZN a skos:Concept, sosa:Procedure;
  dct:description "A procedure for measuring Available Zinc"@en;
  dct:identifier "http://anzsoil.org/def/soil/au/edu/fed-uni/procedure/AVL-ZN"^^xsd:anyURI;
  rdfs:label "Available Zinc procedure"@en;
  skos:definition "A procedure for measuring Available Zinc"@en;
  skos:inScheme <http://anzoil.org/def/soil/au/edu/fed-uni>;
  skos:notation "AVL-ZN";
  skos:prefLabel "Available Zinc procedure"@en;
  skos:topConceptOf <http://anzoil.org/def/soil/au/edu/fed-uni> .

procedure:AW-TOT-C a skos:Concept, sosa:Procedure;
  dct:description "A procedure for measuring Total Carbon acid wash"@en;
  dct:identifier "http://anzsoil.org/def/soil/au/edu/fed-uni/procedure/AW-TOT-C"^^xsd:anyURI;
  rdfs:label "Total C acid wash procedure"@en;
  skos:definition "A procedure for measuring Total Carbon acid wash"@en;
  skos:inScheme <http://anzoil.org/def/soil/au/edu/fed-uni>;
  skos:notation "AW-TOT-C";
  skos:prefLabel "Total C acid wash procedure"@en;
  skos:topConceptOf <http://anzoil.org/def/soil/au/edu/fed-uni> .

procedure:B a skos:Concept, sosa:Procedure;
  dct:description "A procedure for measuring Boron"@en;
  dct:identifier "http://anzsoil.org/def/soil/au/edu/fed-uni/procedure/B"^^xsd:anyURI;
  rdfs:label "Boron procedure"@en;
  skos:definition "A procedure for measuring Boron"@en;
  skos:inScheme <http://anzoil.org/def/soil/au/edu/fed-uni>;
  skos:notation "B";
  skos:prefLabel "Boron procedure"@en;
  skos:topConceptOf <http://anzoil.org/def/soil/au/edu/fed-uni> .

procedure:BACL-EXCH-H a skos:Concept, sosa:Procedure;
  dct:description "A procedure for measuring Hydrogen H+ by Barium Chloride-Triethanolamine method. Reference: Peech, M., Cowan, R.L. & Baker, J.H. (1962). Soil Science Society American Procedures, A critical study of the Barium chloride-Triethanolamine and ammonium acetate methods for determining exchangeable Hydrogen of soils."@en;
  dct:identifier "http://anzsoil.org/def/soil/au/edu/fed-uni/procedure/BACL-EXCH-H"^^xsd:anyURI;
  rdfs:label "Exchangeable Hydrogen H+ procedure - Barium Chloride-Triethanolamine"@en;
  skos:definition "A procedure for measuring Hydrogen H+ by Barium Chloride-Triethanolamine method. Reference: Peech, M., Cowan, R.L. & Baker, J.H. (1962). Soil Science Society American Procedures, A critical study of the Barium chloride-Triethanolamine and ammonium acetate methods for determining exchangeable Hydrogen of soils."@en;
  skos:inScheme <http://anzoil.org/def/soil/au/edu/fed-uni>;
  skos:notation "BACL-EXCH-H";
  skos:prefLabel "Exchangeable Hydrogen H+ procedure - Barium Chloride-Triethanolamine"@en;
  skos:topConceptOf <http://anzoil.org/def/soil/au/edu/fed-uni> .

procedure:BCI a skos:Concept, sosa:Procedure;
  dct:description "A procedure for measuring pH Buffering Capacity Index"@en;
  dct:identifier "http://anzsoil.org/def/soil/au/edu/fed-uni/procedure/BCI"^^xsd:anyURI;
  rdfs:label "pH buffering capacity index procedure"@en;
  skos:definition "A procedure for measuring pH Buffering Capacity Index"@en;
  skos:inScheme <http://anzoil.org/def/soil/au/edu/fed-uni>;
  skos:notation "BCI";
  skos:prefLabel "pH buffering capacity index procedure"@en;
  skos:topConceptOf <http://anzoil.org/def/soil/au/edu/fed-uni> .

procedure:BROMF-AL a skos:Concept, sosa:Procedure;
  dct:description "A procedure for measuring Aluminium following Bromfield, S.M. (1987). Reference: Simple tests for the assessment of aluminium and manganese levels in acid soils. Australian Journal Agriculture 27, 399-404."@en;
  dct:identifier "http://anzsoil.org/def/soil/au/edu/fed-uni/procedure/BROMF-AL"^^xsd:anyURI;
  rdfs:label "Aluminium procedure - Bromfield method (1987)"@en;
  skos:definition "A procedure for measuring Aluminium following Bromfield, S.M. (1987). Reference: Simple tests for the assessment of aluminium and manganese levels in acid soils. Australian Journal Agriculture 27, 399-404."@en;
  skos:inScheme <http://anzoil.org/def/soil/au/edu/fed-uni>;
  skos:notation "BROMF-AL";
  skos:prefLabel "Aluminium procedure - Bromfield method (1987)"@en;
  skos:topConceptOf <http://anzoil.org/def/soil/au/edu/fed-uni> .

procedure:BRU-N a skos:Concept, sosa:Procedure;
  dct:description "A procedure for measuring Available Nitrogen calcium chloride, brucine"@en;
  dct:identifier "http://anzsoil.org/def/soil/au/edu/fed-uni/procedure/BRU-N"^^xsd:anyURI;
  rdfs:label "Available Nitrogen procedure - calcium chloride, brucine"@en;
  skos:definition "A procedure for measuring Available Nitrogen calcium chloride, brucine"@en;
  skos:inScheme <http://anzoil.org/def/soil/au/edu/fed-uni>;
  skos:notation "BRU-N";
  skos:prefLabel "Available Nitrogen procedure - calcium chloride, brucine"@en;
  skos:topConceptOf <http://anzoil.org/def/soil/au/edu/fed-uni> .

procedure:CA a skos:Concept, sosa:Procedure;
  dct:description "A procedure for measuring Calcium"@en;
  dct:identifier "http://anzsoil.org/def/soil/au/edu/fed-uni/procedure/CA"^^xsd:anyURI;
  rdfs:label "Calcium procedure"@en;
  skos:definition "A procedure for measuring Calcium"@en;
  skos:inScheme <http://anzoil.org/def/soil/au/edu/fed-uni>;
  skos:notation "CA";
  skos:prefLabel "Calcium procedure"@en;
  skos:topConceptOf <http://anzoil.org/def/soil/au/edu/fed-uni> .

procedure:CACL2-AL a skos:Concept, sosa:Procedure;
  dct:description "A procedure for measuring Alumnium as calcium chloride extractable"@en;
  dct:identifier "http://anzsoil.org/def/soil/au/edu/fed-uni/procedure/CACL2-AL"^^xsd:anyURI;
  rdfs:label "Alumnium - calcium chloride extractable procedure"@en;
  skos:definition "A procedure for measuring Alumnium as calcium chloride extractable"@en;
  skos:inScheme <http://anzoil.org/def/soil/au/edu/fed-uni>;
  skos:notation "CACL2-AL";
  skos:prefLabel "Alumnium - calcium chloride extractable procedure"@en;
  skos:topConceptOf <http://anzoil.org/def/soil/au/edu/fed-uni> .

procedure:CACL2a-SI a skos:Concept, sosa:Procedure;
  dct:description "A procedure for measuring Silicon extraction CaCl2 method (Ref:Haysom, M. B. C. and L. S. Chapman. 1975. Some aspects of the calcium silicate trials at Mackay. Proc. Qld. Soc. Sugar Cane Technol. 42:117-122). Detetion FIA"@en;
  dct:identifier "http://anzsoil.org/def/soil/au/edu/fed-uni/procedure/CACL2a-SI"^^xsd:anyURI;
  rdfs:label "Silicon procedure - CaCl2 extraction, FIA"@en;
  skos:definition "A procedure for measuring Silicon extraction CaCl2 method (Ref:Haysom, M. B. C. and L. S. Chapman. 1975. Some aspects of the calcium silicate trials at Mackay. Proc. Qld. Soc. Sugar Cane Technol. 42:117-122). Detetion FIA"@en;
  skos:inScheme <http://anzoil.org/def/soil/au/edu/fed-uni>;
  skos:notation "CACl2a-SI";
  skos:prefLabel "Silicon procedure - CaCl2 extraction, FIA"@en;
  skos:topConceptOf <http://anzoil.org/def/soil/au/edu/fed-uni> .

procedure:CACL2-PH a skos:Concept, sosa:Procedure;
  dct:description "A procedure for measuring pH of a calcium chloride extract"@en;
  dct:identifier "http://anzsoil.org/def/soil/au/edu/fed-uni/procedure/CACL2-PH"^^xsd:anyURI;
  rdfs:label "pH of a calcium chloride extract procedure"@en;
  skos:definition "A procedure for measuring pH of a calcium chloride extract"@en;
  skos:inScheme <http://anzoil.org/def/soil/au/edu/fed-uni>;
  skos:notation "CACL2-PH";
  skos:prefLabel "pH of a calcium chloride extract procedure"@en;
  skos:topConceptOf <http://anzoil.org/def/soil/au/edu/fed-uni> .

procedure:CEC a skos:Concept, sosa:Procedure;
  dct:description "A procedure for measuring Cation Exchange Capacity"@en;
  dct:identifier "http://anzsoil.org/def/soil/au/edu/fed-uni/procedure/CEC"^^xsd:anyURI;
  rdfs:label "Cation Exchange Capacity procedure"@en;
  skos:definition "A procedure for measuring Cation Exchange Capacity"@en;
  skos:inScheme <http://anzoil.org/def/soil/au/edu/fed-uni>;
  skos:notation "CEC";
  skos:prefLabel "Cation Exchange Capacity procedure"@en;
  skos:topConceptOf <http://anzoil.org/def/soil/au/edu/fed-uni> .

procedure:CEC-AL a skos:Concept, sosa:Procedure;
  dct:description "A procedure for measuring Aluminium as % of Exchangeable Cations"@en;
  dct:identifier "http://anzsoil.org/def/soil/au/edu/fed-uni/procedure/CEC-AL"^^xsd:anyURI;
  rdfs:label "Aluminium - as % of Exchangeable cations procedure"@en;
  skos:definition "A procedure for measuring Aluminium as % of Exchangeable Cations"@en;
  skos:inScheme <http://anzoil.org/def/soil/au/edu/fed-uni>;
  skos:notation "CEC-AL";
  skos:prefLabel "Aluminium - as % of Exchangeable cations procedure"@en;
  skos:topConceptOf <http://anzoil.org/def/soil/au/edu/fed-uni> .

procedure:CEC-NA a skos:Concept, sosa:Procedure;
  dct:description "A procedure for measuring Sodium as % of Exchangeable Cations"@en;
  dct:identifier "http://anzsoil.org/def/soil/au/edu/fed-uni/procedure/CEC-NA"^^xsd:anyURI;
  rdfs:label "Sodium - as % of Exchangeable Cations procedure"@en;
  skos:definition "A procedure for measuring Sodium as % of Exchangeable Cations"@en;
  skos:inScheme <http://anzoil.org/def/soil/au/edu/fed-uni>;
  skos:notation "CEC-NA";
  skos:prefLabel "Sodium - as % of Exchangeable Cations procedure"@en;
  skos:topConceptOf <http://anzoil.org/def/soil/au/edu/fed-uni> .

procedure:CL a skos:Concept, sosa:Procedure;
  dct:description "A procedure for measuring Chloride"@en;
  dct:identifier "http://anzsoil.org/def/soil/au/edu/fed-uni/procedure/CL"^^xsd:anyURI;
  rdfs:label "Chloride procedure"@en;
  skos:definition "A procedure for measuring Chloride"@en;
  skos:inScheme <http://anzoil.org/def/soil/au/edu/fed-uni>;
  skos:notation "CL";
  skos:prefLabel "Chloride procedure"@en;
  skos:topConceptOf <http://anzoil.org/def/soil/au/edu/fed-uni> .

procedure:CMR a skos:Concept, sosa:Procedure;
  dct:description "A procedure for measuring Calcium to Magnesium Ratio"@en;
  dct:identifier "http://anzsoil.org/def/soil/au/edu/fed-uni/procedure/CMR"^^xsd:anyURI;
  rdfs:label "Calcium to Magnesium Ratio procedure"@en;
  skos:definition "A procedure for measuring Calcium to Magnesium Ratio"@en;
  skos:inScheme <http://anzoil.org/def/soil/au/edu/fed-uni>;
  skos:notation "CA/MG";
  skos:prefLabel "Calcium to Magnesium Ratio procedure"@en;
  skos:topConceptOf <http://anzoil.org/def/soil/au/edu/fed-uni> .

procedure:CU a skos:Concept, sosa:Procedure;
  dct:description "A procedure for measuring Copper"@en;
  dct:identifier "http://anzsoil.org/def/soil/au/edu/fed-uni/procedure/CU"^^xsd:anyURI;
  rdfs:label "Copper procedure"@en;
  skos:definition "A procedure for measuring Copper"@en;
  skos:inScheme <http://anzoil.org/def/soil/au/edu/fed-uni>;
  skos:notation "CU";
  skos:prefLabel "Copper procedure"@en;
  skos:topConceptOf <http://anzoil.org/def/soil/au/edu/fed-uni> .

procedure:DGT-P a skos:Concept, sosa:Procedure;
  dct:description "A procedure for measuring a soil's ability to maintain soil solution phosphorus by Diffusive Gradient in Thin-Films procedure (DGT)."@en;
  dct:identifier "http://anzsoil.org/def/soil/au/edu/fed-uni/procedure/DGT-P"^^xsd:anyURI;
  rdfs:label "Phosphorus by diffusive gradient in thin-films procedure (DGT-P)"@en;
  skos:definition "A procedure for measuring a soil's ability to maintain soil solution phosphorus by Diffusive Gradient in Thin-Films procedure (DGT)."@en;
  skos:inScheme <http://anzoil.org/def/soil/au/edu/fed-uni>;
  skos:notation "DGT-P";
  skos:prefLabel "Phosphorus by diffusive gradient in thin-films procedure (DGT-P)"@en;
  skos:topConceptOf <http://anzoil.org/def/soil/au/edu/fed-uni> .

procedure:EC a skos:Concept, sosa:Procedure;
  dct:description "A procedure for measuring Electrical Conductivity (EC)"@en;
  dct:identifier "http://anzsoil.org/def/soil/au/edu/fed-uni/procedure/EC"^^xsd:anyURI;
  rdfs:label "Electrical Conductivity (EC) procedure"@en;
  skos:definition "A procedure for measuring Electrical Conductivity (EC)"@en;
  skos:inScheme <http://anzoil.org/def/soil/au/edu/fed-uni>;
  skos:notation "EC";
  skos:prefLabel "Electrical Conductivity (EC) procedure"@en;
  skos:topConceptOf <http://anzoil.org/def/soil/au/edu/fed-uni> .

procedure:ECEC a skos:Concept, sosa:Procedure;
  dct:description "A procedure for measuring Effective Cation Exchange Capacity"@en;
  dct:identifier "http://anzsoil.org/def/soil/au/edu/fed-uni/procedure/ECEC"^^xsd:anyURI;
  rdfs:label "Effective Cation Exchange Capacity procedure"@en;
  skos:definition "A procedure for measuring Effective Cation Exchange Capacity"@en;
  skos:inScheme <http://anzoil.org/def/soil/au/edu/fed-uni>;
  skos:notation "ECEC";
  skos:prefLabel "Effective Cation Exchange Capacity procedure"@en;
  skos:topConceptOf <http://anzoil.org/def/soil/au/edu/fed-uni> .

procedure:ECEC-NA a skos:Concept, sosa:Procedure;
  dct:description "A procedure for measuring Sodium as % of Effective Cation Exchange Capacity"@en;
  dct:identifier "http://anzsoil.org/def/soil/au/edu/fed-uni/procedure/ECEC-NA"^^xsd:anyURI;
  rdfs:label "Sodium procedure - as % of effective cation exchange capacity"@en;
  skos:definition "A procedure for measuring Sodium as % of Effective Cation Exchange Capacity"@en;
  skos:inScheme <http://anzoil.org/def/soil/au/edu/fed-uni>;
  skos:notation "ECEC-NA";
  skos:prefLabel "Sodium procedure - as % of effective cation exchange capacity"@en;
  skos:topConceptOf <http://anzoil.org/def/soil/au/edu/fed-uni> .

procedure:ECSE-SP a skos:Concept, sosa:Procedure;
  dct:description "A procedure for measuring Procedure for measuring Electrical Conductivity of a saturation extract following Slavich and GH Peterson (1993)"@en;
  dct:identifier "http://anzsoil.org/def/soil/au/edu/fed-uni/procedure/ECSE-SP"^^xsd:anyURI;
  rdfs:label "Electrical Conductivity of a saturation extract (ECse) procedure - Slavich and Peterson method"@en;
  skos:definition "A procedure for measuring Procedure for measuring Electrical Conductivity of a saturation extract following Slavich and GH Peterson (1993)"@en;
  skos:inScheme <http://anzoil.org/def/soil/au/edu/fed-uni>;
  skos:notation "ECSE-SP";
  skos:prefLabel "Electrical Conductivity of a saturation extract (ECse) procedure - Slavich and Peterson method"@en;
  skos:topConceptOf <http://anzoil.org/def/soil/au/edu/fed-uni> .

procedure:EXCH-AL a skos:Concept, sosa:Procedure;
  dct:description "A procedure for measuring Exchangeable Aluminium"@en;
  dct:identifier "http://anzsoil.org/def/soil/au/edu/fed-uni/procedure/EXCH-AL"^^xsd:anyURI;
  rdfs:label "Exchangeable Aluminium procedure"@en;
  skos:definition "A procedure for measuring Exchangeable Aluminium"@en;
  skos:inScheme <http://anzoil.org/def/soil/au/edu/fed-uni>;
  skos:notation "EXCH-AL";
  skos:prefLabel "Exchangeable Aluminium procedure"@en;
  skos:topConceptOf <http://anzoil.org/def/soil/au/edu/fed-uni> .

procedure:EXCH-CA a skos:Concept, sosa:Procedure;
  dct:description "A procedure for measuring Exchangeable Calcium"@en;
  dct:identifier "http://anzsoil.org/def/soil/au/edu/fed-uni/procedure/EXCH-CA"^^xsd:anyURI;
  rdfs:label "Exchangeable Calcium procedure"@en;
  skos:definition "A procedure for measuring Exchangeable Calcium"@en;
  skos:inScheme <http://anzoil.org/def/soil/au/edu/fed-uni>;
  skos:notation "EXCH-CA";
  skos:prefLabel "Exchangeable Calcium procedure"@en;
  skos:topConceptOf <http://anzoil.org/def/soil/au/edu/fed-uni> .

procedure:EXCH-H a skos:Concept, sosa:Procedure;
  dct:description "A procedure for measuring Hydrogen H+"@en;
  dct:identifier "http://anzsoil.org/def/soil/au/edu/fed-uni/procedure/EXCH-H"^^xsd:anyURI;
  rdfs:label "Exchangeable Hydrogen H+ procedure"@en;
  skos:definition "A procedure for measuring Hydrogen H+"@en;
  skos:inScheme <http://anzoil.org/def/soil/au/edu/fed-uni>;
  skos:notation "EXCH-H";
  skos:prefLabel "Exchangeable Hydrogen H+ procedure"@en;
  skos:topConceptOf <http://anzoil.org/def/soil/au/edu/fed-uni> .

procedure:EXCH-K a skos:Concept, sosa:Procedure;
  dct:description "A procedure for measuring Exchangeable Potassium"@en;
  dct:identifier "http://anzsoil.org/def/soil/au/edu/fed-uni/procedure/EXCH-K"^^xsd:anyURI;
  rdfs:label "Exchangeable Potassium procedure"@en;
  skos:definition "A procedure for measuring Exchangeable Potassium"@en;
  skos:inScheme <http://anzoil.org/def/soil/au/edu/fed-uni>;
  skos:notation "EXCH-K";
  skos:prefLabel "Exchangeable Potassium procedure"@en;
  skos:topConceptOf <http://anzoil.org/def/soil/au/edu/fed-uni> .

procedure:EXCH-MG a skos:Concept, sosa:Procedure;
  dct:description "A procedure for measuring Exchangeable Magnesium"@en;
  dct:identifier "http://anzsoil.org/def/soil/au/edu/fed-uni/procedure/EXCH-MG"^^xsd:anyURI;
  rdfs:label "Exchangeable Magnesium procedure"@en;
  skos:definition "A procedure for measuring Exchangeable Magnesium"@en;
  skos:inScheme <http://anzoil.org/def/soil/au/edu/fed-uni>;
  skos:notation "EXCH-MG";
  skos:prefLabel "Exchangeable Magnesium procedure"@en;
  skos:topConceptOf <http://anzoil.org/def/soil/au/edu/fed-uni> .

procedure:EXCH-NA a skos:Concept, sosa:Procedure;
  dct:description "A procedure for measuring Exchangeable Sodium"@en;
  dct:identifier "http://anzsoil.org/def/soil/au/edu/fed-uni/procedure/EXCH-NA"^^xsd:anyURI;
  rdfs:label "Exchangeable Sodium procedure"@en;
  skos:definition "A procedure for measuring Exchangeable Sodium"@en;
  skos:inScheme <http://anzoil.org/def/soil/au/edu/fed-uni>;
  skos:notation "EXCH-NA";
  skos:prefLabel "Exchangeable Sodium procedure"@en;
  skos:topConceptOf <http://anzoil.org/def/soil/au/edu/fed-uni> .

procedure:FE a skos:Concept, sosa:Procedure;
  dct:description "A procedure for measuring Iron"@en;
  dct:identifier "http://anzsoil.org/def/soil/au/edu/fed-uni/procedure/FE"^^xsd:anyURI;
  rdfs:label "Iron procedure"@en;
  skos:definition "A procedure for measuring Iron"@en;
  skos:inScheme <http://anzoil.org/def/soil/au/edu/fed-uni>;
  skos:notation "FE";
  skos:prefLabel "Iron procedure"@en;
  skos:topConceptOf <http://anzoil.org/def/soil/au/edu/fed-uni> .

procedure:GTRI a skos:Concept, sosa:Procedure;
  dct:description "A procedure for measuring Grass Tetany Risk Index (GTRI) specific for pasture, where GTRI=K/(Ca + Mg)"@en;
  dct:identifier "http://anzsoil.org/def/soil/au/edu/fed-uni/procedure/GTRI"^^xsd:anyURI;
  rdfs:label "Grass tetany risk index procedure"@en;
  skos:definition "A procedure for measuring Grass Tetany Risk Index (GTRI) specific for pasture, where GTRI=K/(Ca + Mg)"@en;
  skos:inScheme <http://anzoil.org/def/soil/au/edu/fed-uni>;
  skos:notation "GTRI";
  skos:prefLabel "Grass tetany risk index procedure"@en;
  skos:topConceptOf <http://anzoil.org/def/soil/au/edu/fed-uni> .

procedure:H2O-PH a skos:Concept, sosa:Procedure;
  dct:description "A procedure for measuring pH of a soil/water suspension"@en;
  dct:identifier "http://anzsoil.org/def/soil/au/edu/fed-uni/procedure/H2O-PH"^^xsd:anyURI;
  rdfs:label "pH of a soil/water suspension procedure"@en;
  skos:definition "A procedure for measuring pH of a soil/water suspension"@en;
  skos:inScheme <http://anzoil.org/def/soil/au/edu/fed-uni>;
  skos:notation "H2O-PH";
  skos:prefLabel "pH of a soil/water suspension procedure"@en;
  skos:topConceptOf <http://anzoil.org/def/soil/au/edu/fed-uni> .

procedure:HWS-B a skos:Concept, sosa:Procedure;
  dct:description "A procedure for measuring Boron as hot water soluble"@en;
  dct:identifier "http://anzsoil.org/def/soil/au/edu/fed-uni/procedure/HWS-B"^^xsd:anyURI;
  rdfs:label "Boron - hot water soluble procedure"@en;
  skos:definition "A procedure for measuring Boron as hot water soluble"@en;
  skos:inScheme <http://anzoil.org/def/soil/au/edu/fed-uni>;
  skos:notation "HWS-B";
  skos:prefLabel "Boron - hot water soluble procedure"@en;
  skos:topConceptOf <http://anzoil.org/def/soil/au/edu/fed-uni> .

procedure:HWS-ICP-B a skos:Concept, sosa:Procedure;
  dct:description "A procedure for measuring Boron as hot water soluble - ICP"@en;
  dct:identifier "http://anzsoil.org/def/soil/au/edu/fed-uni/procedure/HWS-ICP-B"^^xsd:anyURI;
  rdfs:label "Boron - hot water soluble procedure, ICP"@en;
  skos:definition "A procedure for measuring Boron as hot water soluble - ICP"@en;
  skos:inScheme <http://anzoil.org/def/soil/au/edu/fed-uni>;
  skos:notation "HWS-ICP-B";
  skos:prefLabel "Boron - hot water soluble procedure, ICP"@en;
  skos:topConceptOf <http://anzoil.org/def/soil/au/edu/fed-uni> .

procedure:ICP-TOT-CA a skos:Concept, sosa:Procedure;
  dct:description "A procedure for measuring Total Calcium - ICP"@en;
  dct:identifier "http://anzsoil.org/def/soil/au/edu/fed-uni/procedure/ICP-TOT-CA"^^xsd:anyURI;
  rdfs:label "Total Calcium procedure - ICP"@en;
  skos:definition "A procedure for measuring Total Calcium - ICP"@en;
  skos:inScheme <http://anzoil.org/def/soil/au/edu/fed-uni>;
  skos:notation "ICP-TOT-CA";
  skos:prefLabel "Total Calcium procedure - ICP"@en;
  skos:topConceptOf <http://anzoil.org/def/soil/au/edu/fed-uni> .

procedure:ICP-TOT-CO a skos:Concept, sosa:Procedure;
  dct:description "A procedure for measuring Total Cobalt - ICP"@en;
  dct:identifier "http://anzsoil.org/def/soil/au/edu/fed-uni/procedure/ICP-TOT-CO"^^xsd:anyURI;
  rdfs:label "Total Cobalt procedure - ICP"@en;
  skos:definition "A procedure for measuring Total Cobalt - ICP"@en;
  skos:inScheme <http://anzoil.org/def/soil/au/edu/fed-uni>;
  skos:notation "ICP-TOT-CO";
  skos:prefLabel "Total Cobalt procedure - ICP"@en;
  skos:topConceptOf <http://anzoil.org/def/soil/au/edu/fed-uni> .

procedure:ICP-TOT-CU a skos:Concept, sosa:Procedure;
  dct:description "A procedure for measuring Total Copper - ICP"@en;
  dct:identifier "http://anzsoil.org/def/soil/au/edu/fed-uni/procedure/ICP-TOT-CU"^^xsd:anyURI;
  rdfs:label "Total Copper procedure - ICP"@en;
  skos:definition "A procedure for measuring Total Copper - ICP"@en;
  skos:inScheme <http://anzoil.org/def/soil/au/edu/fed-uni>;
  skos:notation "ICP-TOT-CU";
  skos:prefLabel "Total Copper procedure - ICP"@en;
  skos:topConceptOf <http://anzoil.org/def/soil/au/edu/fed-uni> .

procedure:ICP-TOT-FE a skos:Concept, sosa:Procedure;
  dct:description "A procedure for measuring Total Iron - ICP"@en;
  dct:identifier "http://anzsoil.org/def/soil/au/edu/fed-uni/procedure/ICP-TOT-FE"^^xsd:anyURI;
  rdfs:label "Total Iron procedure - ICP"@en;
  skos:definition "A procedure for measuring Total Iron - ICP"@en;
  skos:inScheme <http://anzoil.org/def/soil/au/edu/fed-uni>;
  skos:notation "ICP-TOT-FE";
  skos:prefLabel "Total Iron procedure - ICP"@en;
  skos:topConceptOf <http://anzoil.org/def/soil/au/edu/fed-uni> .

procedure:ICP-TOT-K a skos:Concept, sosa:Procedure;
  dct:description "A procedure for measuring Total Potassium - ICP"@en;
  dct:identifier "http://anzsoil.org/def/soil/au/edu/fed-uni/procedure/ICP-TOT-K"^^xsd:anyURI;
  rdfs:label "Total Potassium procedure - ICP"@en;
  skos:definition "A procedure for measuring Total Potassium - ICP"@en;
  skos:inScheme <http://anzoil.org/def/soil/au/edu/fed-uni>;
  skos:notation "ICP-TOT-K";
  skos:prefLabel "Total Potassium procedure - ICP"@en;
  skos:topConceptOf <http://anzoil.org/def/soil/au/edu/fed-uni> .

procedure:ICP-TOT-MG a skos:Concept, sosa:Procedure;
  dct:description "A procedure for measuring Total Magnesium - ICP"@en;
  dct:identifier "http://anzsoil.org/def/soil/au/edu/fed-uni/procedure/ICP-TOT-MG"^^xsd:anyURI;
  rdfs:label "Total Magnesium procedure - ICP"@en;
  skos:definition "A procedure for measuring Total Magnesium - ICP"@en;
  skos:inScheme <http://anzoil.org/def/soil/au/edu/fed-uni>;
  skos:notation "ICP-TOT-MG";
  skos:prefLabel "Total Magnesium procedure - ICP"@en;
  skos:topConceptOf <http://anzoil.org/def/soil/au/edu/fed-uni> .

procedure:ICP-TOT-MN a skos:Concept, sosa:Procedure;
  dct:description "A procedure for measuring Total Manganese - ICP"@en;
  dct:identifier "http://anzsoil.org/def/soil/au/edu/fed-uni/procedure/ICP-TOT-MN"^^xsd:anyURI;
  rdfs:label "Total Manganese procedure - ICP"@en;
  skos:definition "A procedure for measuring Total Manganese - ICP"@en;
  skos:inScheme <http://anzoil.org/def/soil/au/edu/fed-uni>;
  skos:notation "ICP-TOT-MN";
  skos:prefLabel "Total Manganese procedure - ICP"@en;
  skos:topConceptOf <http://anzoil.org/def/soil/au/edu/fed-uni> .

procedure:ICP-TOT-NA a skos:Concept, sosa:Procedure;
  dct:description "A procedure for measuring Total Sodium - ICP"@en;
  dct:identifier "http://anzsoil.org/def/soil/au/edu/fed-uni/procedure/ICP-TOT-NA"^^xsd:anyURI;
  rdfs:label "Total Sodium procedure - ICP"@en;
  skos:definition "A procedure for measuring Total Sodium - ICP"@en;
  skos:inScheme <http://anzoil.org/def/soil/au/edu/fed-uni>;
  skos:notation "ICP-TOT-NA";
  skos:prefLabel "Total Sodium procedure - ICP"@en;
  skos:topConceptOf <http://anzoil.org/def/soil/au/edu/fed-uni> .

procedure:ICP-TOT-P a skos:Concept, sosa:Procedure;
  dct:description "A procedure for measuring Total Phosphorus - ICP"@en;
  dct:identifier "http://anzsoil.org/def/soil/au/edu/fed-uni/procedure/ICP-TOT-P"^^xsd:anyURI;
  rdfs:label "Total Phosphorus procedure - ICP"@en;
  skos:definition "A procedure for measuring Total Phosphorus - ICP"@en;
  skos:inScheme <http://anzoil.org/def/soil/au/edu/fed-uni>;
  skos:notation "ICP-TOT-P";
  skos:prefLabel "Total Phosphorus procedure - ICP"@en;
  skos:topConceptOf <http://anzoil.org/def/soil/au/edu/fed-uni> .

procedure:ICP-TOT-ZN a skos:Concept, sosa:Procedure;
  dct:description "A procedure for measuring Total Zinc - ICP"@en;
  dct:identifier "http://anzsoil.org/def/soil/au/edu/fed-uni/procedure/ICP-TOT-ZN"^^xsd:anyURI;
  rdfs:label "Total Zinc procedure - ICP"@en;
  skos:definition "A procedure for measuring Total Zinc - ICP"@en;
  skos:inScheme <http://anzoil.org/def/soil/au/edu/fed-uni>;
  skos:notation "ICP-TOT-ZN";
  skos:prefLabel "Total Zinc procedure - ICP"@en;
  skos:topConceptOf <http://anzoil.org/def/soil/au/edu/fed-uni> .

procedure:K a skos:Concept, sosa:Procedure;
  dct:description "A procedure for measuring Potassium"@en;
  dct:identifier "http://anzsoil.org/def/soil/au/edu/fed-uni/procedure/K"^^xsd:anyURI;
  rdfs:label "Potassium procedure"@en;
  skos:definition "A procedure for measuring Potassium"@en;
  skos:inScheme <http://anzoil.org/def/soil/au/edu/fed-uni>;
  skos:notation "K";
  skos:prefLabel "Potassium procedure"@en;
  skos:topConceptOf <http://anzoil.org/def/soil/au/edu/fed-uni> .

procedure:MG a skos:Concept, sosa:Procedure;
  dct:description "A procedure for measuring Magnesium"@en;
  dct:identifier "http://anzsoil.org/def/soil/au/edu/fed-uni/procedure/MG"^^xsd:anyURI;
  rdfs:label "Magnesium procedure"@en;
  skos:definition "A procedure for measuring Magnesium"@en;
  skos:inScheme <http://anzoil.org/def/soil/au/edu/fed-uni>;
  skos:notation "MG";
  skos:prefLabel "Magnesium procedure"@en;
  skos:topConceptOf <http://anzoil.org/def/soil/au/edu/fed-uni> .

procedure:MIK-AVL-FE a skos:Concept, sosa:Procedure;
  dct:description "A procedure for measuring Available Iron Mikhail method"@en;
  dct:identifier "http://anzsoil.org/def/soil/au/edu/fed-uni/procedure/MIK-AVL-FE"^^xsd:anyURI;
  rdfs:label "Available Iron procedure - Mikhail method"@en;
  skos:definition "A procedure for measuring Available Iron Mikhail method"@en;
  skos:inScheme <http://anzoil.org/def/soil/au/edu/fed-uni>;
  skos:notation "MIK-AVL-FE";
  skos:prefLabel "Available Iron procedure - Mikhail method"@en;
  skos:topConceptOf <http://anzoil.org/def/soil/au/edu/fed-uni> .

procedure:MIK-AVL-MN a skos:Concept, sosa:Procedure;
  dct:description "A procedure for measuring Available Manganese Mikhail method"@en;
  dct:identifier "http://anzsoil.org/def/soil/au/edu/fed-uni/procedure/MIK-AVL-MN"^^xsd:anyURI;
  rdfs:label "Available Manganese procedure - Mikhail method"@en;
  skos:definition "A procedure for measuring Available Manganese Mikhail method"@en;
  skos:inScheme <http://anzoil.org/def/soil/au/edu/fed-uni>;
  skos:notation "MIK-AVL-MN";
  skos:prefLabel "Available Manganese procedure - Mikhail method"@en;
  skos:topConceptOf <http://anzoil.org/def/soil/au/edu/fed-uni> .

procedure:MIR a skos:Concept, sosa:Procedure;
  dct:description "The procedure of Mid Infrared Spectroscopy (MIR)"@en;
  dct:identifier "http://anzsoil.org/def/soil/au/edu/fed-uni/procedure/MIR"^^xsd:anyURI;
  rdfs:label "MIR procedure"@en;
  skos:definition "The procedure of Mid Infrared Spectroscopy (MIR)"@en;
  skos:inScheme <http://anzoil.org/def/soil/au/edu/fed-uni>;
  skos:notation "MIR";
  skos:prefLabel "MIR procedure"@en;
  skos:topConceptOf <http://anzoil.org/def/soil/au/edu/fed-uni> .

procedure:NA a skos:Concept, sosa:Procedure;
  dct:description "A procedure for measuring Sodium"@en;
  dct:identifier "http://anzsoil.org/def/soil/au/edu/fed-uni/procedure/NA"^^xsd:anyURI;
  rdfs:label "Sodium procedure"@en;
  skos:definition "A procedure for measuring Sodium"@en;
  skos:inScheme <http://anzoil.org/def/soil/au/edu/fed-uni>;
  skos:notation "NA";
  skos:prefLabel "Sodium procedure"@en;
  skos:topConceptOf <http://anzoil.org/def/soil/au/edu/fed-uni> .

procedure:NACL2 a skos:Concept, sosa:Procedure;
  dct:description "A procedure for measuring Choride salts as NaCl2"@en;
  dct:identifier "http://anzsoil.org/def/soil/au/edu/fed-uni/procedure/NACL2"^^xsd:anyURI;
  rdfs:label "Choride salts as NaCl2 procedure"@en;
  skos:definition "A procedure for measuring Choride salts as NaCl2"@en;
  skos:inScheme <http://anzoil.org/def/soil/au/edu/fed-uni>;
  skos:notation "NACL2";
  skos:prefLabel "Choride salts as NaCl2 procedure"@en;
  skos:topConceptOf <http://anzoil.org/def/soil/au/edu/fed-uni> .

procedure:NH4 a skos:Concept, sosa:Procedure;
  dct:description "A procedure for measuring Ammonium"@en;
  dct:identifier "http://anzsoil.org/def/soil/au/edu/fed-uni/procedure/NH4"^^xsd:anyURI;
  rdfs:label "Ammonium procedure"@en;
  skos:definition "A procedure for measuring Ammonium"@en;
  skos:inScheme <http://anzoil.org/def/soil/au/edu/fed-uni>;
  skos:notation "NH4";
  skos:prefLabel "Ammonium procedure"@en;
  skos:topConceptOf <http://anzoil.org/def/soil/au/edu/fed-uni> .

procedure:NH4-NO3 a skos:Concept, sosa:Procedure;
  dct:description "A procedure for measuring Mineral-N (Ammonium and Nitrate)"@en;
  dct:identifier "http://anzsoil.org/def/soil/au/edu/fed-uni/procedure/NH4-NO3"^^xsd:anyURI;
  rdfs:label "Mineral-N (Nitrate + Ammonium) procedure"@en;
  skos:definition "A procedure for measuring Mineral-N (Ammonium and Nitrate)"@en;
  skos:inScheme <http://anzoil.org/def/soil/au/edu/fed-uni>;
  skos:notation "NH4-NO3";
  skos:prefLabel "Mineral-N (Nitrate + Ammonium) procedure"@en;
  skos:topConceptOf <http://anzoil.org/def/soil/au/edu/fed-uni> .

procedure:NO3 a skos:Concept, sosa:Procedure;
  dct:description "A procedure for measuring Nitrate"@en;
  dct:identifier "http://anzsoil.org/def/soil/au/edu/fed-uni/procedure/NO3"^^xsd:anyURI;
  rdfs:label "Nitrate procedure"@en;
  skos:definition "A procedure for measuring Nitrate"@en;
  skos:inScheme <http://anzoil.org/def/soil/au/edu/fed-uni>;
  skos:notation "NO3";
  skos:prefLabel "Nitrate procedure"@en;
  skos:topConceptOf <http://anzoil.org/def/soil/au/edu/fed-uni> .

procedure:P a skos:Concept, sosa:Procedure;
  dct:description "A procedure for measuring Phosphorus"@en;
  dct:identifier "http://anzsoil.org/def/soil/au/edu/fed-uni/procedure/P"^^xsd:anyURI;
  rdfs:label "Phosphorus procedure"@en;
  skos:definition "A procedure for measuring Phosphorus"@en;
  skos:inScheme <http://anzoil.org/def/soil/au/edu/fed-uni>;
  skos:notation "P";
  skos:prefLabel "Phosphorus procedure"@en;
  skos:topConceptOf <http://anzoil.org/def/soil/au/edu/fed-uni> .

procedure:P6-LP a skos:Concept, sosa:Procedure;
  dct:description "A procedure for measuring Loveday & Pyle dispersion index"@en;
  dct:identifier "http://anzsoil.org/def/soil/au/edu/fed-uni/procedure/P6-LP"^^xsd:anyURI;
  rdfs:label "Loveday & Pyle dispersion index procedure"@en;
  skos:definition "A procedure for measuring Loveday & Pyle dispersion index"@en;
  skos:inScheme <http://anzoil.org/def/soil/au/edu/fed-uni>;
  skos:notation "P6-LP";
  skos:prefLabel "Loveday & Pyle dispersion index procedure"@en;
  skos:topConceptOf <http://anzoil.org/def/soil/au/edu/fed-uni> .

procedure:PBI a skos:Concept, sosa:Procedure;
  dct:description "A procedure for measuring Phosphorus Buffering Index"@en;
  dct:identifier "http://anzsoil.org/def/soil/au/edu/fed-uni/procedure/PBI"^^xsd:anyURI;
  rdfs:label "Phosphorus Buffering Index procedure"@en;
  skos:definition "A procedure for measuring Phosphorus Buffering Index"@en;
  skos:inScheme <http://anzoil.org/def/soil/au/edu/fed-uni>;
  skos:notation "PBI";
  skos:prefLabel "Phosphorus Buffering Index procedure"@en;
  skos:topConceptOf <http://anzoil.org/def/soil/au/edu/fed-uni> .

procedure:PERI a skos:Concept, sosa:Procedure;
  dct:description "A procedure for measuring Phosphorus Environmental Risk Index. It is calculated from the available P and the Phosphorus Buffer Index (PBI)."@en;
  dct:identifier "http://anzsoil.org/def/soil/au/edu/fed-uni/procedure/PERI"^^xsd:anyURI;
  rdfs:label "Phosphorus Environmental Risk Index procedure"@en;
  skos:definition "A procedure for measuring Phosphorus Environmental Risk Index. It is calculated from the available P and the Phosphorus Buffer Index (PBI)."@en;
  skos:inScheme <http://anzoil.org/def/soil/au/edu/fed-uni>;
  skos:notation "PERI";
  skos:prefLabel "Phosphorus Environmental Risk Index procedure"@en;
  skos:topConceptOf <http://anzoil.org/def/soil/au/edu/fed-uni> .

procedure:PRI-AJ a skos:Concept, sosa:Procedure;
  dct:description "A procedure for measuring Phosphorus Retention Index following method of llen, D.G. and Jeffrey, R.C. (1990). Methods for analysis of phosphorus. Western Australian Soil Report of Investigation No.37 Chemistry Centre WA, p. 37"@en;
  dct:identifier "http://anzsoil.org/def/soil/au/edu/fed-uni/procedure/PRI-AJ"^^xsd:anyURI;
  rdfs:label "Phosphorus Retention Index (PRI) procedure - Allen & Jeffrey 1990"@en;
  skos:definition "A procedure for measuring Phosphorus Retention Index following method of llen, D.G. and Jeffrey, R.C. (1990). Methods for analysis of phosphorus. Western Australian Soil Report of Investigation No.37 Chemistry Centre WA, p. 37"@en;
  skos:inScheme <http://anzoil.org/def/soil/au/edu/fed-uni>;
  skos:notation "PRI-AJ";
  skos:prefLabel "Phosphorus Retention Index (PRI) procedure - Allen & Jeffrey 1990"@en;
  skos:topConceptOf <http://anzoil.org/def/soil/au/edu/fed-uni> .

procedure:PSR a skos:Concept, sosa:Procedure;
  dct:description "A procedure for measuring Potassium to Sodium Ratio"@en;
  dct:identifier "http://anzsoil.org/def/soil/au/edu/fed-uni/procedure/PSR"^^xsd:anyURI;
  rdfs:label "Potassium to Sodium Ratio procedure"@en;
  skos:definition "A procedure for measuring Potassium to Sodium Ratio"@en;
  skos:inScheme <http://anzoil.org/def/soil/au/edu/fed-uni>;
  skos:notation "K/NA";
  skos:prefLabel "Potassium to Sodium Ratio procedure"@en;
  skos:topConceptOf <http://anzoil.org/def/soil/au/edu/fed-uni> .

procedure:RCH-N a skos:Concept, sosa:Procedure;
  dct:description "A procedure for measuring Nitrogen - Richlands"@en;
  dct:identifier "http://anzsoil.org/def/soil/au/edu/fed-uni/procedure/RCH-N"^^xsd:anyURI;
  rdfs:label "Richlands Nitrogen procedure"@en;
  skos:definition "A procedure for measuring Nitrogen - Richlands"@en;
  skos:inScheme <http://anzoil.org/def/soil/au/edu/fed-uni>;
  skos:notation "RCH-N";
  skos:prefLabel "Richlands Nitrogen procedure"@en;
  skos:topConceptOf <http://anzoil.org/def/soil/au/edu/fed-uni> .

procedure:R-FE a skos:Concept, sosa:Procedure;
  dct:description "A procedure for measuring Reactive Iron"@en;
  dct:identifier "http://anzsoil.org/def/soil/au/edu/fed-uni/procedure/R-FE"^^xsd:anyURI;
  rdfs:label "Reactive Iron procedure"@en;
  skos:definition "A procedure for measuring Reactive Iron"@en;
  skos:inScheme <http://anzoil.org/def/soil/au/edu/fed-uni>;
  skos:notation "R-FE";
  skos:prefLabel "Reactive Iron procedure"@en;
  skos:topConceptOf <http://anzoil.org/def/soil/au/edu/fed-uni> .

procedure:S a skos:Concept, sosa:Procedure;
  dct:description "A procedure for measuring Sulfur"@en;
  dct:identifier "http://anzsoil.org/def/soil/au/edu/fed-uni/procedure/S"^^xsd:anyURI;
  rdfs:label "Sulfur procedure"@en;
  skos:definition "A procedure for measuring Sulfur"@en;
  skos:inScheme <http://anzoil.org/def/soil/au/edu/fed-uni>;
  skos:notation "S";
  skos:prefLabel "Sulfur procedure"@en;
  skos:topConceptOf <http://anzoil.org/def/soil/au/edu/fed-uni> .

procedure:SOC a skos:Concept, sosa:Procedure;
  dct:description "A procedure for measuring Soil Organic Carbon"@en;
  dct:identifier "http://anzsoil.org/def/soil/au/edu/fed-uni/procedure/SOC"^^xsd:anyURI;
  rdfs:label "Soil Organic Carbon procedure"@en;
  skos:definition "A procedure for measuring Soil Organic Carbon"@en;
  skos:inScheme <http://anzoil.org/def/soil/au/edu/fed-uni>;
  skos:notation "SOC";
  skos:prefLabel "Soil Organic Carbon procedure"@en;
  skos:topConceptOf <http://anzoil.org/def/soil/au/edu/fed-uni> .

procedure:TOT-C a skos:Concept, sosa:Procedure;
  dct:description "A procedure for measuring Total Carbon"@en;
  dct:identifier "http://anzsoil.org/def/soil/au/edu/fed-uni/procedure/TOT-C"^^xsd:anyURI;
  rdfs:label "Total C procedure"@en;
  skos:definition "A procedure for measuring Total Carbon"@en;
  skos:inScheme <http://anzoil.org/def/soil/au/edu/fed-uni>;
  skos:notation "TOT-C";
  skos:prefLabel "Total C procedure"@en;
  skos:topConceptOf <http://anzoil.org/def/soil/au/edu/fed-uni> .

procedure:TOT-N a skos:Concept, sosa:Procedure;
  dct:description "A procedure for measuring Total Nitrogen"@en;
  dct:identifier "http://anzsoil.org/def/soil/au/edu/fed-uni/procedure/TOT-N"^^xsd:anyURI;
  rdfs:label "Total Nitrogen procedure"@en;
  skos:definition "A procedure for measuring Total Nitrogen"@en;
  skos:inScheme <http://anzoil.org/def/soil/au/edu/fed-uni>;
  skos:notation "TOT-N";
  skos:prefLabel "Total Nitrogen procedure"@en;
  skos:topConceptOf <http://anzoil.org/def/soil/au/edu/fed-uni> .

procedure:WB-N a skos:Concept, sosa:Procedure;
  dct:description "A procedure for measuring Organic Nitrogen Walkley Black method"@en;
  dct:identifier "http://anzsoil.org/def/soil/au/edu/fed-uni/procedure/WB-N"^^xsd:anyURI;
  rdfs:label "Organic N procedure - Walkley Black method"@en;
  skos:definition "A procedure for measuring Organic Nitrogen Walkley Black method"@en;
  skos:inScheme <http://anzoil.org/def/soil/au/edu/fed-uni>;
  skos:notation "WB-N";
  skos:prefLabel "Organic N procedure - Walkley Black method"@en;
  skos:topConceptOf <http://anzoil.org/def/soil/au/edu/fed-uni> .

procedure:ZN a skos:Concept, sosa:Procedure;
  dct:description "A procedure for measuring Zinc"@en;
  dct:identifier "http://anzsoil.org/def/soil/au/edu/fed-uni/procedure/ZN"^^xsd:anyURI;
  rdfs:label "Zinc procedure"@en;
  skos:definition "A procedure for measuring Zinc"@en;
  skos:inScheme <http://anzoil.org/def/soil/au/edu/fed-uni>;
  skos:notation "ZN";
  skos:prefLabel "Zinc procedure"@en;
  skos:topConceptOf <http://anzoil.org/def/soil/au/edu/fed-uni> .

procedure:field-soil-texture a skos:Concept, sosa:Procedure;
  dct:description "A procedure for measuring Field texture is a measure of the behaviour of a small handful of soil when moistened and kneaded into a ball and then pressed out between thumb and forefinger. Field texture grades are characterised the behaviour of the moist bolus."@en;
  dct:identifier "http://anzsoil.org/def/soil/au/edu/fed-uni/procedure/field-soil-texture"^^xsd:anyURI;
  rdfs:label "Field soil texture procedure"@en;
  skos:definition "A procedure for measuring Field texture is a measure of the behaviour of a small handful of soil when moistened and kneaded into a ball and then pressed out between thumb and forefinger. Field texture grades are characterised the behaviour of the moist bolus."@en;
  skos:inScheme <http://anzoil.org/def/soil/au/edu/fed-uni>;
  skos:prefLabel "Field soil texture procedure"@en;
  skos:topConceptOf <http://anzoil.org/def/soil/au/edu/fed-uni> .

procedure:bulk-density-soil a skos:Concept, sosa:Procedure;
  dct:description "A procedure for measuring Bulk Density"@en;
  dct:identifier "http://anzsoil.org/def/soil/au/edu/fed-uni/procedure/bulk-density-soil"^^xsd:anyURI;
  rdfs:label "Bulk Density procedure"@en;
  skos:definition "A procedure for measuring Bulk Density"@en;
  skos:inScheme <http://anzoil.org/def/soil/au/edu/fed-uni>;
  skos:prefLabel "Bulk Density procedure"@en;
  skos:topConceptOf <http://anzoil.org/def/soil/au/edu/fed-uni> .

procedure:gravel-1 a skos:Concept, sosa:Procedure;
  dct:description "A procedure for measuring gravel content of soil by estimating visually and by running the fingers through the soil"@en;
  dct:identifier "http://anzsoil.org/def/soil/au/edu/fed-uni/procedure/gravel-1"^^xsd:anyURI;
  rdfs:label "Gravel estimation procedure - visually and running fingers through soil"@en;
  skos:definition "A procedure for measuring gravel content of soil by estimating visually and by running the fingers through the soil"@en;
  skos:inScheme <http://anzoil.org/def/soil/au/edu/fed-uni>;
  skos:prefLabel "Gravel estimation procedure - visually and running fingers through soil"@en;
  skos:topConceptOf <http://anzoil.org/def/soil/au/edu/fed-uni> .

procedure:gravel-2 a skos:Concept, sosa:Procedure;
  dct:description "A procedure for measuring the gravel content of soil by weight"@en;
  dct:identifier "http://anzsoil.org/def/soil/au/edu/fed-uni/procedure/gravel-2"^^xsd:anyURI;
  rdfs:label "Gravel procedure - by weight"@en;
  skos:definition "A procedure for measuring the gravel content of soil by weight"@en;
  skos:inScheme <http://anzoil.org/def/soil/au/edu/fed-uni>;
  skos:prefLabel "Gravel procedure - by weight"@en;
  skos:topConceptOf <http://anzoil.org/def/soil/au/edu/fed-uni> .

procedure:15D1-BACL-H a skos:Concept, sosa:Procedure;
  dct:description "This procedure is a calculation of exchangeable hydrogen H+ from ‘Adjusted Cation Exchange Capacity’ (CEC) where Adjusted CEC is calculated by subtracting ‘Adjusted Hydrogen’ from CEC. The underlying methods are: 1. for exchangeable bases (Ca2+, Mg2+ , Na+ and K+) - 15D1 of Rayment and Lyons 2011l- 1 M ammonium acetate at pH 7.0, pre-treatment for soluble salts, manual leach and 2. ‘Adjusted Hydrogen’ - A procedure for measuring H+ by Barium Chloride-Triethanolamine method. Reference: Peech, M., Cowan, R.L. & Baker, J.H. (1962). Soil Science Society American Procedures, A critical study of the Barium chloride-Triethanolamine and ammonium acetate methods for determining exchangeable Hydrogen of soils."@en;
  dct:identifier "http://anzsoil.org/def/soil/au/edu/fed-uni/procedure/15D1-BACL-H"^^xsd:anyURI;
  rdfs:label "Exchangable hydrogen H+ procedure - 15D1 and Barium Chloride-Triethanolamine"@en;
  skos:definition "This procedure is a calculation of exchangeable hydrogen H+ from ‘Adjusted Cation Exchange Capacity’ (CEC) where Adjusted CEC is calculated by subtracting ‘Adjusted Hydrogen’ from CEC. The underlying methods are: 1. for exchangeable bases (Ca2+, Mg2+ , Na+ and K+) - 15D1 of Rayment and Lyons 2011l- 1 M ammonium acetate at pH 7.0, pre-treatment for soluble salts, manual leach and 2. ‘Adjusted Hydrogen’ - A procedure for measuring H+ by Barium Chloride-Triethanolamine method. Reference: Peech, M., Cowan, R.L. & Baker, J.H. (1962). Soil Science Society American Procedures, A critical study of the Barium chloride-Triethanolamine and ammonium acetate methods for determining exchangeable Hydrogen of soils."@en;
  skos:inScheme <http://anzoil.org/def/soil/au/edu/fed-uni>;
  skos:notation "15D1-BACL-H";
  skos:prefLabel "Exchangable hydrogen H+ procedure - 15D1 and Barium Chloride-Triethanolamine"@en;
  skos:topConceptOf <http://anzoil.org/def/soil/au/edu/fed-uni> .

procedure:15D1-BACL-K a skos:Concept, sosa:Procedure;
  dct:description "This procedure is a calculation of exchangeable potassium from ‘Adjusted Cation Exchange Capacity’ (CEC) where Adjusted CEC is calculated by subtracting ‘Adjusted Hydrogen’ from CEC. The underlying methods are: 1. for exchangeable bases (Ca2+, Mg2+ , Na+ and K+) - 15D1 of Rayment and Lyons 2011l- 1 M ammonium acetate at pH 7.0, pre-treatment for soluble salts, manual leach and 2. ‘Adjusted Hydrogen’ - A procedure for measuring H+ by Barium Chloride-Triethanolamine method. Reference: Peech, M., Cowan, R.L. & Baker, J.H. (1962). Soil Science Society American Procedures, A critical study of the Barium chloride-Triethanolamine and ammonium acetate methods for determining exchangeable Hydrogen of soils."@en;
  dct:identifier "http://anzsoil.org/def/soil/au/edu/fed-uni/procedure/15D1-BACL-K"^^xsd:anyURI;
  rdfs:label "Exchangable potassium procedure - 15D1 and Barium Chloride-Triethanolamine"@en;
  skos:definition "This procedure is a calculation of exchangeable potassium from ‘Adjusted Cation Exchange Capacity’ (CEC) where Adjusted CEC is calculated by subtracting ‘Adjusted Hydrogen’ from CEC. The underlying methods are: 1. for exchangeable bases (Ca2+, Mg2+ , Na+ and K+) - 15D1 of Rayment and Lyons 2011l- 1 M ammonium acetate at pH 7.0, pre-treatment for soluble salts, manual leach and 2. ‘Adjusted Hydrogen’ - A procedure for measuring H+ by Barium Chloride-Triethanolamine method. Reference: Peech, M., Cowan, R.L. & Baker, J.H. (1962). Soil Science Society American Procedures, A critical study of the Barium chloride-Triethanolamine and ammonium acetate methods for determining exchangeable Hydrogen of soils."@en;
  skos:inScheme <http://anzoil.org/def/soil/au/edu/fed-uni>;
  skos:notation "15D1-BACL-K";
  skos:prefLabel "Exchangable potassium procedure - 15D1 and Barium Chloride-Triethanolamine"@en;
  skos:topConceptOf <http://anzoil.org/def/soil/au/edu/fed-uni> .

procedure:15D1-BACL-MG a skos:Concept, sosa:Procedure;
  dct:description "This procedure is a calculation of exchangeable magnesium from ‘Adjusted Cation Exchange Capacity’ (CEC) where Adjusted CEC is calculated by subtracting ‘Adjusted Hydrogen’ from CEC. The underlying methods are: 1. for exchangeable bases (Ca2+, Mg2+ , Na+ and K+) - 15D1 of Rayment and Lyons 2011l- 1 M ammonium acetate at pH 7.0, pre-treatment for soluble salts, manual leach and 2. ‘Adjusted Hydrogen’ - A procedure for measuring H+ by Barium Chloride-Triethanolamine method. Reference: Peech, M., Cowan, R.L. & Baker, J.H. (1962). Soil Science Society American Procedures, A critical study of the Barium chloride-Triethanolamine and ammonium acetate methods for determining exchangeable Hydrogen of soils."@en;
  dct:identifier "http://anzsoil.org/def/soil/au/edu/fed-uni/procedure/15D1-BACL-MG"^^xsd:anyURI;
  rdfs:label "Exchangable magnesium procedure - 15D1 and Barium Chloride-Triethanolamine"@en;
  skos:definition "This procedure is a calculation of exchangeable magnesium from ‘Adjusted Cation Exchange Capacity’ (CEC) where Adjusted CEC is calculated by subtracting ‘Adjusted Hydrogen’ from CEC. The underlying methods are: 1. for exchangeable bases (Ca2+, Mg2+ , Na+ and K+) - 15D1 of Rayment and Lyons 2011l- 1 M ammonium acetate at pH 7.0, pre-treatment for soluble salts, manual leach and 2. ‘Adjusted Hydrogen’ - A procedure for measuring H+ by Barium Chloride-Triethanolamine method. Reference: Peech, M., Cowan, R.L. & Baker, J.H. (1962). Soil Science Society American Procedures, A critical study of the Barium chloride-Triethanolamine and ammonium acetate methods for determining exchangeable Hydrogen of soils."@en;
  skos:inScheme <http://anzoil.org/def/soil/au/edu/fed-uni>;
  skos:notation "15D1-BACL-MG";
  skos:prefLabel "Exchangable magnesium procedure - 15D1 and Barium Chloride-Triethanolamine"@en;
  skos:topConceptOf <http://anzoil.org/def/soil/au/edu/fed-uni> .

procedure:15D1-BACL-NA a skos:Concept, sosa:Procedure;
  dct:description "This procedure is a calculation of exchangeable sodium from ‘Adjusted Cation Exchange Capacity’ (CEC) where Adjusted CEC is calculated by subtracting ‘Adjusted Hydrogen’ from CEC. The underlying methods are: 1. for exchangeable bases (Ca2+, Mg2+ , Na+ and K+) - 15D1 of Rayment and Lyons 2011l- 1 M ammonium acetate at pH 7.0, pre-treatment for soluble salts, manual leach and 2. ‘Adjusted Hydrogen’ - A procedure for measuring H+ by Barium Chloride-Triethanolamine method. Reference: Peech, M., Cowan, R.L. & Baker, J.H. (1962). Soil Science Society American Procedures, A critical study of the Barium chloride-Triethanolamine and ammonium acetate methods for determining exchangeable Hydrogen of soils."@en;
  dct:identifier "http://anzsoil.org/def/soil/au/edu/fed-uni/procedure/15D1-BACL-NA"^^xsd:anyURI;
  rdfs:label "Exchangable sodium procedure - 15D1 and Barium Chloride-Triethanolamine"@en;
  skos:definition "This procedure is a calculation of exchangeable sodium from ‘Adjusted Cation Exchange Capacity’ (CEC) where Adjusted CEC is calculated by subtracting ‘Adjusted Hydrogen’ from CEC. The underlying methods are: 1. for exchangeable bases (Ca2+, Mg2+ , Na+ and K+) - 15D1 of Rayment and Lyons 2011l- 1 M ammonium acetate at pH 7.0, pre-treatment for soluble salts, manual leach and 2. ‘Adjusted Hydrogen’ - A procedure for measuring H+ by Barium Chloride-Triethanolamine method. Reference: Peech, M., Cowan, R.L. & Baker, J.H. (1962). Soil Science Society American Procedures, A critical study of the Barium chloride-Triethanolamine and ammonium acetate methods for determining exchangeable Hydrogen of soils."@en;
  skos:inScheme <http://anzoil.org/def/soil/au/edu/fed-uni>;
  skos:notation "15D1-BACL-NA";
  skos:prefLabel "Exchangable sodium procedure - 15D1 and Barium Chloride-Triethanolamine"@en;
  skos:topConceptOf <http://anzoil.org/def/soil/au/edu/fed-uni> .

procedure:15D1-CA a skos:Concept, sosa:Procedure;
  dct:description "A procedure for measuring exchangeable calcium by 1 M ammonium acetate at pH 7.0, pre-treatment for soluble salts, manual leach"@en;
  dct:identifier "http://anzsoil.org/def/soil/au/edu/fed-uni/procedure/15D1-CA"^^xsd:anyURI;
  rdfs:label "Exchangeable calcium procedure - 1 M ammonium acetate at pH 7.0, pre-treatment for soluble salts, manual leach"@en;
  skos:definition "A procedure for measuring exchangeable calcium by 1 M ammonium acetate at pH 7.0, pre-treatment for soluble salts, manual leach"@en;
  skos:inScheme <http://anzoil.org/def/soil/au/edu/fed-uni>;
  skos:notation "15D1-CA";
  skos:prefLabel "Exchangeable calcium procedure - 1 M ammonium acetate at pH 7.0, pre-treatment for soluble salts, manual leach"@en;
  skos:topConceptOf <http://anzoil.org/def/soil/au/edu/fed-uni> .

procedure:15D1-K a skos:Concept, sosa:Procedure;
  dct:description "A procedure for measuring exchangeable potassium by 1 M ammonium acetate at pH 7.0, pre-treatment for soluble salts, manual leach"@en;
  dct:identifier "http://anzsoil.org/def/soil/au/edu/fed-uni/procedure/15D1-K"^^xsd:anyURI;
  rdfs:label "Exchangeable potassium procedure - 1 M ammonium acetate at pH 7.0, pre-treatment for soluble salts, manual leach"@en;
  skos:definition "A procedure for measuring exchangeable potassium by 1 M ammonium acetate at pH 7.0, pre-treatment for soluble salts, manual leach"@en;
  skos:inScheme <http://anzoil.org/def/soil/au/edu/fed-uni>;
  skos:notation "15D1-K";
  skos:prefLabel "Exchangeable potassium procedure - 1 M ammonium acetate at pH 7.0, pre-treatment for soluble salts, manual leach"@en;
  skos:topConceptOf <http://anzoil.org/def/soil/au/edu/fed-uni> .

procedure:15D1-MG a skos:Concept, sosa:Procedure;
  dct:description "A procedure for measuring exchangable magnesium by 1 M ammonium acetate at pH 7.0, pre-treatment for soluble salts, manual leach"@en;
  dct:identifier "http://anzsoil.org/def/soil/au/edu/fed-uni/procedure/15D1-MG"^^xsd:anyURI;
  rdfs:label "Exchangeable magnesium procedure - 1 M ammonium acetate at pH 7.0, pre-treatment for soluble salts, manual leach"@en;
  skos:definition "A procedure for measuring exchangable magnesium by 1 M ammonium acetate at pH 7.0, pre-treatment for soluble salts, manual leach"@en;
  skos:inScheme <http://anzoil.org/def/soil/au/edu/fed-uni>;
  skos:notation "15D1-MG";
  skos:prefLabel "Exchangeable magnesium procedure - 1 M ammonium acetate at pH 7.0, pre-treatment for soluble salts, manual leach"@en;
  skos:topConceptOf <http://anzoil.org/def/soil/au/edu/fed-uni> .

procedure:15D1-NA a skos:Concept, sosa:Procedure;
  dct:description "A procedure for measuring exchangeable sodium by 1 M ammonium acetate at pH 7.0, pre-treatment for soluble salts, manual leach"@en;
  dct:identifier "http://anzsoil.org/def/soil/au/edu/fed-uni/procedure/15D1-NA"^^xsd:anyURI;
  rdfs:label "Exchangeable sodium procedure - 1 M ammonium acetate at pH 7.0, pre-treatment for soluble salts, manual leach"@en;
  skos:definition "A procedure for measuring exchangeable sodium by 1 M ammonium acetate at pH 7.0, pre-treatment for soluble salts, manual leach"@en;
  skos:inScheme <http://anzoil.org/def/soil/au/edu/fed-uni>;
  skos:notation "15D1-NA";
  skos:prefLabel "Exchangeable sodium procedure - 1 M ammonium acetate at pH 7.0, pre-treatment for soluble salts, manual leach"@en;
  skos:topConceptOf <http://anzoil.org/def/soil/au/edu/fed-uni> .

procedure:PAW a skos:Concept, sosa:Procedure;
  dct:description "A procedure for measuring plant available water"@en;
  dct:identifier "http://anzsoil.org/def/soil/au/edu/fed-uni/procedure/PAW"^^xsd:anyURI;
  rdfs:label "Plant available water procedure"@en;
  skos:definition "A procedure for measuring plant available water"@en;
  skos:inScheme <http://anzoil.org/def/soil/au/edu/fed-uni>;
  skos:notation "PAW";
  skos:prefLabel "Plant available water procedure"@en;
  skos:topConceptOf <http://anzoil.org/def/soil/au/edu/fed-uni> .

procedure:WB-MOD-2-TOC a skos:Concept, sosa:Procedure;
  dct:description "A procedure for measuring Total Organic Carbon by multiplying the concentration of Organic Matter as determined by a Modified Walkley and Black Method, by 0.5"@en;
  dct:identifier "http://anzsoil.org/def/soil/au/edu/fed-uni/procedure/WB-MOD-2-TOC"^^xsd:anyURI;
  rdfs:label "Total Organic Carbon by modified Walkley & Black 2 procedure"@en;
  skos:definition "A procedure for measuring Total Organic Carbon by multiplying the concentration of Organic Matter as determined by a Modified Walkley and Black Method, by 0.5"@en;
  skos:inScheme <http://anzoil.org/def/soil/au/edu/fed-uni>;
  skos:notation "WB-MOD-2-TOC";
  skos:prefLabel "Total Organic Carbon by modified Walkley & Black 2 procedure"@en;
  skos:topConceptOf <http://anzoil.org/def/soil/au/edu/fed-uni> .

procedure:WB-MOD-TOC a skos:Concept, sosa:Procedure;
  dct:description "A procedure for measuring Total Organic Carbon by multiplying the concentration of Organic Matter as determined by a Modified Walkley and Black Method, by 0.58 (the inverse function of the 1.724 factor)"@en;
  dct:identifier "http://anzsoil.org/def/soil/au/edu/fed-uni/procedure/WB-MOD-TOC"^^xsd:anyURI;
  rdfs:label "Total Organic Carbon by modified Walkley & Black 1 procedure"@en;
  skos:definition "A procedure for measuring Total Organic Carbon by multiplying the concentration of Organic Matter as determined by a Modified Walkley and Black Method, by 0.58 (the inverse function of the 1.724 factor)"@en;
  skos:inScheme <http://anzoil.org/def/soil/au/edu/fed-uni>;
  skos:notation "WB-MOD-TOC";
  skos:prefLabel "Total Organic Carbon by modified Walkley & Black 1 procedure"@en;
  skos:topConceptOf <http://anzoil.org/def/soil/au/edu/fed-uni> .

procedure:WE-OC-ON a skos:Concept, sosa:ObservableProperty, sosa:Procedure;
  dct:description "A procedure for measuring water-extractable organic C:N. Haney, R.L. et al. 2012. Soil Organic C:N vs. water-extractable organic C:N. Open Journal of Soil Science, 2012, 2, 269-274."@en,
    "Water-extractable organic carbon to nitrogen ratio"@en;
  dct:identifier "http://anzsoil.org/def/soil/au/edu/fed-uni/procedure/WE-OC-ON"^^xsd:anyURI,
    "http://anzsoil.org/def/soil/au/edu/fed-uni/property/WE-OC-ON"^^xsd:anyURI;
  rdfs:label "Water extractable organic C:N procedure"@en, "Water-extractable organic carbon to nitrogen ratio"@en;
  skos:definition "A procedure for measuring water-extractable organic C:N. Haney, R.L. et al. 2012. Soil Organic C:N vs. water-extractable organic C:N. Open Journal of Soil Science, 2012, 2, 269-274."@en,
    "Water-extractable organic carbon to nitrogen ratio"@en;
  skos:inScheme <http://anzoil.org/def/soil/au/edu/fed-uni>;
  skos:notation "WE-OC-ON";
  skos:prefLabel "Water extractable organic C:N procedure"@en, "Water-extractable organic carbon to nitrogen ratio"@en;
  skos:topConceptOf <http://anzoil.org/def/soil/au/edu/fed-uni> .

procedure:CO2-MA a skos:Concept, sosa:Procedure;
  dct:description "A procedure for calculating an indicator of microbial activity (0 - 100) from CO2 emitted by microbes, 3 days under laboratory conditions"@en;
  dct:identifier "http://anzsoil.org/def/soil/au/edu/fed-uni/procedure/CO2-MA"^^xsd:anyURI;
  rdfs:label "Microbial activity by CO2 respiration - 3 days laboratory"@en;
  skos:definition "A procedure for calculating an indicator of microbial activity (0 - 100) from CO2 emitted by microbes, 3 days under laboratory conditions"@en;
  skos:inScheme <http://anzoil.org/def/soil/au/edu/fed-uni>;
  skos:notation "CO2-MA";
  skos:prefLabel "Microbial activity by CO2 respiration - 3 days laboratory"@en;
  skos:topConceptOf <http://anzoil.org/def/soil/au/edu/fed-uni> .

procedure:CO2-MBR a skos:Concept, sosa:Procedure;
  dct:description "A procedure for calculating soil microbial basal respiration from CO2 emitted by microbes, 3 days under laboratory conditions. Olinger et al. (1996). Methods in Soil Biology, pp 93 - 110"@en;
  dct:identifier "http://anzsoil.org/def/soil/au/edu/fed-uni/procedure/CO2-MBR"^^xsd:anyURI;
  rdfs:label "Microbial basal respiration by CO2 production - 3 days laboratory."@en;
  skos:definition "A procedure for calculating soil microbial basal respiration from CO2 emitted by microbes, 3 days under laboratory conditions. Olinger et al. (1996). Methods in Soil Biology, pp 93 - 110"@en;
  skos:inScheme <http://anzoil.org/def/soil/au/edu/fed-uni>;
  skos:notation "CO2-MBR";
  skos:prefLabel "Microbial basal respiration by CO2 production - 3 days laboratory."@en;
  skos:topConceptOf <http://anzoil.org/def/soil/au/edu/fed-uni> .

procedure:CO2-MIN-N a skos:Concept, sosa:Procedure;
  dct:description "A procedure esitmaing mineralisable nitrogen from CO2 production - 3 days under laboratory conditions. Franzluebbers (1999), Soil Biochem 31, pp1083 - 1090; Gilmore (2011), Crop Soils Mar - Apr 37 - 40; Paul (editor) 2004, Soil Microbiology Ecology and Boichemistry, 4th edn."@en;
  dct:identifier "http://anzsoil.org/def/soil/au/edu/fed-uni/procedure/CO2-MIN-N"^^xsd:anyURI;
  rdfs:label "Mineralisable nitrogen by CO2 - 3 days laboratory."@en;
  skos:definition "A procedure esitmaing mineralisable nitrogen from CO2 production - 3 days under laboratory conditions. Franzluebbers (1999), Soil Biochem 31, pp1083 - 1090; Gilmore (2011), Crop Soils Mar - Apr 37 - 40; Paul (editor) 2004, Soil Microbiology Ecology and Boichemistry, 4th edn."@en;
  skos:inScheme <http://anzoil.org/def/soil/au/edu/fed-uni>;
  skos:notation "CO2-MIN-N";
  skos:prefLabel "Mineralisable nitrogen by CO2 - 3 days laboratory."@en;
  skos:topConceptOf <http://anzoil.org/def/soil/au/edu/fed-uni> .

procedure:CO2-MIN-P a skos:Concept, sosa:Procedure;
  dct:description "A procedure esitmaing mineralisable phosphorus from CO2 production - 3 days under laboratory conditions. Franzluebbers (1999), Soil Biochem 31, pp1083 - 1090; Gilmore (2011), Crop Soils Mar - Apr 37 - 40; Paul (editor) 2004, Soil Microbiology Ecology and Boichemistry, 4th edn."@en;
  dct:identifier "http://anzsoil.org/def/soil/au/edu/fed-uni/procedure/CO2-MIN-P"^^xsd:anyURI;
  rdfs:label "Mineralisable phosphorus by CO2 - 3 days laboratory."@en;
  skos:definition "A procedure esitmaing mineralisable phosphorus from CO2 production - 3 days under laboratory conditions. Franzluebbers (1999), Soil Biochem 31, pp1083 - 1090; Gilmore (2011), Crop Soils Mar - Apr 37 - 40; Paul (editor) 2004, Soil Microbiology Ecology and Boichemistry, 4th edn."@en;
  skos:inScheme <http://anzoil.org/def/soil/au/edu/fed-uni>;
  skos:notation "CO2-MIN-P";
  skos:prefLabel "Mineralisable phosphorus by CO2 - 3 days laboratory."@en;
  skos:topConceptOf <http://anzoil.org/def/soil/au/edu/fed-uni> .

procedure:CO2-SBR-C a skos:Concept, sosa:Procedure;
  dct:description "A procedure for estimating soil microbial basal respiration from CO2 emitted by microbes. Reported as carbon. From 7 to 28 days in undisturbed soil under laboratory conditions. Olinger et al. (1996). Methods in Soil Biology, pp 93 - 110"@en;
  dct:identifier "http://anzsoil.org/def/soil/au/edu/fed-uni/procedure/CO2-SBR-C"^^xsd:anyURI;
  rdfs:label "Soil basal respiration - 7 - 28 days laboratory."@en;
  skos:definition "A procedure for estimating soil microbial basal respiration from CO2 emitted by microbes. Reported as carbon. From 7 to 28 days in undisturbed soil under laboratory conditions. Olinger et al. (1996). Methods in Soil Biology, pp 93 - 110"@en;
  skos:inScheme <http://anzoil.org/def/soil/au/edu/fed-uni>;
  skos:notation "CO2-SBR-C";
  skos:prefLabel "Soil basal respiration - 7 - 28 days laboratory."@en;
  skos:topConceptOf <http://anzoil.org/def/soil/au/edu/fed-uni> .

procedure:CO2-SMB a skos:Concept, sosa:Procedure;
  dct:description "A procedure for estimating soil microbial carbon from CO2 emitted by microbes, 3 days under laboratory conditions. Olinger et al. (1996). Methods in Soil Biology, pp 93 - 110"@en;
  dct:identifier "http://anzsoil.org/def/soil/au/edu/fed-uni/procedure/CO2-SMB"^^xsd:anyURI;
  rdfs:label "Soil microbial biomass by CO2 respiration - 3 days laboratory."@en;
  skos:definition "A procedure for estimating soil microbial carbon from CO2 emitted by microbes, 3 days under laboratory conditions. Olinger et al. (1996). Methods in Soil Biology, pp 93 - 110"@en;
  skos:inScheme <http://anzoil.org/def/soil/au/edu/fed-uni>;
  skos:notation "CO2-SMB";
  skos:prefLabel "Soil microbial biomass by CO2 respiration - 3 days laboratory."@en;
  skos:topConceptOf <http://anzoil.org/def/soil/au/edu/fed-uni> .

procedure:PLFA-DR a skos:Concept, sosa:Procedure;
  dct:description "A procedure extracting phospholipid fatty acids from the cell walls of soil biota, and then calculating an estimate of the soil biological related soil property of disease resistance"@en;
  dct:identifier "http://anzsoil.org/def/soil/au/edu/fed-uni/procedure/PLFA-DR"^^xsd:anyURI;
  rdfs:label "Disease resistance - by phospholipid fatty acid"@en;
  skos:definition "A procedure extracting phospholipid fatty acids from the cell walls of soil biota, and then calculating an estimate of the soil biological related soil property of disease resistance"@en;
  skos:inScheme <http://anzoil.org/def/soil/au/edu/fed-uni>;
  skos:notation "PLFA-DR";
  skos:prefLabel "Disease resistance - by phospholipid fatty acid"@en;
  skos:topConceptOf <http://anzoil.org/def/soil/au/edu/fed-uni> .

procedure:PLFA-DRR a skos:Concept, sosa:Procedure;
  dct:description "A procedure extracting phospholipid fatty acids from the cell walls of soil biota, and then calculating an estimate of the soil biological related soil property of drought resistance"@en;
  dct:identifier "http://anzsoil.org/def/soil/au/edu/fed-uni/procedure/PLFA-DRR"^^xsd:anyURI;
  rdfs:label "Drought resistance - by phospholipid fatty acid"@en;
  skos:definition "A procedure extracting phospholipid fatty acids from the cell walls of soil biota, and then calculating an estimate of the soil biological related soil property of drought resistance"@en;
  skos:inScheme <http://anzoil.org/def/soil/au/edu/fed-uni>;
  skos:notation "PLFA-DRR";
  skos:prefLabel "Drought resistance - by phospholipid fatty acid"@en;
  skos:topConceptOf <http://anzoil.org/def/soil/au/edu/fed-uni> .

procedure:PLFA-FB a skos:Concept, sosa:Procedure;
  dct:description "A procedure extracting phospholipid fatty acids from the cell walls of soil biota, and then calculating an estimate of fungal to bacterial ratio"@en;
  dct:identifier "http://anzsoil.org/def/soil/au/edu/fed-uni/procedure/PLFA-FB"^^xsd:anyURI;
  rdfs:label "Fungal to bacterial ratio - by phospholipid fatty acid"@en;
  skos:definition "A procedure extracting phospholipid fatty acids from the cell walls of soil biota, and then calculating an estimate of fungal to bacterial ratio"@en;
  skos:inScheme <http://anzoil.org/def/soil/au/edu/fed-uni>;
  skos:notation "PLFA-F/B";
  skos:prefLabel "Fungal to bacterial ratio - by phospholipid fatty acid"@en;
  skos:topConceptOf <http://anzoil.org/def/soil/au/edu/fed-uni> .

procedure:PLFA-MBAL a skos:Concept, sosa:Procedure;
  dct:description "A procedure extracting phospholipid fatty acids from the cell walls of soil biota, and then calculating an estimate of the soil biological related soil property of microbial balance"@en;
  dct:identifier "http://anzsoil.org/def/soil/au/edu/fed-uni/procedure/PLFA-MBAL"^^xsd:anyURI;
  rdfs:label "Microbial balance - by phospholipid fatty acid"@en;
  skos:definition "A procedure extracting phospholipid fatty acids from the cell walls of soil biota, and then calculating an estimate of the soil biological related soil property of microbial balance"@en;
  skos:inScheme <http://anzoil.org/def/soil/au/edu/fed-uni>;
  skos:notation "PLFA-MBAL";
  skos:prefLabel "Microbial balance - by phospholipid fatty acid"@en;
  skos:topConceptOf <http://anzoil.org/def/soil/au/edu/fed-uni> .

procedure:PLFA-MD a skos:Concept, sosa:Procedure;
  dct:description "A procedure extracting phospholipid fatty acids from the cell walls of soil biota, and then calculating an estimate of microbial diversity"@en;
  dct:identifier "http://anzsoil.org/def/soil/au/edu/fed-uni/procedure/PLFA-MD"^^xsd:anyURI;
  rdfs:label "Microbial diversity - by phospholipid fatty acid"@en;
  skos:definition "A procedure extracting phospholipid fatty acids from the cell walls of soil biota, and then calculating an estimate of microbial diversity"@en;
  skos:inScheme <http://anzoil.org/def/soil/au/edu/fed-uni>;
  skos:notation "PLFA-MD";
  skos:prefLabel "Microbial diversity - by phospholipid fatty acid"@en;
  skos:topConceptOf <http://anzoil.org/def/soil/au/edu/fed-uni> .

procedure:PLFA-MF-B a skos:Concept, sosa:Procedure;
  dct:description "A procedure extracting phospholipid fatty acids from the cell walls of soil biota, and then calculating an estimate of mycorrhizal fungi biomass"@en;
  dct:identifier "http://anzsoil.org/def/soil/au/edu/fed-uni/procedure/PLFA-MF-B"^^xsd:anyURI;
  rdfs:label "Mycorrhizal fungi biomass - by phospholipid fatty acid"@en;
  skos:definition "A procedure extracting phospholipid fatty acids from the cell walls of soil biota, and then calculating an estimate of mycorrhizal fungi biomass"@en;
  skos:inScheme <http://anzoil.org/def/soil/au/edu/fed-uni>;
  skos:notation "PLFA-MF-B";
  skos:prefLabel "Mycorrhizal fungi biomass - by phospholipid fatty acid"@en;
  skos:topConceptOf <http://anzoil.org/def/soil/au/edu/fed-uni> .

procedure:PLFA-NA-VAM a skos:Concept, sosa:Procedure;
  dct:description "A procedure extracting phospholipid fatty acids from the cell walls of soil biota, and then calculating an estimate of nutrient accessibility by vesicular mycorrhizal fungi (VAM)"@en;
  dct:identifier "http://anzsoil.org/def/soil/au/edu/fed-uni/procedure/PLFA-NA-VAM"^^xsd:anyURI;
  rdfs:label "Nutrient accessibility by VAM - by phospholipid fatty acid"@en;
  skos:definition "A procedure extracting phospholipid fatty acids from the cell walls of soil biota, and then calculating an estimate of nutrient accessibility by vesicular mycorrhizal fungi (VAM)"@en;
  skos:inScheme <http://anzoil.org/def/soil/au/edu/fed-uni>;
  skos:notation "PLFA-NA-VAM";
  skos:prefLabel "Nutrient accessibility by VAM - by phospholipid fatty acid"@en;
  skos:topConceptOf <http://anzoil.org/def/soil/au/edu/fed-uni> .

procedure:PLFA-NCR a skos:Concept, sosa:Procedure;
  dct:description "A procedure extracting phospholipid fatty acids from the cell walls of soil biota, and then calculating an estimate of the soil biological related soil property of nutrient cycling rate"@en;
  dct:identifier "http://anzsoil.org/def/soil/au/edu/fed-uni/procedure/PLFA-NCR"^^xsd:anyURI;
  rdfs:label "Nutrient cycling rate - by phospholipid fatty acid"@en;
  skos:definition "A procedure extracting phospholipid fatty acids from the cell walls of soil biota, and then calculating an estimate of the soil biological related soil property of nutrient cycling rate"@en;
  skos:inScheme <http://anzoil.org/def/soil/au/edu/fed-uni>;
  skos:notation "PLFA-NCR";
  skos:prefLabel "Nutrient cycling rate - by phospholipid fatty acid"@en;
  skos:topConceptOf <http://anzoil.org/def/soil/au/edu/fed-uni> .

procedure:PLFA-NSR a skos:Concept, sosa:Procedure;
  dct:description "A procedure extracting phospholipid fatty acids from the cell walls of soil biota, and then calculating an estimate of the soil biological related soil property of nutrient solubilisation rate"@en;
  dct:identifier "http://anzsoil.org/def/soil/au/edu/fed-uni/procedure/PLFA-NSR"^^xsd:anyURI;
  rdfs:label "Nutrient solubilisation rate - by phospholipid fatty acid"@en;
  skos:definition "A procedure extracting phospholipid fatty acids from the cell walls of soil biota, and then calculating an estimate of the soil biological related soil property of nutrient solubilisation rate"@en;
  skos:inScheme <http://anzoil.org/def/soil/au/edu/fed-uni>;
  skos:notation "PLFA-NSR";
  skos:prefLabel "Nutrient solubilisation rate - by phospholipid fatty acid"@en;
  skos:topConceptOf <http://anzoil.org/def/soil/au/edu/fed-uni> .

procedure:PLFA-PB a skos:Concept, sosa:Procedure;
  dct:description "A procedure extracting phospholipid fatty acids from the cell walls of soil biota, and then calculating an estimate of protozoan biomass"@en;
  dct:identifier "http://anzsoil.org/def/soil/au/edu/fed-uni/procedure/PLFA-PB"^^xsd:anyURI;
  rdfs:label "Protozoa biomass - by phospholipid fatty acid"@en;
  skos:definition "A procedure extracting phospholipid fatty acids from the cell walls of soil biota, and then calculating an estimate of protozoan biomass"@en;
  skos:inScheme <http://anzoil.org/def/soil/au/edu/fed-uni>;
  skos:notation "PLFA-PB";
  skos:prefLabel "Protozoa biomass - by phospholipid fatty acid"@en;
  skos:topConceptOf <http://anzoil.org/def/soil/au/edu/fed-uni> .

procedure:PLFA-RB a skos:Concept, sosa:Procedure;
  dct:description "A procedure extracting phospholipid fatty acids from the cell walls of soil biota, and then calculating an estimate of the soil biological related soil property of residue breakdown rate"@en;
  dct:identifier "http://anzsoil.org/def/soil/au/edu/fed-uni/procedure/PLFA-RB"^^xsd:anyURI;
  rdfs:label "Residue breakdown rate - by phospholipid fatty acid"@en;
  skos:definition "A procedure extracting phospholipid fatty acids from the cell walls of soil biota, and then calculating an estimate of the soil biological related soil property of residue breakdown rate"@en;
  skos:inScheme <http://anzoil.org/def/soil/au/edu/fed-uni>;
  skos:notation "PLFA-RB";
  skos:prefLabel "Residue breakdown rate - by phospholipid fatty acid"@en;
  skos:topConceptOf <http://anzoil.org/def/soil/au/edu/fed-uni> .

procedure:PLFA-TAB a skos:Concept, sosa:Procedure;
  dct:description "A procedure extracting phospholipid fatty acids from the cell walls of soil biota, and then calculating an estimate of true anaerobe biomass"@en;
  dct:identifier "http://anzsoil.org/def/soil/au/edu/fed-uni/procedure/PLFA-TAB"^^xsd:anyURI;
  rdfs:label "True anaerobe biomass - by phospholipid fatty acid"@en;
  skos:definition "A procedure extracting phospholipid fatty acids from the cell walls of soil biota, and then calculating an estimate of true anaerobe biomass"@en;
  skos:inScheme <http://anzoil.org/def/soil/au/edu/fed-uni>;
  skos:notation "PLFA-TAB";
  skos:prefLabel "True anaerobe biomass - by phospholipid fatty acid"@en;
  skos:topConceptOf <http://anzoil.org/def/soil/au/edu/fed-uni> .

procedure:PLFA-TBB a skos:Concept, sosa:Procedure;
  dct:description "A procedure extracting phospholipid fatty acids from the cell walls of soil biota, and then calculating an estimate of total bacterial biomass"@en;
  dct:identifier "http://anzsoil.org/def/soil/au/edu/fed-uni/procedure/PLFA-TBB"^^xsd:anyURI;
  rdfs:label "Total bacterial biomass - by phospholipid fatty acid"@en;
  skos:definition "A procedure extracting phospholipid fatty acids from the cell walls of soil biota, and then calculating an estimate of total bacterial biomass"@en;
  skos:inScheme <http://anzoil.org/def/soil/au/edu/fed-uni>;
  skos:notation "PLFA-TBB";
  skos:prefLabel "Total bacterial biomass - by phospholipid fatty acid"@en;
  skos:topConceptOf <http://anzoil.org/def/soil/au/edu/fed-uni> .

procedure:PLFA-TFB a skos:Concept, sosa:Procedure;
  dct:description "A procedure extracting phospholipid fatty acids from the cell walls of soil biota, and then calculating an estimate of total funal biomass"@en;
  dct:identifier "http://anzsoil.org/def/soil/au/edu/fed-uni/procedure/PLFA-TFB"^^xsd:anyURI;
  rdfs:label "Total fungal biomass - by phospholipid fatty acid"@en;
  skos:definition "A procedure extracting phospholipid fatty acids from the cell walls of soil biota, and then calculating an estimate of total funal biomass"@en;
  skos:inScheme <http://anzoil.org/def/soil/au/edu/fed-uni>;
  skos:notation "PLFA-TFB";
  skos:prefLabel "Total fungal biomass - by phospholipid fatty acid"@en;
  skos:topConceptOf <http://anzoil.org/def/soil/au/edu/fed-uni> .

procedure:PLFA-TMB a skos:Concept, sosa:Procedure;
  dct:description "A procedure extracting phospholipid fatty acids from the cell walls of soil biota, and then calculating an estimate of total microbial biomass"@en;
  dct:identifier "http://anzsoil.org/def/soil/au/edu/fed-uni/procedure/PLFA-TMB"^^xsd:anyURI;
  rdfs:label "Total microbial biomass - by phospholipid fatty acid"@en;
  skos:definition "A procedure extracting phospholipid fatty acids from the cell walls of soil biota, and then calculating an estimate of total microbial biomass"@en;
  skos:inScheme <http://anzoil.org/def/soil/au/edu/fed-uni>;
  skos:notation "PLFA-TMB";
  skos:prefLabel "Total microbial biomass - by phospholipid fatty acid"@en;
  skos:topConceptOf <http://anzoil.org/def/soil/au/edu/fed-uni> .

procedure:SC-30-NETP a skos:Concept, sosa:Procedure;
  dct:description "A procedure measuring phosphorus solubilisation (mineralisation) by soil microbes and P 'lock-up' (immobilisation) over one month under a simulated crop (at 28 degrees Celsius and 30 % mycorrhizal colonisation). Net P release is the net increase in plant-available P due to solubilisation by microbes above any solubilised P that becomes locked up again over one month. Assumes a sampling depth of 10 cm and a bulk density (BD) of 1.2 kg/L. For other depths and densities use mg/kg x(depth (cm)/10) x BD (g/mL)"@en;
  dct:identifier "http://anzsoil.org/def/soil/au/edu/fed-uni/procedure/SC-30-NETP"^^xsd:anyURI;
  rdfs:label "Net phosphorus release - simulated crop 30 days"@en;
  skos:definition "A procedure measuring phosphorus solubilisation (mineralisation) by soil microbes and P 'lock-up' (immobilisation) over one month under a simulated crop (at 28 degrees Celsius and 30 % mycorrhizal colonisation). Net P release is the net increase in plant-available P due to solubilisation by microbes above any solubilised P that becomes locked up again over one month. Assumes a sampling depth of 10 cm and a bulk density (BD) of 1.2 kg/L. For other depths and densities use mg/kg x(depth (cm)/10) x BD (g/mL)"@en;
  skos:inScheme <http://anzoil.org/def/soil/au/edu/fed-uni>;
  skos:notation "SC-30-NETP";
  skos:prefLabel "Net phosphorus release - simulated crop 30 days"@en;
  skos:topConceptOf <http://anzoil.org/def/soil/au/edu/fed-uni> .

procedure:SC-30-NFIX a skos:Concept, sosa:Procedure;
  dct:description "A procedure measuring the amount of N fixed from atmospheric N predominately by microbial action, under a simulated crop, 28 degrees Celsius, 30 % mycorrhizal colonisation, one month"@en;
  dct:identifier "http://anzsoil.org/def/soil/au/edu/fed-uni/procedure/SC-30-NFIX"^^xsd:anyURI;
  rdfs:label "N fixation - simulated crop 30 days"@en;
  skos:definition "A procedure measuring the amount of N fixed from atmospheric N predominately by microbial action, under a simulated crop, 28 degrees Celsius, 30 % mycorrhizal colonisation, one month"@en;
  skos:inScheme <http://anzoil.org/def/soil/au/edu/fed-uni>;
  skos:notation "SC-30-NFIX";
  skos:prefLabel "N fixation - simulated crop 30 days"@en;
  skos:topConceptOf <http://anzoil.org/def/soil/au/edu/fed-uni> .

procedure:SC-30-NMIN a skos:Concept, sosa:Procedure;
  dct:description "A procedure measuring the amount of ammonium N (NH4) converted to nitrate N (NO3) by microbial action after 7 days under a simulated crop"@en;
  dct:identifier "http://anzsoil.org/def/soil/au/edu/fed-uni/procedure/SC-30-NMIN"^^xsd:anyURI;
  rdfs:label "N mineralisation - simulated crop 30 days"@en;
  skos:definition "A procedure measuring the amount of ammonium N (NH4) converted to nitrate N (NO3) by microbial action after 7 days under a simulated crop"@en;
  skos:inScheme <http://anzoil.org/def/soil/au/edu/fed-uni>;
  skos:notation "SC-30-NMIN";
  skos:prefLabel "N mineralisation - simulated crop 30 days"@en;
  skos:topConceptOf <http://anzoil.org/def/soil/au/edu/fed-uni> .

procedure:SC-30-NR a skos:Concept, sosa:Procedure;
  dct:description "A procedure measuing N release on rewetting, under simulated crop conditions over one month"@en;
  dct:identifier "http://anzsoil.org/def/soil/au/edu/fed-uni/procedure/SC-30-NR"^^xsd:anyURI;
  rdfs:label "N release - simulated crop 30 days"@en;
  skos:definition "A procedure measuing N release on rewetting, under simulated crop conditions over one month"@en;
  skos:inScheme <http://anzoil.org/def/soil/au/edu/fed-uni>;
  skos:notation "SC-30-NR";
  skos:prefLabel "N release - simulated crop 30 days"@en;
  skos:topConceptOf <http://anzoil.org/def/soil/au/edu/fed-uni> .

procedure:SC-7-PFERT a skos:Concept, sosa:Procedure;
  dct:description "A procedure measuring soluble Phosphorus remaining after 7 days under simulated crop (at 28 degrees Celsius and 30 % mycorrhizal colonisation). Assumes a sampling depth of 10 cm and a bulk density (BD) of 1.2 kg/L. For other depths and densities use mg/kg x (depth (cm)/10) x BD (g/mL). It is assumed the field minimum is 5 %"@en;
  dct:identifier "http://anzsoil.org/def/soil/au/edu/fed-uni/procedure/SC-7-PFERT"^^xsd:anyURI;
  rdfs:label "P fertiliser availablity - simulated crop 7 days"@en;
  skos:definition "A procedure measuring soluble Phosphorus remaining after 7 days under simulated crop (at 28 degrees Celsius and 30 % mycorrhizal colonisation). Assumes a sampling depth of 10 cm and a bulk density (BD) of 1.2 kg/L. For other depths and densities use mg/kg x (depth (cm)/10) x BD (g/mL). It is assumed the field minimum is 5 %"@en;
  skos:inScheme <http://anzoil.org/def/soil/au/edu/fed-uni>;
  skos:notation "SC-7-PFERT";
  skos:prefLabel "P fertiliser availablity - simulated crop 7 days"@en;
  skos:topConceptOf <http://anzoil.org/def/soil/au/edu/fed-uni> .

procedure:SC-7-PREL a skos:Concept, sosa:Procedure;
  dct:description "A procedure measuring the amount of plant available P mineralised from total P per week (at 28 degrees Celsius and 30 % mycorrhizal colonisation). Measured under simulated crop. Assumes a sampling depth of 10 cm and a bulk density (BD) of 1.2 kg/L. For other depths and densities use mg/kg x(depth (cm)/10) x BD (g/mL)"@en;
  dct:identifier "http://anzsoil.org/def/soil/au/edu/fed-uni/procedure/SC-7-PREL"^^xsd:anyURI;
  rdfs:label "Phosphorus release - simulated crop 7 days"@en;
  skos:definition "A procedure measuring the amount of plant available P mineralised from total P per week (at 28 degrees Celsius and 30 % mycorrhizal colonisation). Measured under simulated crop. Assumes a sampling depth of 10 cm and a bulk density (BD) of 1.2 kg/L. For other depths and densities use mg/kg x(depth (cm)/10) x BD (g/mL)"@en;
  skos:inScheme <http://anzoil.org/def/soil/au/edu/fed-uni>;
  skos:notation "SC-7-PREL";
  skos:prefLabel "Phosphorus release - simulated crop 7 days"@en;
  skos:topConceptOf <http://anzoil.org/def/soil/au/edu/fed-uni> .

procedure:WP-P a skos:Concept, sosa:Procedure;
  dct:description "Soil P procedure - Wutscher and Perkins"@en;
  dct:identifier "http://anzsoil.org/def/soil/au/edu/fed-uni/procedure/WP-P"^^xsd:anyURI;
  rdfs:label "Phosphorus procedure - Wutscher and Perkins"@en;
  skos:definition "Soil P procedure - Wutscher and Perkins"@en;
  skos:inScheme <http://anzoil.org/def/soil/au/edu/fed-uni>;
  skos:notation "WP-P";
  skos:prefLabel "Phosphorus procedure - Wutscher and Perkins"@en;
  skos:topConceptOf <http://anzoil.org/def/soil/au/edu/fed-uni> .

procedure:AL a skos:Concept, sosa:Procedure;
  dct:description "A procedure for measuring Aluminium"@en;
  dct:identifier "http://anzsoil.org/def/soil/au/edu/fed-uni/procedure/AL"^^xsd:anyURI;
  rdfs:label "Aluminium procedure"@en;
  skos:definition "A procedure for measuring Aluminium"@en;
  skos:inScheme <http://anzoil.org/def/soil/au/edu/fed-uni>;
  skos:notation "AL";
  skos:prefLabel "Aluminium procedure"@en;
  skos:topConceptOf <http://anzoil.org/def/soil/au/edu/fed-uni> .

procedure:CO a skos:Concept, sosa:Procedure;
  dct:description "A procedure for measuring Cobalt"@en;
  dct:identifier "http://anzsoil.org/def/soil/au/edu/fed-uni/procedure/CO"^^xsd:anyURI;
  rdfs:label "Cobalt procedure"@en;
  skos:definition "A procedure for measuring Cobalt"@en;
  skos:inScheme <http://anzoil.org/def/soil/au/edu/fed-uni>;
  skos:notation "CO";
  skos:prefLabel "Cobalt procedure"@en;
  skos:topConceptOf <http://anzoil.org/def/soil/au/edu/fed-uni> .

procedure:MO a skos:Concept, sosa:Procedure;
  dct:description "A procedure for measuring Molybdenum"@en;
  dct:identifier "http://anzsoil.org/def/soil/au/edu/fed-uni/procedure/MO"^^xsd:anyURI;
  rdfs:label "Molybdenum procedure"@en;
  skos:definition "A procedure for measuring Molybdenum"@en;
  skos:inScheme <http://anzoil.org/def/soil/au/edu/fed-uni>;
  skos:notation "MO";
  skos:prefLabel "Molybdenum procedure"@en;
  skos:topConceptOf <http://anzoil.org/def/soil/au/edu/fed-uni> .

procedure:SE a skos:Concept, sosa:Procedure;
  dct:description "A procedure for measuring Selenium"@en;
  dct:identifier "http://anzsoil.org/def/soil/au/edu/fed-uni/procedure/SE"^^xsd:anyURI;
  rdfs:label "Selenium procedure"@en;
  skos:definition "A procedure for measuring Selenium"@en;
  skos:inScheme <http://anzoil.org/def/soil/au/edu/fed-uni>;
  skos:notation "SE";
  skos:prefLabel "Selenium procedure"@en;
  skos:topConceptOf <http://anzoil.org/def/soil/au/edu/fed-uni> .

procedure:SI a skos:Concept, sosa:Procedure;
  dct:description "A procedure for measuring Silicon"@en;
  dct:identifier "http://anzsoil.org/def/soil/au/edu/fed-uni/procedure/SI"^^xsd:anyURI;
  rdfs:label "Silicon procedure"@en;
  skos:definition "A procedure for measuring Silicon"@en;
  skos:inScheme <http://anzoil.org/def/soil/au/edu/fed-uni>;
  skos:notation "SI";
  skos:prefLabel "Silicon procedure"@en;
  skos:topConceptOf <http://anzoil.org/def/soil/au/edu/fed-uni> .

procedure:WE-OC a skos:Concept, sosa:Procedure;
  dct:description "A procedure for measuring water-extractable Carbon. Haney, R.L. et al. 2012. Soil Organic C:N vs. water-extractable organic C:N. Open Journal of Soil Science, 2012, 2, 269-274."@en;
  dct:identifier "http://anzsoil.org/def/soil/au/edu/fed-uni/procedure/WE-OC"^^xsd:anyURI;
  rdfs:label "Water extractable organic carbon procedure"@en;
  skos:definition "A procedure for measuring water-extractable Carbon. Haney, R.L. et al. 2012. Soil Organic C:N vs. water-extractable organic C:N. Open Journal of Soil Science, 2012, 2, 269-274."@en;
  skos:inScheme <http://anzoil.org/def/soil/au/edu/fed-uni>;
  skos:notation "WE-OC";
  skos:prefLabel "Water extractable organic carbon procedure"@en;
  skos:topConceptOf <http://anzoil.org/def/soil/au/edu/fed-uni> .

procedure:WE-ON a skos:Concept, sosa:Procedure;
  dct:description "A procedure for measuring water-extractable organic Nitrogen. Haney, R.L. et al. 2012. Soil Organic C:N vs. water-extractable organic C:N. Open Journal of Soil Science, 2012, 2, 269-274."@en;
  dct:identifier "http://anzsoil.org/def/soil/au/edu/fed-uni/procedure/WE-ON"^^xsd:anyURI;
  rdfs:label "Water extractable organic nitrogen procedure"@en;
  skos:definition "A procedure for measuring water-extractable organic Nitrogen. Haney, R.L. et al. 2012. Soil Organic C:N vs. water-extractable organic C:N. Open Journal of Soil Science, 2012, 2, 269-274."@en;
  skos:inScheme <http://anzoil.org/def/soil/au/edu/fed-uni>;
  skos:notation "WE-ON";
  skos:prefLabel "Water extractable organic nitrogen procedure"@en;
  skos:topConceptOf <http://anzoil.org/def/soil/au/edu/fed-uni> .

procedure:18F1-S a skos:Concept, sosa:Procedure;
  dct:description "A procedure for measuring Sulfur by Mehlich-3"@en;
  dct:identifier "http://anzsoil.org/def/soil/au/edu/fed-uni/procedure/18F1-S"^^xsd:anyURI;
  rdfs:label "Mehlich 3-extractable S"@en;
  skos:definition "A procedure for measuring Sulfur by Mehlich-3"@en;
  skos:inScheme <http://anzoil.org/def/soil/au/edu/fed-uni>;
  skos:notation "18F1-S";
  skos:prefLabel "Mehlich 3-extractable S"@en;
  skos:topConceptOf <http://anzoil.org/def/soil/au/edu/fed-uni> .

procedure:PH a skos:Concept, sosa:Procedure;
  dct:description "A procedure for measuring soil pH"@en;
  dct:identifier "http://anzsoil.org/def/soil/au/edu/fed-uni/procedure/PH"^^xsd:anyURI;
  rdfs:label "Soil pH procedure"@en;
  skos:definition "A procedure for measuring soil pH"@en;
  skos:inScheme <http://anzoil.org/def/soil/au/edu/fed-uni>;
  skos:notation "pH";
  skos:prefLabel "Soil pH procedure"@en;
  skos:topConceptOf <http://anzoil.org/def/soil/au/edu/fed-uni> .

procedure:S10-CA a skos:Concept, sosa:Procedure;
  dct:description "A procedure for measuring Calcium by Morgan 1 Inhouse Method S10 EAL Environmental Analysis Laboratory Southern Cross University, Based on Morgan 1941"@en;
  dct:identifier "http://anzsoil.org/def/soil/au/edu/fed-uni/procedure/S10-CA"^^xsd:anyURI;
  rdfs:label "Morgan 1 EAL - Ca"@en;
  skos:definition "A procedure for measuring Calcium by Morgan 1 Inhouse Method S10 EAL Environmental Analysis Laboratory Southern Cross University, Based on Morgan 1941"@en;
  skos:inScheme <http://anzoil.org/def/soil/au/edu/fed-uni>;
  skos:notation "S10-CA";
  skos:prefLabel "Morgan 1 EAL - Ca"@en;
  skos:topConceptOf <http://anzoil.org/def/soil/au/edu/fed-uni> .

procedure:S10-MG a skos:Concept, sosa:Procedure;
  dct:description "A procedure for measuring Magnesium by Morgan 1 Inhouse Method S10 EAL Environmental Analysis Laboratory Southern Cross University, Based on Morgan 1941"@en;
  dct:identifier "http://anzsoil.org/def/soil/au/edu/fed-uni/procedure/S10-MG"^^xsd:anyURI;
  rdfs:label "Morgan 1 EAL - Mg"@en;
  skos:definition "A procedure for measuring Magnesium by Morgan 1 Inhouse Method S10 EAL Environmental Analysis Laboratory Southern Cross University, Based on Morgan 1941"@en;
  skos:inScheme <http://anzoil.org/def/soil/au/edu/fed-uni>;
  skos:notation "S10-MG";
  skos:prefLabel "Morgan 1 EAL - Mg"@en;
  skos:topConceptOf <http://anzoil.org/def/soil/au/edu/fed-uni> .

procedure:S10-K a skos:Concept, sosa:Procedure;
  dct:description "A procedure for measuring Potassium by Morgan 1 Inhouse Method S10 EAL Environmental Analysis Laboratory Southern Cross University, Based on Morgan 1941"@en;
  dct:identifier "http://anzsoil.org/def/soil/au/edu/fed-uni/procedure/S10-K"^^xsd:anyURI;
  rdfs:label "Morgan 1 EAL - K"@en;
  skos:definition "A procedure for measuring Potassium by Morgan 1 Inhouse Method S10 EAL Environmental Analysis Laboratory Southern Cross University, Based on Morgan 1941"@en;
  skos:inScheme <http://anzoil.org/def/soil/au/edu/fed-uni>;
  skos:notation "S10-K";
  skos:prefLabel "Morgan 1 EAL - K"@en;
  skos:topConceptOf <http://anzoil.org/def/soil/au/edu/fed-uni> .

procedure:S10-P a skos:Concept, sosa:Procedure;
  dct:description "A procedure for measuring Phosphorus by Morgan 1 Inhouse Method S10 EAL Environmental Analysis Laboratory Southern Cross University, Based on Morgan 1941"@en;
  dct:identifier "http://anzsoil.org/def/soil/au/edu/fed-uni/procedure/S10-P"^^xsd:anyURI;
  rdfs:label "Morgan 1 EAL - P"@en;
  skos:definition "A procedure for measuring Phosphorus by Morgan 1 Inhouse Method S10 EAL Environmental Analysis Laboratory Southern Cross University, Based on Morgan 1941"@en;
  skos:inScheme <http://anzoil.org/def/soil/au/edu/fed-uni>;
  skos:notation "S10-P";
  skos:prefLabel "Morgan 1 EAL - P"@en;
  skos:topConceptOf <http://anzoil.org/def/soil/au/edu/fed-uni> .

procedure:15M1-CNR a skos:Concept, sosa:Procedure;
  dct:description "A procedure for measuring Carbon to Nitrogen Ratio"@en;
  dct:identifier "http://anzsoil.org/def/soil/au/edu/fed-uni/procedure/15M1-CNR"^^xsd:anyURI;
  rdfs:label "Carbon to Nitrogen Ratio procedure"@en;
  skos:definition "A procedure for measuring Carbon to Nitrogen Ratio"@en;
  skos:inScheme <http://anzoil.org/def/soil/au/edu/fed-uni>;
  skos:notation "15M1-C/N";
  skos:prefLabel "Carbon to Nitrogen Ratio procedure"@en;
  skos:topConceptOf <http://anzoil.org/def/soil/au/edu/fed-uni> .

procedure:6A1-MOD a skos:Concept, sosa:Procedure;
  dct:description "Procedure measuring Soil Organic Matter (SOM) - Modified from W&B mehod 6A1 Soil Chemical Methods Australasia 1. (2011), by George E Rayment and David J Lyons"@en;
  dct:identifier "http://anzsoil.org/def/soil/au/edu/fed-uni/procedure/6A1-MOD"^^xsd:anyURI;
  rdfs:label "Soil Organic Matter (SOM) - Modified W&B"@en;
  skos:definition "Procedure measuring Soil Organic Matter (SOM) - Modified from W&B mehod 6A1 Soil Chemical Methods Australasia 1. (2011), by George E Rayment and David J Lyons"@en;
  skos:inScheme <http://anzoil.org/def/soil/au/edu/fed-uni>;
  skos:notation "6A1-MOD";
  skos:prefLabel "Soil Organic Matter (SOM) - Modified W&B"@en;
  skos:topConceptOf <http://anzoil.org/def/soil/au/edu/fed-uni> .

procedure:TAE-CA a skos:Concept, sosa:Procedure;
  dct:description "A procedure for measuring total acid extractable Calcium"@en;
  dct:identifier "http://anzsoil.org/def/soil/au/edu/fed-uni/procedure/TAE-CA"^^xsd:anyURI;
  rdfs:label "Total acid extractable Calcium procedure"@en;
  skos:definition "A procedure for measuring total acid extractable Calcium"@en;
  skos:inScheme <http://anzoil.org/def/soil/au/edu/fed-uni>;
  skos:notation "TAE-CA";
  skos:prefLabel "Total acid extractable Calcium procedure"@en;
  skos:topConceptOf <http://anzoil.org/def/soil/au/edu/fed-uni> .

procedure:TAE-MG a skos:Concept, sosa:Procedure;
  dct:description "A procedure for measuring total acid extractable Magnesium"@en;
  dct:identifier "http://anzsoil.org/def/soil/au/edu/fed-uni/procedure/TAE-MG"^^xsd:anyURI;
  rdfs:label "Total acid extractable Magnesium procedure"@en;
  skos:definition "A procedure for measuring total acid extractable Magnesium"@en;
  skos:inScheme <http://anzoil.org/def/soil/au/edu/fed-uni>;
  skos:notation "TAE-MG";
  skos:prefLabel "Total acid extractable Magnesium procedure"@en;
  skos:topConceptOf <http://anzoil.org/def/soil/au/edu/fed-uni> .

procedure:TAE-K a skos:Concept, sosa:Procedure;
  dct:description "A procedure for measuring total acid extractable Potassium"@en;
  dct:identifier "http://anzsoil.org/def/soil/au/edu/fed-uni/procedure/TAE-K"^^xsd:anyURI;
  rdfs:label "Total acid extractable Potassium procedure"@en;
  skos:definition "A procedure for measuring total acid extractable Potassium"@en;
  skos:inScheme <http://anzoil.org/def/soil/au/edu/fed-uni>;
  skos:notation "TAE-K";
  skos:prefLabel "Total acid extractable Potassium procedure"@en;
  skos:topConceptOf <http://anzoil.org/def/soil/au/edu/fed-uni> .

procedure:TAE-NA a skos:Concept, sosa:Procedure;
  dct:description "A procedure for measuring total acid extractable Sodium"@en;
  dct:identifier "http://anzsoil.org/def/soil/au/edu/fed-uni/procedure/TAE-NA"^^xsd:anyURI;
  rdfs:label "Total acid extractable Sodium procedure"@en;
  skos:definition "A procedure for measuring total acid extractable Sodium"@en;
  skos:inScheme <http://anzoil.org/def/soil/au/edu/fed-uni>;
  skos:notation "TAE-NA";
  skos:prefLabel "Total acid extractable Sodium procedure"@en;
  skos:topConceptOf <http://anzoil.org/def/soil/au/edu/fed-uni> .

procedure:TAE-S a skos:Concept, sosa:Procedure;
  dct:description "A procedure for measuring total acid extractable Sulfur"@en;
  dct:identifier "http://anzsoil.org/def/soil/au/edu/fed-uni/procedure/TAE-S"^^xsd:anyURI;
  rdfs:label "Total acid extractable Sulfur procedure"@en;
  skos:definition "A procedure for measuring total acid extractable Sulfur"@en;
  skos:inScheme <http://anzoil.org/def/soil/au/edu/fed-uni>;
  skos:notation "TAE-S";
  skos:prefLabel "Total acid extractable Sulfur procedure"@en;
  skos:topConceptOf <http://anzoil.org/def/soil/au/edu/fed-uni> .

procedure:TAE-P a skos:Concept, sosa:Procedure;
  dct:description "A procedure for measuring total acid extractable Phosphorus"@en;
  dct:identifier "http://anzsoil.org/def/soil/au/edu/fed-uni/procedure/TAE-P"^^xsd:anyURI;
  rdfs:label "Total acid extractable Phosphorus procedure"@en;
  skos:definition "A procedure for measuring total acid extractable Phosphorus"@en;
  skos:inScheme <http://anzoil.org/def/soil/au/edu/fed-uni>;
  skos:notation "TAE-P";
  skos:prefLabel "Total acid extractable Phosphorus procedure"@en;
  skos:topConceptOf <http://anzoil.org/def/soil/au/edu/fed-uni> .

procedure:TAE-ZN a skos:Concept, sosa:Procedure;
  dct:description "A procedure for measuring total acid extractable Zinc"@en;
  dct:identifier "http://anzsoil.org/def/soil/au/edu/fed-uni/procedure/TAE-ZN"^^xsd:anyURI;
  rdfs:label "Total acid extractable Zinc procedure"@en;
  skos:definition "A procedure for measuring total acid extractable Zinc"@en;
  skos:inScheme <http://anzoil.org/def/soil/au/edu/fed-uni>;
  skos:notation "TAE-ZN";
  skos:prefLabel "Total acid extractable Zinc procedure"@en;
  skos:topConceptOf <http://anzoil.org/def/soil/au/edu/fed-uni> .

procedure:TAE-MN a skos:Concept, sosa:Procedure;
  dct:description "A procedure for measuring total acid extractable Manganese"@en;
  dct:identifier "http://anzsoil.org/def/soil/au/edu/fed-uni/procedure/TAE-MN"^^xsd:anyURI;
  rdfs:label "Total acid extractable Manganese procedure"@en;
  skos:definition "A procedure for measuring total acid extractable Manganese"@en;
  skos:inScheme <http://anzoil.org/def/soil/au/edu/fed-uni>;
  skos:notation "TAE-MN";
  skos:prefLabel "Total acid extractable Manganese procedure"@en;
  skos:topConceptOf <http://anzoil.org/def/soil/au/edu/fed-uni> .

procedure:TAE-FE a skos:Concept, sosa:Procedure;
  dct:description "A procedure for measuring total acid extractable Iron"@en;
  dct:identifier "http://anzsoil.org/def/soil/au/edu/fed-uni/procedure/TAE-FE"^^xsd:anyURI;
  rdfs:label "Total acid extractable Iron procedure"@en;
  skos:definition "A procedure for measuring total acid extractable Iron"@en;
  skos:inScheme <http://anzoil.org/def/soil/au/edu/fed-uni>;
  skos:notation "TAE-FE";
  skos:prefLabel "Total acid extractable Iron procedure"@en;
  skos:topConceptOf <http://anzoil.org/def/soil/au/edu/fed-uni> .

procedure:TAE-CU a skos:Concept, sosa:Procedure;
  dct:description "A procedure for measuring total acid extractable Copper"@en;
  dct:identifier "http://anzsoil.org/def/soil/au/edu/fed-uni/procedure/TAE-CU"^^xsd:anyURI;
  rdfs:label "Total acid extractable Copper procedure"@en;
  skos:definition "A procedure for measuring total acid extractable Copper"@en;
  skos:inScheme <http://anzoil.org/def/soil/au/edu/fed-uni>;
  skos:notation "TAE-CU";
  skos:prefLabel "Total acid extractable Copper procedure"@en;
  skos:topConceptOf <http://anzoil.org/def/soil/au/edu/fed-uni> .

procedure:TAE-B a skos:Concept, sosa:Procedure;
  dct:description "A procedure for measuring total acid extractable Boron"@en;
  dct:identifier "http://anzsoil.org/def/soil/au/edu/fed-uni/procedure/TAE-B"^^xsd:anyURI;
  rdfs:label "Total acid extractable Boron procedure"@en;
  skos:definition "A procedure for measuring total acid extractable Boron"@en;
  skos:inScheme <http://anzoil.org/def/soil/au/edu/fed-uni>;
  skos:notation "TAE-B";
  skos:prefLabel "Total acid extractable Boron procedure"@en;
  skos:topConceptOf <http://anzoil.org/def/soil/au/edu/fed-uni> .

procedure:TAE-SI a skos:Concept, sosa:Procedure;
  dct:description "A procedure for measuring total acid extractable Silicon"@en;
  dct:identifier "http://anzsoil.org/def/soil/au/edu/fed-uni/procedure/TAE-SI"^^xsd:anyURI;
  rdfs:label "Total acid extractable Silicon procedure"@en;
  skos:definition "A procedure for measuring total acid extractable Silicon"@en;
  skos:inScheme <http://anzoil.org/def/soil/au/edu/fed-uni>;
  skos:notation "TAE-SI";
  skos:prefLabel "Total acid extractable Silicon procedure"@en;
  skos:topConceptOf <http://anzoil.org/def/soil/au/edu/fed-uni> .

procedure:TAE-AL a skos:Concept, sosa:Procedure;
  dct:description "A procedure for measuring total acid extractable Aluminium"@en;
  dct:identifier "http://anzsoil.org/def/soil/au/edu/fed-uni/procedure/TAE-AL"^^xsd:anyURI;
  rdfs:label "Total acid extractable Aluminium procedure"@en;
  skos:definition "A procedure for measuring total acid extractable Aluminium"@en;
  skos:inScheme <http://anzoil.org/def/soil/au/edu/fed-uni>;
  skos:notation "TAE-AL";
  skos:prefLabel "Total acid extractable Aluminium procedure"@en;
  skos:topConceptOf <http://anzoil.org/def/soil/au/edu/fed-uni> .

procedure:TAE-MO a skos:Concept, sosa:Procedure;
  dct:description "A procedure for measuring total acid extractable Molybdenum"@en;
  dct:identifier "http://anzsoil.org/def/soil/au/edu/fed-uni/procedure/TAE-MO"^^xsd:anyURI;
  rdfs:label "Total acid extractable Molybdenum procedure"@en;
  skos:definition "A procedure for measuring total acid extractable Molybdenum"@en;
  skos:inScheme <http://anzoil.org/def/soil/au/edu/fed-uni>;
  skos:notation "TAE-MO";
  skos:prefLabel "Total acid extractable Molybdenum procedure"@en;
  skos:topConceptOf <http://anzoil.org/def/soil/au/edu/fed-uni> .

procedure:TAE-CO a skos:Concept, sosa:Procedure;
  dct:description "A procedure for measuring total acid extractable Cobalt"@en;
  dct:identifier "http://anzsoil.org/def/soil/au/edu/fed-uni/procedure/TAE-CO"^^xsd:anyURI;
  rdfs:label "Total acid extractable Cobalt procedure"@en;
  skos:definition "A procedure for measuring total acid extractable Cobalt"@en;
  skos:inScheme <http://anzoil.org/def/soil/au/edu/fed-uni>;
  skos:notation "TAE-CO";
  skos:prefLabel "Total acid extractable Cobalt procedure"@en;
  skos:topConceptOf <http://anzoil.org/def/soil/au/edu/fed-uni> .

procedure:TAE-SE a skos:Concept, sosa:Procedure;
  dct:description "A procedure for measuring total acid extractable Selenium"@en;
  dct:identifier "http://anzsoil.org/def/soil/au/edu/fed-uni/procedure/TAE-SE"^^xsd:anyURI;
  rdfs:label "Total acid extractable Selenium procedure"@en;
  skos:definition "A procedure for measuring total acid extractable Selenium"@en;
  skos:inScheme <http://anzoil.org/def/soil/au/edu/fed-uni>;
  skos:notation "TAE-SE";
  skos:prefLabel "Total acid extractable Selenium procedure"@en;
  skos:topConceptOf <http://anzoil.org/def/soil/au/edu/fed-uni> .

procedure:15D1-BACL-CA a skos:Concept, sosa:Procedure;
  dct:description "This procedure is a calculation of exchangeable calcium from ‘Adjusted Cation Exchange Capacity’ (CEC) where Adjusted CEC is calculated by subtracting ‘Adjusted Hydrogen’ from CEC. The underlying methods are: 1. for exchangeable bases (Ca2+, Mg2+ , Na+ and K+) - 15D1 of Rayment and Lyons 2011l- 1 M ammonium acetate at pH 7.0, pre-treatment for soluble salts, manual leach and 2. ‘Adjusted Hydrogen’ - A procedure for measuring H+ by Barium Chloride-Triethanolamine method. Reference: Peech, M., Cowan, R.L. & Baker, J.H. (1962). Soil Science Society American Procedures, A critical study of the Barium chloride-Triethanolamine and ammonium acetate methods for determining exchangeable Hydrogen of soils."@en;
  dct:identifier "http://anzsoil.org/def/soil/au/edu/fed-uni/procedure/15D1-BACL-CA"^^xsd:anyURI;
  rdfs:label "Exchangable calcium procedure - 15D1 and Barium Chloride-Triethanolamine"@en;
  skos:definition "This procedure is a calculation of exchangeable calcium from ‘Adjusted Cation Exchange Capacity’ (CEC) where Adjusted CEC is calculated by subtracting ‘Adjusted Hydrogen’ from CEC. The underlying methods are: 1. for exchangeable bases (Ca2+, Mg2+ , Na+ and K+) - 15D1 of Rayment and Lyons 2011l- 1 M ammonium acetate at pH 7.0, pre-treatment for soluble salts, manual leach and 2. ‘Adjusted Hydrogen’ - A procedure for measuring H+ by Barium Chloride-Triethanolamine method. Reference: Peech, M., Cowan, R.L. & Baker, J.H. (1962). Soil Science Society American Procedures, A critical study of the Barium chloride-Triethanolamine and ammonium acetate methods for determining exchangeable Hydrogen of soils."@en;
  skos:inScheme <http://anzoil.org/def/soil/au/edu/fed-uni>;
  skos:notation "15D1-BACL-CA";
  skos:prefLabel "Exchangable calcium procedure - 15D1 and Barium Chloride-Triethanolamine"@en;
  skos:topConceptOf <http://anzoil.org/def/soil/au/edu/fed-uni> .

procedure:MN a skos:Concept, sosa:Procedure;
  dct:description "A procedure for measuring Manganese"@en;
  dct:identifier "http://anzsoil.org/def/soil/au/edu/fed-uni/procedure/MN"^^xsd:anyURI;
  rdfs:label "Manganese procedure"@en;
  skos:definition "A procedure for measuring Manganese"@en;
  skos:inScheme <http://anzoil.org/def/soil/au/edu/fed-uni>;
  skos:notation "MN";
  skos:prefLabel "Manganese procedure"@en;
  skos:topConceptOf <http://anzoil.org/def/soil/au/edu/fed-uni> .

procedure:9K1 a skos:Concept, sosa:Procedure;
  dct:description "A procedure for measuring Mehlich 3-P saturation ratio"@en;
  dct:identifier "http://anzsoil.org/def/soil/au/edu/fed-uni/procedure/9K1"^^xsd:anyURI;
  rdfs:label "Mehlich 3-P saturation ratio"@en;
  skos:definition "A procedure for measuring Mehlich 3-P saturation ratio"@en;
  skos:inScheme <http://anzoil.org/def/soil/au/edu/fed-uni>;
  skos:notation "9K1";
  skos:prefLabel "Mehlich 3-P saturation ratio"@en;
  skos:topConceptOf <http://anzoil.org/def/soil/au/edu/fed-uni> .

procedure:soil-texture a skos:Concept, sosa:Procedure;
  dct:description "A procedure for measuring soil texture, method undefined"@en;
  dct:identifier "http://anzsoil.org/def/soil/au/edu/fed-uni/procedure/soil-texture"^^xsd:anyURI;
  rdfs:label "Soil Texture procedure"@en;
  skos:definition "A procedure for measuring soil texture, method undefined"@en;
  skos:inScheme <http://anzoil.org/def/soil/au/edu/fed-uni>;
  skos:prefLabel "Soil Texture procedure"@en;
  skos:topConceptOf <http://anzoil.org/def/soil/au/edu/fed-uni> .

procedure:SOM a skos:Concept, sosa:Procedure;
  dct:description "A procedure for measuring Soil Organic Matter (SOM)"@en;
  dct:identifier "http://anzsoil.org/def/soil/au/edu/fed-uni/procedure/SOM"^^xsd:anyURI;
  rdfs:label "Soil Organic Matter procedure"@en;
  skos:definition "A procedure for measuring Soil Organic Matter (SOM)"@en;
  skos:inScheme <http://anzoil.org/def/soil/au/edu/fed-uni>;
  skos:notation "SOM";
  skos:prefLabel "Soil Organic Matter procedure"@en;
  skos:topConceptOf <http://anzoil.org/def/soil/au/edu/fed-uni> .

procedure:field-soil-texture-organic a skos:Concept, sosa:Procedure;
  dct:description "Organic soils texture is determined by the size of mineral particles finer than 2 mm (NCST). In a sense, organic soils do have a texture related to the plant materials from which they formed and the degree of decomposition, exposure and drying. These field texture names may be used to characterise materials that on field examination are considered to be clearly dominated organic matter. Peats may be assessed examining the degree of decomposition and distinctness of plant remains. This work is adapted from Soil Survey Staff (1975) and Avery (1980). [R.C. McDonald and R.F. Isbell, in Australian soil and land survey field handbook (3rd edn)]"@en;
  dct:identifier "http://anzsoil.org/def/soil/au/edu/fed-uni/procedure/field-soil-texture-organic"^^xsd:anyURI;
  rdfs:label "Organic soils field texture grading method"@en;
  skos:definition "Organic soils texture is determined by the size of mineral particles finer than 2 mm (NCST). In a sense, organic soils do have a texture related to the plant materials from which they formed and the degree of decomposition, exposure and drying. These field texture names may be used to characterise materials that on field examination are considered to be clearly dominated organic matter. Peats may be assessed examining the degree of decomposition and distinctness of plant remains. This work is adapted from Soil Survey Staff (1975) and Avery (1980). [R.C. McDonald and R.F. Isbell, in Australian soil and land survey field handbook (3rd edn)]"@en;
  skos:inScheme <http://anzoil.org/def/soil/au/edu/fed-uni>;
  skos:prefLabel "Organic soils field texture grading method"@en;
  skos:topConceptOf <http://anzoil.org/def/soil/au/edu/fed-uni> .

procedure:WE-CN a skos:Concept, sosa:Procedure;
  dct:description "A procedure for measuring water-extractable Organic Carbon to Nitrogen ratio. Haney, R.L. et al. 2012. Soil Organic C:N vs. water-extractable organic C:N. Open Journal of Soil Science, 2012, 2, 269-274."@en;
  dct:identifier "http://anzsoil.org/def/soil/au/edu/fed-uni/procedure/WE-CN"^^xsd:anyURI;
  rdfs:label "Water extractable carbon to nitrogen ration procedure"@en;
  skos:definition "A procedure for measuring water-extractable Organic Carbon to Nitrogen ratio. Haney, R.L. et al. 2012. Soil Organic C:N vs. water-extractable organic C:N. Open Journal of Soil Science, 2012, 2, 269-274."@en;
  skos:inScheme <http://anzoil.org/def/soil/au/edu/fed-uni>;
  skos:notation "WE-CN";
  skos:prefLabel "Water extractable carbon to nitrogen ration procedure"@en;
  skos:topConceptOf <http://anzoil.org/def/soil/au/edu/fed-uni> .

procedure:WB-OM a skos:Concept, sosa:Procedure;
  dct:description "Organic Matter - W&B x 1.72"@en;
  dct:identifier "http://anzsoil.org/def/soil/au/edu/fed-uni/procedure/WB-OM"^^xsd:anyURI;
  rdfs:label "Organic Matter - W&B x 1.72"@en;
  skos:definition "Organic Matter calculated as Organic C W&B x 1.72, where Organic C W&B is determined by method 6A1 in Soil Chemical Methods Australasia 1. (2011), by George E Rayment and David J Lyons ISBN: 9780643101364"@en;
  skos:inScheme <http://anzoil.org/def/soil/au/edu/fed-uni>;
  skos:notation "WB-OM";
  skos:prefLabel "Organic Matter - W&B x 1.72"@en;
  skos:topConceptOf <http://anzoil.org/def/soil/au/edu/fed-uni> .

procedure:15D-CA a skos:Concept, sosa:Procedure;
  dct:description "A procedure for measuring Exchangeable calcium - 1 M ammonium acetate at pH 7.0"@en;
  dct:identifier "http://anzsoil.org/def/soil/au/edu/fed-uni/procedure/15D-CA"^^xsd:anyURI;
  rdfs:label "Exchangeable bases and CEC - 1 M ammonium acetate at pH 7.0"@en;
  skos:definition "A procedure for measuring Exchangeable calcium - 1 M ammonium acetate at pH 7.0procedure for measuring Exchangeable calcium - 1 M ammonium acetate at pH 7.0"@en;
  skos:inScheme <http://anzoil.org/def/soil/au/edu/fed-uni>;
  skos:notation "15D-CA";
  skos:prefLabel "Exchangeable bases and CEC - 1 M ammonium acetate at pH 7.0"@en;
  skos:topConceptOf <http://anzoil.org/def/soil/au/edu/fed-uni> .

procedure:bray-2 a skos:Concept, sosa:Procedure;
  dct:description "Bray 2 phosphorus procedure as defined by Bray, R.H and Kurtz, L.T. (1945). Determination of total, organic and available forms of phosphorus in soils. Soil Science 59:39-45."@en;
  dct:identifier "http://anzsoil.org/def/soil/au/edu/fed-uni/procedure/bray-2"^^xsd:anyURI;
  rdfs:label "Bray 2 Phosphorus"@en;
  skos:definition "Bray 2 phosphorus procedure as defined by Bray, R.H and Kurtz, L.T. (1945). Determination of total, organic and available forms of phosphorus in soils. Soil Science 59:39-45."@en;
  skos:inScheme <http://anzoil.org/def/soil/au/edu/fed-uni>;
  skos:notation "bray-2";
  skos:prefLabel "Bray 2 Phosphorus"@en;
  skos:topConceptOf <http://anzoil.org/def/soil/au/edu/fed-uni> .

property:POC-concentration a skos:Concept, sosa:ObservableProperty;
  dct:description "Concentration of particulate organic carbon"@en;
  dct:identifier "http://anzsoil.org/def/soil/au/edu/fed-uni/property/POC-concentration"^^xsd:anyURI;
  rdfs:label "Concentration of particulate organic carbon"@en;
  skos:definition "Concentration of particulate organic carbon"@en;
  skos:inScheme <http://anzoil.org/def/soil/au/edu/fed-uni>;
  skos:prefLabel "Concentration of particulate organic carbon"@en;
  skos:topConceptOf <http://anzoil.org/def/soil/au/edu/fed-uni> .

property:HUM-concentration a skos:Concept, sosa:ObservableProperty;
  dct:description "Concentration of organic carbon as humus or decomposed materials < 0.053mm"@en;
  dct:identifier "http://anzsoil.org/def/soil/au/edu/fed-uni/property/HUM-concentration"^^xsd:anyURI;
  rdfs:label "Concentration of organic carbon as humus or decomposed materials < 0.053mm"@en;
  skos:definition "Concentration of organic carbon as humus or decomposed materials < 0.053mm"@en;
  skos:inScheme <http://anzoil.org/def/soil/au/edu/fed-uni>;
  skos:prefLabel "Concentration of organic carbon as humus or decomposed materials < 0.053mm"@en;
  skos:topConceptOf <http://anzoil.org/def/soil/au/edu/fed-uni> .

property:REC-concentration a skos:Concept, sosa:ObservableProperty;
  dct:description "Concentration of recalcitrant organic carbon"@en;
  dct:identifier "http://anzsoil.org/def/soil/au/edu/fed-uni/property/REC-concentration"^^xsd:anyURI;
  rdfs:label "Concentration of recalcitrant organic carbon"@en;
  skos:definition "Concentration of recalcitrant organic carbon"@en;
  skos:inScheme <http://anzoil.org/def/soil/au/edu/fed-uni>;
  skos:prefLabel "Concentration of recalcitrant organic carbon"@en;
  skos:topConceptOf <http://anzoil.org/def/soil/au/edu/fed-uni> .

property:SOM-concentration a skos:Concept, sosa:ObservableProperty;
  dct:description "Soil organic matter concentration"@en;
  dct:identifier "http://anzsoil.org/def/soil/au/edu/fed-uni/property/SOM-concentration"^^xsd:anyURI;
  rdfs:label "Soil organic matter concentration"@en;
  skos:definition "Soil organic matter concentration"@en;
  skos:inScheme <http://anzoil.org/def/soil/au/edu/fed-uni>;
  skos:prefLabel "Soil organic matter concentration"@en;
  skos:topConceptOf <http://anzoil.org/def/soil/au/edu/fed-uni> .

property:clay-content a skos:Concept, sosa:ObservableProperty;
  dct:description "The approximate content of clay (particles less than 0.002 mm in diameter) (Marshall 1947)"@en;
  dct:identifier "http://anzsoil.org/def/soil/au/edu/fed-uni/property/clay-content"^^xsd:anyURI;
  rdfs:label "Clay content"@en;
  skos:definition "The approximate content of clay (particles less than 0.002 mm in diameter) (Marshall 1947)"@en;
  skos:inScheme <http://anzoil.org/def/soil/au/edu/fed-uni>;
  skos:prefLabel "Clay content"@en;
  skos:topConceptOf <http://anzoil.org/def/soil/au/edu/fed-uni> .

property:sand-content a skos:Concept, sosa:ObservableProperty;
  dct:description "The approximate content of sand (particles between 0.02 mm and 2.0 mm diameter) (Marshall 1947)"@en;
  dct:identifier "http://anzsoil.org/def/soil/au/edu/fed-uni/property/sand-content"^^xsd:anyURI;
  rdfs:label "Sand content"@en;
  skos:definition "The approximate content of sand (particles between 0.02 mm and 2.0 mm diameter) (Marshall 1947)"@en;
  skos:inScheme <http://anzoil.org/def/soil/au/edu/fed-uni>;
  skos:prefLabel "Sand content"@en;
  skos:topConceptOf <http://anzoil.org/def/soil/au/edu/fed-uni> .

property:silt-content a skos:Concept, sosa:ObservableProperty;
  dct:description "The approximate content of silt (particles between 0.002 and 0.02 mm in diameter) (Marshall 1947)"@en;
  dct:identifier "http://anzsoil.org/def/soil/au/edu/fed-uni/property/silt-content"^^xsd:anyURI;
  rdfs:label "Silt content"@en;
  skos:definition "The approximate content of silt (particles between 0.002 and 0.02 mm in diameter) (Marshall 1947)"@en;
  skos:inScheme <http://anzoil.org/def/soil/au/edu/fed-uni>;
  skos:prefLabel "Silt content"@en;
  skos:topConceptOf <http://anzoil.org/def/soil/au/edu/fed-uni> .

property:lower-depth-boundary a skos:Concept, sosa:ObservableProperty;
  dct:description "The lower depth boundary, that is the deepest or furthermost from the surface"@en;
  dct:identifier "http://anzsoil.org/def/soil/au/edu/fed-uni/property/lower-depth-boundary"^^xsd:anyURI;
  rdfs:label "The lower depth boundary"@en;
  skos:definition "The lower depth boundary, that is the deepest or furthermost from the surface"@en;
  skos:inScheme <http://anzoil.org/def/soil/au/edu/fed-uni>;
  skos:prefLabel "The lower depth boundary"@en;
  skos:topConceptOf <http://anzoil.org/def/soil/au/edu/fed-uni> .

property:upper-depth-boundary a skos:Concept, sosa:ObservableProperty;
  dct:description "The upper depth boundary, that is the closest to the surface"@en;
  dct:identifier "http://anzsoil.org/def/soil/au/edu/fed-uni/property/upper-depth-boundary"^^xsd:anyURI;
  rdfs:label "The upper depth boundary"@en;
  skos:definition "The upper depth boundary, that is the closest to the surface"@en;
  skos:inScheme <http://anzoil.org/def/soil/au/edu/fed-uni>;
  skos:prefLabel "The upper depth boundary"@en;
  skos:topConceptOf <http://anzoil.org/def/soil/au/edu/fed-uni> .

property:phosphorus-saturation-ratio a skos:Concept, sosa:ObservableProperty;
  dct:description "Phosphorus saturation ratio"@en;
  dct:identifier "http://anzsoil.org/def/soil/au/edu/fed-uni/property/phosphorus-saturation-ratio"^^xsd:anyURI;
  rdfs:label "Phosphorus saturation ratio"@en;
  skos:definition "Phosphorus saturation ratio"@en;
  skos:inScheme <http://anzoil.org/def/soil/au/edu/fed-uni>;
  skos:prefLabel "Phosphorus saturation ratio"@en;
  skos:topConceptOf <http://anzoil.org/def/soil/au/edu/fed-uni> .

property:phosphorus-retention-index a skos:Concept, sosa:ObservableProperty;
  dct:description "Phosphorus retention index defined as the ratio of the adsorbed phosphorus to the equilibrium concentration"@en;
  dct:identifier "http://anzsoil.org/def/soil/au/edu/fed-uni/property/phosphorus-retention-index"^^xsd:anyURI;
  rdfs:label "Phosphorus Retention Index"@en;
  skos:definition "Phosphorus retention index defined as the ratio of the adsorbed phosphorus to the equilibrium concentration"@en;
  skos:inScheme <http://anzoil.org/def/soil/au/edu/fed-uni>;
  skos:prefLabel "Phosphorus Retention Index"@en;
  skos:topConceptOf <http://anzoil.org/def/soil/au/edu/fed-uni> .

property:calcium-magnesium-ratio a skos:Concept, sosa:ObservableProperty;
  dct:description "Calcium to magnesium ratio"@en;
  dct:identifier "http://anzsoil.org/def/soil/au/edu/fed-uni/property/calcium-magnesium-ratio"^^xsd:anyURI;
  rdfs:label "Calcium to magnesium ratio"@en;
  skos:definition "Calcium to magnesium ratio"@en;
  skos:inScheme <http://anzoil.org/def/soil/au/edu/fed-uni>;
  skos:notation "CA/MG";
  skos:prefLabel "Calcium to magnesium ratio"@en;
  skos:topConceptOf <http://anzoil.org/def/soil/au/edu/fed-uni> .

property:potassium-magnesium-ratio a skos:Concept, sosa:ObservableProperty;
  dct:description "The ratio of potassium to magnesium"@en;
  dct:identifier "http://anzsoil.org/def/soil/au/edu/fed-uni/property/potassium-magnesium-ratio"^^xsd:anyURI;
  rdfs:label "Potassium to magnesium ratio"@en;
  skos:definition "The ratio of potassium to magnesium"@en;
  skos:inScheme <http://anzoil.org/def/soil/au/edu/fed-uni>;
  skos:notation "K/MG";
  skos:prefLabel "Potassium to magnesium ratio"@en;
  skos:topConceptOf <http://anzoil.org/def/soil/au/edu/fed-uni> .

property:potassium-sodium-ratio a skos:Concept, sosa:ObservableProperty;
  dct:description "Potassium to sodium ratio"@en;
  dct:identifier "http://anzsoil.org/def/soil/au/edu/fed-uni/property/potassium-sodium-ratio"^^xsd:anyURI;
  rdfs:label "Potassium to sodium ratio"@en;
  skos:definition "Potassium to sodium ratio"@en;
  skos:inScheme <http://anzoil.org/def/soil/au/edu/fed-uni>;
  skos:notation "K/NA";
  skos:prefLabel "Potassium to sodium ratio"@en;
  skos:topConceptOf <http://anzoil.org/def/soil/au/edu/fed-uni> .

property:exchangeable-cation-ratio a skos:Concept, sosa:ObservableProperty;
  dct:description "Exchageable cation ratio"@en;
  dct:identifier "http://anzsoil.org/def/soil/au/edu/fed-uni/property/exchangeable-cation-ratio"^^xsd:anyURI;
  rdfs:label "Exchangeable cation ratio"@en;
  skos:definition "Exchageable cation ratio"@en;
  skos:inScheme <http://anzoil.org/def/soil/au/edu/fed-uni>;
  skos:notation "ECR";
  skos:prefLabel "Exchangeable cation ratio"@en;
  skos:topConceptOf <http://anzoil.org/def/soil/au/edu/fed-uni> .

property:grass-tetany-risk-index a skos:Concept, sosa:ObservableProperty;
  dct:description "Grass tetany risk index"@en;
  dct:identifier "http://anzsoil.org/def/soil/au/edu/fed-uni/property/grass-tetany-risk-index"^^xsd:anyURI;
  rdfs:label "Grass tetany risk index"@en;
  skos:definition "Grass tetany risk index"@en;
  skos:inScheme <http://anzoil.org/def/soil/au/edu/fed-uni>;
  skos:notation "GTRI";
  skos:prefLabel "Grass tetany risk index"@en;
  skos:topConceptOf <http://anzoil.org/def/soil/au/edu/fed-uni> .

property:phosphorus-environmental-risk-index a skos:Concept, sosa:ObservableProperty;
  dct:description "Phosphorus environmental risk index"@en;
  dct:identifier "http://anzsoil.org/def/soil/au/edu/fed-uni/property/phosphorus-environmental-risk-index"^^xsd:anyURI;
  rdfs:label "Phosphorus environmental risk index"@en;
  skos:definition "Phosphorus environmental risk index"@en;
  skos:inScheme <http://anzoil.org/def/soil/au/edu/fed-uni>;
  skos:notation "PERI";
  skos:prefLabel "Phosphorus environmental risk index"@en;
  skos:topConceptOf <http://anzoil.org/def/soil/au/edu/fed-uni> .

procedure:TOC-TN a skos:Concept, sosa:ObservableProperty;
  dct:description "Total organic carbon to total nitrogen ratio"@en;
  dct:identifier "http://anzsoil.org/def/soil/au/edu/fed-uni/property/TOC-TN"^^xsd:anyURI;
  rdfs:label "Total organic carbon to total nitrogen ratio"@en;
  skos:definition "Total organic carbon to total nitrogen ratio"@en;
  skos:inScheme <http://anzoil.org/def/soil/au/edu/fed-uni>;
  skos:prefLabel "Total organic carbon to total nitrogen ratio"@en;
  skos:topConceptOf <http://anzoil.org/def/soil/au/edu/fed-uni> .

procedure:OC-TN a skos:Concept, sosa:ObservableProperty;
  dct:description "Organic carbon to total nitrogen ratio"@en;
  dct:identifier "http://anzsoil.org/def/soil/au/edu/fed-uni/property/OC-TN"^^xsd:anyURI;
  rdfs:label "Organic carbon to total nitrogen ratio"@en;
  skos:definition "Organic carbon to total nitrogen ratio"@en;
  skos:inScheme <http://anzoil.org/def/soil/au/edu/fed-uni>;
  skos:prefLabel "Organic carbon to total nitrogen ratio"@en;
  skos:topConceptOf <http://anzoil.org/def/soil/au/edu/fed-uni> .

property:evc-vic a skos:Concept, sosa:ObservableProperty;
  dct:description "\"Ecological Vegetation Classes (EVC) are the standard unit for classifying vegetation types in Victoria. EVCs are described through a combination of floristics, lifeforms and ecological characteristics, and through an inferred fidelity to particular environmental attributes. Each EVC includes a collection of floristic communities (i.e. lower level in the classification) that occur across a biogeographic range, and although differing in species, have similar habitat and ecological processes operating.\" Source: Victoria State Government, Departmend of Land, Water and Planning, https://www.environment.vic.gov.au/biodiversity/bioregions-and-evc-benchmarks last accessed 23/03/2020."@en;
  dct:identifier "http://anzsoil.org/def/soil/au/edu/fed-uni/property/evc-vic"^^xsd:anyURI;
  rdfs:label "Ecological Vegetation Class (VIctorian, Australia)"@en;
  skos:definition "\"Ecological Vegetation Classes (EVC) are the standard unit for classifying vegetation types in Victoria. EVCs are described through a combination of floristics, lifeforms and ecological characteristics, and through an inferred fidelity to particular environmental attributes. Each EVC includes a collection of floristic communities (i.e. lower level in the classification) that occur across a biogeographic range, and although differing in species, have similar habitat and ecological processes operating.\" Source: Victoria State Government, Departmend of Land, Water and Planning, https://www.environment.vic.gov.au/biodiversity/bioregions-and-evc-benchmarks last accessed 23/03/2020."@en;
  skos:inScheme <http://anzoil.org/def/soil/au/edu/fed-uni>;
  skos:notation "EVC";
  skos:prefLabel "Ecological Vegetation Class (VIctorian, Australia)"@en;
  skos:topConceptOf <http://anzoil.org/def/soil/au/edu/fed-uni> .

object:POC a skos:Concept;
  dct:description "A biologically significant fraction of soil organic carbon defined as individual pieces of plant debris that are <2 mm but > 0.053 mm"@en;
  dct:identifier "http://anzsoil.org/def/soil/au/edu/fed-uni/object/POC"^^xsd:anyURI;
  dct:source "Baldock JA (2008) Soil carbon: the basics. CSIRO Fact Sheet, as cited in Soil Chemical Methods Australasia 1. (2011), by George E Rayment and David J Lyons"@en;
  rdfs:label "Particulate Organic Carbon"@en;
  skos:definition "A biologically significant fraction of soil organic carbon defined as individual pieces of plant debris that are <2 mm but > 0.053 mm"@en;
  skos:inScheme <http://anzoil.org/def/soil/au/edu/fed-uni>;
  skos:prefLabel "Particulate Organic Carbon"@en;
  skos:topConceptOf <http://anzoil.org/def/soil/au/edu/fed-uni> .

object:HUM a skos:Concept;
  dct:description "A biologically significant fraction of soil organic carbon defined as humus or decomposed materials <0.053 mm, dominated by molecules adhering to soil minerals and colloids (Baldock JA (2008) Soil carbon: the basics. CSIRO Fact Sheet, as cited in Soil Chemical Methods Australasia 1. (2011), by George E Rayment and David J Lyons)"@en;
  dct:identifier "http://anzsoil.org/def/soil/au/edu/fed-uni/object/HUM"^^xsd:anyURI;
  dct:source "Baldock JA (2008) Soil carbon: the basics. CSIRO Fact Sheet, as cited in Soil Chemical Methods Australasia 1. (2011), by George E Rayment and David J Lyons"@en;
  rdfs:label "Humus or decomposed materials <0.053 mm"@en;
  skos:definition "A biologically significant fraction of soil organic carbon defined as humus or decomposed materials <0.053 mm, dominated by molecules adhering to soil minerals and colloids (Baldock JA (2008) Soil carbon: the basics. CSIRO Fact Sheet, as cited in Soil Chemical Methods Australasia 1. (2011), by George E Rayment and David J Lyons)"@en;
  skos:inScheme <http://anzoil.org/def/soil/au/edu/fed-uni>;
  skos:prefLabel "Humus or decomposed materials <0.053 mm"@en;
  skos:topConceptOf <http://anzoil.org/def/soil/au/edu/fed-uni> .

object:REC a skos:Concept;
  dct:description "A biologically significant fraction of soil organic carbon defined as biologically stable and typically in the form of charcoal (Baldock JA (2008) Soil carbon: the basics. CSIRO Fact Sheet, as cited in Soil Chemical Methods Australasia 1. (2011), by George E Rayment and David J Lyons)"@en;
  dct:identifier "http://anzsoil.org/def/soil/au/edu/fed-uni/object/REC"^^xsd:anyURI;
  dct:source "Baldock JA (2008) Soil carbon: the basics. CSIRO Fact Sheet, as cited in Soil Chemical Methods Australasia 1. (2011), by George E Rayment and David J Lyons"@en;
  rdfs:label "Recalcitrant Organic Carbon"@en;
  skos:definition "A biologically significant fraction of soil organic carbon defined as biologically stable and typically in the form of charcoal (Baldock JA (2008) Soil carbon: the basics. CSIRO Fact Sheet, as cited in Soil Chemical Methods Australasia 1. (2011), by George E Rayment and David J Lyons)"@en;
  skos:inScheme <http://anzoil.org/def/soil/au/edu/fed-uni>;
  skos:prefLabel "Recalcitrant Organic Carbon"@en;
  skos:topConceptOf <http://anzoil.org/def/soil/au/edu/fed-uni> .

classifier:grey a skos:Concept, sosa:Result;
  dct:description "The soil colour classifier 'grey' - a colour not recorded as hue, value or chroma as descibed in Chapter 8 Soil Profile, by R.C. McDonald and R.F. Isbell, in Australian soil and land survey field handbook (3rd edn) ISBN: 9780643097117. ISBN: 9780643097117"@en;
  dct:identifier "http://anzsoil.org/def/soil/au/edu/fed-uni/classifier/colour/grey"^^xsd:anyURI;
  rdfs:label "grey"@en;
  skos:definition "The soil colour classifier 'grey' - a colour not recorded as hue, value or chroma as descibed in Chapter 8 Soil Profile, by R.C. McDonald and R.F. Isbell, in Australian soil and land survey field handbook (3rd edn) ISBN: 9780643097117. ISBN: 9780643097117"@en;
  skos:inScheme <http://anzoil.org/def/soil/au/edu/fed-uni>;
  skos:prefLabel "grey"@en;
  skos:topConceptOf <http://anzoil.org/def/soil/au/edu/fed-uni> .

classifier:brown a skos:Concept, sosa:Result;
  dct:description "The soil colour classifier of 'brown' - a colour not recorded as hue, value or chroma as descibed in Chapter 8 Soil Profile, by R.C. McDonald and R.F. Isbell, in Australian soil and land survey field handbook (3rd edn) ISBN: 9780643097117. ISBN: 9780643097117."@en;
  dct:identifier "http://anzsoil.org/def/soil/au/edu/fed-uni/classifier/colour/brown"^^xsd:anyURI;
  rdfs:label "brown"@en;
  skos:definition "The soil colour classifier of 'brown' - a colour not recorded as hue, value or chroma as descibed in Chapter 8 Soil Profile, by R.C. McDonald and R.F. Isbell, in Australian soil and land survey field handbook (3rd edn) ISBN: 9780643097117. ISBN: 9780643097117."@en;
  skos:inScheme <http://anzoil.org/def/soil/au/edu/fed-uni>;
  skos:prefLabel "brown"@en;
  skos:topConceptOf <http://anzoil.org/def/soil/au/edu/fed-uni> .

classifier:orange-yellow a skos:Concept, sosa:Result;
  dct:description "The soil colour classifier of 'orange yellow' - a colour not recorded as hue, value or chroma as descibed in Chapter 8 Soil Profile, by R.C. McDonald and R.F. Isbell, in Australian soil and land survey field handbook (3rd edn) ISBN: 9780643097117. ISBN: 9780643097117."@en;
  dct:identifier "http://anzsoil.org/def/soil/au/edu/fed-uni/classifier/colour/orange-yellow"^^xsd:anyURI;
  rdfs:label "orange yellow"@en;
  skos:definition "The soil colour classifier of 'orange yellow' - a colour not recorded as hue, value or chroma as descibed in Chapter 8 Soil Profile, by R.C. McDonald and R.F. Isbell, in Australian soil and land survey field handbook (3rd edn) ISBN: 9780643097117. ISBN: 9780643097117."@en;
  skos:inScheme <http://anzoil.org/def/soil/au/edu/fed-uni>;
  skos:prefLabel "orange yellow"@en;
  skos:topConceptOf <http://anzoil.org/def/soil/au/edu/fed-uni> .

classifier:grey-brown a skos:Concept, sosa:Result;
  dct:description "The soil colour classifier of 'grey brown' - a colour not recorded as hue, value or chroma as descibed in Chapter 8 Soil Profile, by R.C. McDonald and R.F. Isbell, in Australian soil and land survey field handbook (3rd edn) ISBN: 9780643097117.."@en;
  dct:identifier "http://anzsoil.org/def/soil/au/edu/fed-uni/classifier/colour/grey-brown"^^xsd:anyURI;
  rdfs:label "grey brown"@en;
  skos:definition "The soil colour classifier of 'grey brown' - a colour not recorded as hue, value or chroma as descibed in Chapter 8 Soil Profile, by R.C. McDonald and R.F. Isbell, in Australian soil and land survey field handbook (3rd edn) ISBN: 9780643097117.."@en;
  skos:inScheme <http://anzoil.org/def/soil/au/edu/fed-uni>;
  skos:prefLabel "grey brown"@en;
  skos:topConceptOf <http://anzoil.org/def/soil/au/edu/fed-uni> .

classifier:brown-grey a skos:Concept, sosa:Result;
  dct:description "The soil colour classifier of 'brown grey' - a colour not recorded as hue, value or chroma as descibed in Chapter 8 Soil Profile, by R.C. McDonald and R.F. Isbell, in Australian soil and land survey field handbook (3rd edn) ISBN: 9780643097117.."@en;
  dct:identifier "http://anzsoil.org/def/soil/au/edu/fed-uni/classifier/colour/brown-grey"^^xsd:anyURI;
  rdfs:label "brown grey"@en;
  skos:definition "The soil colour classifier of 'brown grey' - a colour not recorded as hue, value or chroma as descibed in Chapter 8 Soil Profile, by R.C. McDonald and R.F. Isbell, in Australian soil and land survey field handbook (3rd edn) ISBN: 9780643097117.."@en;
  skos:inScheme <http://anzoil.org/def/soil/au/edu/fed-uni>;
  skos:prefLabel "brown grey"@en;
  skos:topConceptOf <http://anzoil.org/def/soil/au/edu/fed-uni> .

classifier:dark-grey a skos:Concept, sosa:Result;
  dct:description "The soil colour classifier of 'dark grey' - a colour not recorded as hue, value or chroma as descibed in Chapter 8 Soil Profile, by R.C. McDonald and R.F. Isbell, in Australian soil and land survey field handbook (3rd edn) ISBN: 9780643097117.."@en;
  dct:identifier "http://anzsoil.org/def/soil/au/edu/fed-uni/classifier/colour/dark-grey"^^xsd:anyURI;
  rdfs:label "dark grey"@en;
  skos:definition "The soil colour classifier of 'dark grey' - a colour not recorded as hue, value or chroma as descibed in Chapter 8 Soil Profile, by R.C. McDonald and R.F. Isbell, in Australian soil and land survey field handbook (3rd edn) ISBN: 9780643097117.."@en;
  skos:inScheme <http://anzoil.org/def/soil/au/edu/fed-uni>;
  skos:prefLabel "dark grey"@en;
  skos:topConceptOf <http://anzoil.org/def/soil/au/edu/fed-uni> .

classifier:light-grey a skos:Concept, sosa:Result;
  dct:description "The soil colour classifier of 'light grey' - a colour not recorded as hue, value or chroma as descibed in Chapter 8 Soil Profile, by R.C. McDonald and R.F. Isbell, in Australian soil and land survey field handbook (3rd edn) ISBN: 9780643097117.."@en;
  dct:identifier "http://anzsoil.org/def/soil/au/edu/fed-uni/classifier/colour/light-grey"^^xsd:anyURI;
  rdfs:label "light grey"@en;
  skos:definition "The soil colour classifier of 'light grey' - a colour not recorded as hue, value or chroma as descibed in Chapter 8 Soil Profile, by R.C. McDonald and R.F. Isbell, in Australian soil and land survey field handbook (3rd edn) ISBN: 9780643097117.."@en;
  skos:inScheme <http://anzoil.org/def/soil/au/edu/fed-uni>;
  skos:prefLabel "light grey"@en;
  skos:topConceptOf <http://anzoil.org/def/soil/au/edu/fed-uni> .

classifier:grey-yellow a skos:Concept, sosa:Result;
  dct:description "The soil colour classifier of 'grey yellow' - a colour not recorded as hue, value or chroma as descibed in Chapter 8 Soil Profile, by R.C. McDonald and R.F. Isbell, in Australian soil and land survey field handbook (3rd edn) ISBN: 9780643097117.."@en;
  dct:identifier "http://anzsoil.org/def/soil/au/edu/fed-uni/classifier/colour/grey-yellow"^^xsd:anyURI;
  rdfs:label "grey yellow"@en;
  skos:definition "The soil colour classifier of 'grey yellow' - a colour not recorded as hue, value or chroma as descibed in Chapter 8 Soil Profile, by R.C. McDonald and R.F. Isbell, in Australian soil and land survey field handbook (3rd edn) ISBN: 9780643097117.."@en;
  skos:inScheme <http://anzoil.org/def/soil/au/edu/fed-uni>;
  skos:prefLabel "grey yellow"@en;
  skos:topConceptOf <http://anzoil.org/def/soil/au/edu/fed-uni> .

classifier:dark-brown a skos:Concept, sosa:Result;
  dct:description "The soil colour classifier of 'dark brown' - a colour not recorded as hue, value or chroma as descibed in Chapter 8 Soil Profile, by R.C. McDonald and R.F. Isbell, in Australian soil and land survey field handbook (3rd edn) ISBN: 9780643097117.."@en;
  dct:identifier "http://anzsoil.org/def/soil/au/edu/fed-uni/classifier/colour/dark-brown"^^xsd:anyURI;
  rdfs:label "dark brown"@en;
  skos:definition "The soil colour classifier of 'dark brown' - a colour not recorded as hue, value or chroma as descibed in Chapter 8 Soil Profile, by R.C. McDonald and R.F. Isbell, in Australian soil and land survey field handbook (3rd edn) ISBN: 9780643097117.."@en;
  skos:inScheme <http://anzoil.org/def/soil/au/edu/fed-uni>;
  skos:prefLabel "dark brown"@en;
  skos:topConceptOf <http://anzoil.org/def/soil/au/edu/fed-uni> .

classifier:light-brown a skos:Concept, sosa:Result;
  dct:description "The soil colour classifier of 'light brown' - a colour not recorded as hue, value or chroma as descibed in Chapter 8 Soil Profile, by R.C. McDonald and R.F. Isbell, in Australian soil and land survey field handbook (3rd edn) ISBN: 9780643097117.."@en;
  dct:identifier "http://anzsoil.org/def/soil/au/edu/fed-uni/classifier/colour/light-brown"^^xsd:anyURI;
  rdfs:label "light brown"@en;
  skos:definition "The soil colour classifier of 'light brown' - a colour not recorded as hue, value or chroma as descibed in Chapter 8 Soil Profile, by R.C. McDonald and R.F. Isbell, in Australian soil and land survey field handbook (3rd edn) ISBN: 9780643097117.."@en;
  skos:inScheme <http://anzoil.org/def/soil/au/edu/fed-uni>;
  skos:prefLabel "light brown"@en;
  skos:topConceptOf <http://anzoil.org/def/soil/au/edu/fed-uni> .

classifier:brown-yellow a skos:Concept, sosa:Result;
  dct:description "The soil colour classifier of 'brown yellow' - a colour not recorded as hue, value or chroma as descibed in Chapter 8 Soil Profile, by R.C. McDonald and R.F. Isbell, in Australian soil and land survey field handbook (3rd edn) ISBN: 9780643097117.."@en;
  dct:identifier "http://anzsoil.org/def/soil/au/edu/fed-uni/classifier/colour/brown-yellow"^^xsd:anyURI;
  rdfs:label "brown yellow"@en;
  skos:definition "The soil colour classifier of 'brown yellow' - a colour not recorded as hue, value or chroma as descibed in Chapter 8 Soil Profile, by R.C. McDonald and R.F. Isbell, in Australian soil and land survey field handbook (3rd edn) ISBN: 9780643097117.."@en;
  skos:inScheme <http://anzoil.org/def/soil/au/edu/fed-uni>;
  skos:prefLabel "brown yellow"@en;
  skos:topConceptOf <http://anzoil.org/def/soil/au/edu/fed-uni> .

classifier:red a skos:Concept, sosa:Result;
  dct:description "The soil colour classifier of 'red' - a colour not recorded as hue, value or chroma as descibed in Chapter 8 Soil Profile, by R.C. McDonald and R.F. Isbell, in Australian soil and land survey field handbook (3rd edn) ISBN: 9780643097117.."@en;
  dct:identifier "http://anzsoil.org/def/soil/au/edu/fed-uni/classifier/colour/red"^^xsd:anyURI;
  rdfs:label "red"@en;
  skos:definition "The soil colour classifier of 'red' - a colour not recorded as hue, value or chroma as descibed in Chapter 8 Soil Profile, by R.C. McDonald and R.F. Isbell, in Australian soil and land survey field handbook (3rd edn) ISBN: 9780643097117.."@en;
  skos:inScheme <http://anzoil.org/def/soil/au/edu/fed-uni>;
  skos:prefLabel "red"@en;
  skos:topConceptOf <http://anzoil.org/def/soil/au/edu/fed-uni> .

classifier:grey-black a skos:Concept, sosa:Result;
  dct:description "The soil colour classifier of 'grey black' - a colour not recorded as hue, value or chroma as descibed in Chapter 8 Soil Profile, by R.C. McDonald and R.F. Isbell, in Australian soil and land survey field handbook (3rd edn) ISBN: 9780643097117.."@en;
  dct:identifier "http://anzsoil.org/def/soil/au/edu/fed-uni/classifier/colour/grey-black"^^xsd:anyURI;
  rdfs:label "grey black"@en;
  skos:definition "The soil colour classifier of 'grey black' - a colour not recorded as hue, value or chroma as descibed in Chapter 8 Soil Profile, by R.C. McDonald and R.F. Isbell, in Australian soil and land survey field handbook (3rd edn) ISBN: 9780643097117.."@en;
  skos:inScheme <http://anzoil.org/def/soil/au/edu/fed-uni>;
  skos:prefLabel "grey black"@en;
  skos:topConceptOf <http://anzoil.org/def/soil/au/edu/fed-uni> .

classifier:brown-black a skos:Concept, sosa:Result;
  dct:description "The soil colour classifier of 'brown black' - a colour not recorded as hue, value or chroma as descibed in Chapter 8 Soil Profile, by R.C. McDonald and R.F. Isbell, in Australian soil and land survey field handbook (3rd edn) ISBN: 9780643097117.."@en;
  dct:identifier "http://anzsoil.org/def/soil/au/edu/fed-uni/classifier/colour/brown-black"^^xsd:anyURI;
  rdfs:label "brown black"@en;
  skos:definition "The soil colour classifier of 'brown black' - a colour not recorded as hue, value or chroma as descibed in Chapter 8 Soil Profile, by R.C. McDonald and R.F. Isbell, in Australian soil and land survey field handbook (3rd edn) ISBN: 9780643097117.."@en;
  skos:inScheme <http://anzoil.org/def/soil/au/edu/fed-uni>;
  skos:prefLabel "brown black"@en;
  skos:topConceptOf <http://anzoil.org/def/soil/au/edu/fed-uni> .

classifier:brown-orange a skos:Concept, sosa:Result;
  dct:description "The soil colour classifier of 'brown orange' - a colour not recorded as hue, value or chroma as descibed in Chapter 8 Soil Profile, by R.C. McDonald and R.F. Isbell, in Australian soil and land survey field handbook (3rd edn) ISBN: 9780643097117.."@en;
  dct:identifier "http://anzsoil.org/def/soil/au/edu/fed-uni/classifier/colour/brown-orange"^^xsd:anyURI;
  rdfs:label "brown orange"@en;
  skos:definition "The soil colour classifier of 'brown orange' - a colour not recorded as hue, value or chroma as descibed in Chapter 8 Soil Profile, by R.C. McDonald and R.F. Isbell, in Australian soil and land survey field handbook (3rd edn) ISBN: 9780643097117.."@en;
  skos:inScheme <http://anzoil.org/def/soil/au/edu/fed-uni>;
  skos:prefLabel "brown orange"@en;
  skos:topConceptOf <http://anzoil.org/def/soil/au/edu/fed-uni> .

classifier:brown-white a skos:Concept, sosa:Result;
  dct:description "The soil colour classifier of 'brown white' - a colour not recorded as hue, value or chroma as descibed in Chapter 8 Soil Profile, by R.C. McDonald and R.F. Isbell, in Australian soil and land survey field handbook (3rd edn) ISBN: 9780643097117.."@en;
  dct:identifier "http://anzsoil.org/def/soil/au/edu/fed-uni/classifier/colour/brown-white"^^xsd:anyURI;
  rdfs:label "brown white"@en;
  skos:definition "The soil colour classifier of 'brown white' - a colour not recorded as hue, value or chroma as descibed in Chapter 8 Soil Profile, by R.C. McDonald and R.F. Isbell, in Australian soil and land survey field handbook (3rd edn) ISBN: 9780643097117.."@en;
  skos:inScheme <http://anzoil.org/def/soil/au/edu/fed-uni>;
  skos:prefLabel "brown white"@en;
  skos:topConceptOf <http://anzoil.org/def/soil/au/edu/fed-uni> .

classifier:yellow a skos:Concept, sosa:Result;
  dct:description "The soil colour classifier of 'yellow' - a colour not recorded as hue, value or chroma as descibed in Chapter 8 Soil Profile, by R.C. McDonald and R.F. Isbell, in Australian soil and land survey field handbook (3rd edn) ISBN: 9780643097117.."@en;
  dct:identifier "http://anzsoil.org/def/soil/au/edu/fed-uni/classifier/colour/yellow"^^xsd:anyURI;
  rdfs:label "yellow"@en;
  skos:definition "The soil colour classifier of 'yellow' - a colour not recorded as hue, value or chroma as descibed in Chapter 8 Soil Profile, by R.C. McDonald and R.F. Isbell, in Australian soil and land survey field handbook (3rd edn) ISBN: 9780643097117.."@en;
  skos:inScheme <http://anzoil.org/def/soil/au/edu/fed-uni>;
  skos:prefLabel "yellow"@en;
  skos:topConceptOf <http://anzoil.org/def/soil/au/edu/fed-uni> .

classifier:brown-red a skos:Concept, sosa:Result;
  dct:description "The soil colour classifier of 'brown red' - a colour not recorded as hue, value or chroma as descibed in Chapter 8 Soil Profile, by R.C. McDonald and R.F. Isbell, in Australian soil and land survey field handbook (3rd edn) ISBN: 9780643097117.."@en;
  dct:identifier "http://anzsoil.org/def/soil/au/edu/fed-uni/classifier/colour/brown-red"^^xsd:anyURI;
  rdfs:label "brown red"@en;
  skos:definition "The soil colour classifier of 'brown red' - a colour not recorded as hue, value or chroma as descibed in Chapter 8 Soil Profile, by R.C. McDonald and R.F. Isbell, in Australian soil and land survey field handbook (3rd edn) ISBN: 9780643097117.."@en;
  skos:inScheme <http://anzoil.org/def/soil/au/edu/fed-uni>;
  skos:prefLabel "brown red"@en;
  skos:topConceptOf <http://anzoil.org/def/soil/au/edu/fed-uni> .

classifier:grey-white a skos:Concept, sosa:Result;
  dct:description "The soil colour classifier of 'grey white' - a colour not recorded as hue, value or chroma as descibed in Chapter 8 Soil Profile, by R.C. McDonald and R.F. Isbell, in Australian soil and land survey field handbook (3rd edn) ISBN: 9780643097117.."@en;
  dct:identifier "http://anzsoil.org/def/soil/au/edu/fed-uni/classifier/colour/grey-white"^^xsd:anyURI;
  rdfs:label "grey white"@en;
  skos:definition "The soil colour classifier of 'grey white' - a colour not recorded as hue, value or chroma as descibed in Chapter 8 Soil Profile, by R.C. McDonald and R.F. Isbell, in Australian soil and land survey field handbook (3rd edn) ISBN: 9780643097117.."@en;
  skos:inScheme <http://anzoil.org/def/soil/au/edu/fed-uni>;
  skos:prefLabel "grey white"@en;
  skos:topConceptOf <http://anzoil.org/def/soil/au/edu/fed-uni> .

classifier:yellow-brown a skos:Concept, sosa:Result;
  dct:description "The soil colour classifier of 'yellow brown' - a colour not recorded as hue, value or chroma as descibed in Chapter 8 Soil Profile, by R.C. McDonald and R.F. Isbell, in Australian soil and land survey field handbook (3rd edn) ISBN: 9780643097117.."@en;
  dct:identifier "http://anzsoil.org/def/soil/au/edu/fed-uni/classifier/colour/yellow-brown"^^xsd:anyURI;
  rdfs:label "yellow brown"@en;
  skos:definition "The soil colour classifier of 'yellow brown' - a colour not recorded as hue, value or chroma as descibed in Chapter 8 Soil Profile, by R.C. McDonald and R.F. Isbell, in Australian soil and land survey field handbook (3rd edn) ISBN: 9780643097117.."@en;
  skos:inScheme <http://anzoil.org/def/soil/au/edu/fed-uni>;
  skos:prefLabel "yellow brown"@en;
  skos:topConceptOf <http://anzoil.org/def/soil/au/edu/fed-uni> .

classifier:dark-yellow-brown a skos:Concept, sosa:Result;
  dct:description "The soil colour classifier of 'dark yellow brown' - a colour not recorded as hue, value or chroma as descibed in Chapter 8 Soil Profile, by R.C. McDonald and R.F. Isbell, in Australian soil and land survey field handbook (3rd edn) ISBN: 9780643097117."@en;
  dct:identifier "http://anzsoil.org/def/soil/au/edu/fed-uni/classifier/colour/dark-yellow-brown"^^xsd:anyURI;
  rdfs:label "dark yellow brown"@en;
  skos:definition "The soil colour classifier of 'dark yellow brown' - a colour not recorded as hue, value or chroma as descibed in Chapter 8 Soil Profile, by R.C. McDonald and R.F. Isbell, in Australian soil and land survey field handbook (3rd edn) ISBN: 9780643097117."@en;
  skos:inScheme <http://anzoil.org/def/soil/au/edu/fed-uni>;
  skos:prefLabel "dark yellow brown"@en;
  skos:topConceptOf <http://anzoil.org/def/soil/au/edu/fed-uni> .

classifier:black a skos:Concept, sosa:Result;
  dct:description "The soil colour classifier of 'black' - a colour not recorded as hue, value or chroma as descibed in Chapter 8 Soil Profile, by R.C. McDonald and R.F. Isbell, in Australian soil and land survey field handbook (3rd edn) ISBN: 9780643097117."@en;
  dct:identifier "http://anzsoil.org/def/soil/au/edu/fed-uni/classifier/colour/black"^^xsd:anyURI;
  rdfs:label "black"@en;
  skos:definition "The soil colour classifier of 'black' - a colour not recorded as hue, value or chroma as descibed in Chapter 8 Soil Profile, by R.C. McDonald and R.F. Isbell, in Australian soil and land survey field handbook (3rd edn) ISBN: 9780643097117."@en;
  skos:inScheme <http://anzoil.org/def/soil/au/edu/fed-uni>;
  skos:prefLabel "black"@en;
  skos:topConceptOf <http://anzoil.org/def/soil/au/edu/fed-uni> .

classifier:dark-grey-brown a skos:Concept, sosa:Result;
  dct:description "The soil colour classifier of 'dark-grey-brown' - a colour not recorded as hue, value or chroma as descibed in Chapter 8 Soil Profile, by R.C. McDonald and R.F. Isbell, in Australian soil and land survey field handbook (3rd edn) ISBN: 9780643097117."@en;
  dct:identifier "http://anzsoil.org/def/soil/au/edu/fed-uni/classifier/colour/dark-grey-brown"^^xsd:anyURI;
  rdfs:label "dark grey brown"@en;
  skos:definition "The soil colour classifier of 'dark-grey-brown' - a colour not recorded as hue, value or chroma as descibed in Chapter 8 Soil Profile, by R.C. McDonald and R.F. Isbell, in Australian soil and land survey field handbook (3rd edn) ISBN: 9780643097117."@en;
  skos:inScheme <http://anzoil.org/def/soil/au/edu/fed-uni>;
  skos:prefLabel "dark grey brown"@en;
  skos:topConceptOf <http://anzoil.org/def/soil/au/edu/fed-uni> .

classifier:red-brown a skos:Concept, sosa:Result;
  dct:description "The soil colour classifier of 'red-brown' - a colour not recorded as hue, value or chroma as descibed in Chapter 8 Soil Profile, by R.C. McDonald and R.F. Isbell, in Australian soil and land survey field handbook (3rd edn) ISBN: 9780643097117."@en;
  dct:identifier "http://anzsoil.org/def/soil/au/edu/fed-uni/classifier/colour/red-brown"^^xsd:anyURI;
  rdfs:label "red brown"@en;
  skos:definition "The soil colour classifier of 'red-brown' - a colour not recorded as hue, value or chroma as descibed in Chapter 8 Soil Profile, by R.C. McDonald and R.F. Isbell, in Australian soil and land survey field handbook (3rd edn) ISBN: 9780643097117."@en;
  skos:inScheme <http://anzoil.org/def/soil/au/edu/fed-uni>;
  skos:prefLabel "red brown"@en;
  skos:topConceptOf <http://anzoil.org/def/soil/au/edu/fed-uni> .

classifier:very-dark-grey a skos:Concept, sosa:Result;
  dct:description "The soil colour classifier of 'very-dark-grey' - a colour not recorded as hue, value or chroma as descibed in Chapter 8 Soil Profile, by R.C. McDonald and R.F. Isbell, in Australian soil and land survey field handbook (3rd edn) ISBN: 9780643097117."@en;
  dct:identifier "http://anzsoil.org/def/soil/au/edu/fed-uni/classifier/colour/very-dark-grey"^^xsd:anyURI;
  rdfs:label "very dark grey"@en;
  skos:definition "The soil colour classifier of 'very-dark-grey' - a colour not recorded as hue, value or chroma as descibed in Chapter 8 Soil Profile, by R.C. McDonald and R.F. Isbell, in Australian soil and land survey field handbook (3rd edn) ISBN: 9780643097117."@en;
  skos:inScheme <http://anzoil.org/def/soil/au/edu/fed-uni>;
  skos:prefLabel "very dark grey"@en;
  skos:topConceptOf <http://anzoil.org/def/soil/au/edu/fed-uni> .

classifier:light-olive-brown a skos:Concept, sosa:Result;
  dct:description "The soil colour classifier of 'light-olive-brown' - a colour not recorded as hue, value or chroma as descibed in Chapter 8 Soil Profile, by R.C. McDonald and R.F. Isbell, in Australian soil and land survey field handbook (3rd edn) ISBN: 9780643097117."@en;
  dct:identifier "http://anzsoil.org/def/soil/au/edu/fed-uni/classifier/colour/light-olive-brown"^^xsd:anyURI;
  rdfs:label "light olive brown"@en;
  skos:definition "The soil colour classifier of 'light-olive-brown' - a colour not recorded as hue, value or chroma as descibed in Chapter 8 Soil Profile, by R.C. McDonald and R.F. Isbell, in Australian soil and land survey field handbook (3rd edn) ISBN: 9780643097117."@en;
  skos:inScheme <http://anzoil.org/def/soil/au/edu/fed-uni>;
  skos:prefLabel "light olive brown"@en;
  skos:topConceptOf <http://anzoil.org/def/soil/au/edu/fed-uni> .

classifier:very-dark-grey-brown a skos:Concept, sosa:Result;
  dct:description "The soil colour classifier of 'very-dark-grey-brown' - a colour not recorded as hue, value or chroma as descibed in Chapter 8 Soil Profile, by R.C. McDonald and R.F. Isbell, in Australian soil and land survey field handbook (3rd edn) ISBN: 9780643097117."@en;
  dct:identifier "http://anzsoil.org/def/soil/au/edu/fed-uni/classifier/colour/very-dark-grey-brown"^^xsd:anyURI;
  rdfs:label "very dark grey brown"@en;
  skos:definition "The soil colour classifier of 'very-dark-grey-brown' - a colour not recorded as hue, value or chroma as descibed in Chapter 8 Soil Profile, by R.C. McDonald and R.F. Isbell, in Australian soil and land survey field handbook (3rd edn) ISBN: 9780643097117."@en;
  skos:inScheme <http://anzoil.org/def/soil/au/edu/fed-uni>;
  skos:prefLabel "very dark grey brown"@en;
  skos:topConceptOf <http://anzoil.org/def/soil/au/edu/fed-uni> .

classifier:very-dark-brown a skos:Concept, sosa:Result;
  dct:description "The soil colour classifier of 'very-dark-brown' - a colour not recorded as hue, value or chroma as descibed in Chapter 8 Soil Profile, by R.C. McDonald and R.F. Isbell, in Australian soil and land survey field handbook (3rd edn) ISBN: 9780643097117."@en;
  dct:identifier "http://anzsoil.org/def/soil/au/edu/fed-uni/classifier/colour/very-dark-brown"^^xsd:anyURI;
  rdfs:label "very dark brown"@en;
  skos:definition "The soil colour classifier of 'very-dark-brown' - a colour not recorded as hue, value or chroma as descibed in Chapter 8 Soil Profile, by R.C. McDonald and R.F. Isbell, in Australian soil and land survey field handbook (3rd edn) ISBN: 9780643097117."@en;
  skos:inScheme <http://anzoil.org/def/soil/au/edu/fed-uni>;
  skos:prefLabel "very dark brown"@en;
  skos:topConceptOf <http://anzoil.org/def/soil/au/edu/fed-uni> .

classifier:light-yellow-brown a skos:Concept, sosa:Result;
  dct:description "The soil colour classifier of 'light-yellow-brown' - a colour not recorded as hue, value or chroma as descibed in Chapter 8 Soil Profile, by R.C. McDonald and R.F. Isbell, in Australian soil and land survey field handbook (3rd edn) ISBN: 9780643097117."@en;
  dct:identifier "http://anzsoil.org/def/soil/au/edu/fed-uni/classifier/colour/light-yellow-brown"^^xsd:anyURI;
  rdfs:label "light yellow brown"@en;
  skos:definition "The soil colour classifier of 'light-yellow-brown' - a colour not recorded as hue, value or chroma as descibed in Chapter 8 Soil Profile, by R.C. McDonald and R.F. Isbell, in Australian soil and land survey field handbook (3rd edn) ISBN: 9780643097117."@en;
  skos:inScheme <http://anzoil.org/def/soil/au/edu/fed-uni>;
  skos:prefLabel "light yellow brown"@en;
  skos:topConceptOf <http://anzoil.org/def/soil/au/edu/fed-uni> .

classifier:light-grey-brown a skos:Concept, sosa:Result;
  dct:description "The soil colour classifier of 'light-grey-brown' - a colour not recorded as hue, value or chroma as descibed in Chapter 8 Soil Profile, by R.C. McDonald and R.F. Isbell, in Australian soil and land survey field handbook (3rd edn) ISBN: 9780643097117."@en;
  dct:identifier "http://anzsoil.org/def/soil/au/edu/fed-uni/classifier/colour/light-grey-brown"^^xsd:anyURI;
  rdfs:label "light grey brown"@en;
  skos:definition "The soil colour classifier of 'light-grey-brown' - a colour not recorded as hue, value or chroma as descibed in Chapter 8 Soil Profile, by R.C. McDonald and R.F. Isbell, in Australian soil and land survey field handbook (3rd edn) ISBN: 9780643097117."@en;
  skos:inScheme <http://anzoil.org/def/soil/au/edu/fed-uni>;
  skos:prefLabel "light grey brown"@en;
  skos:topConceptOf <http://anzoil.org/def/soil/au/edu/fed-uni> .

classifier:very-dusky-red a skos:Concept, sosa:Result;
  dct:description "The soil colour classifier of 'very-dusky-red' - a colour not recorded as hue, value or chroma as descibed in Chapter 8 Soil Profile, by R.C. McDonald and R.F. Isbell, in Australian soil and land survey field handbook (3rd edn) ISBN: 9780643097117."@en;
  dct:identifier "http://anzsoil.org/def/soil/au/edu/fed-uni/classifier/colour/very-dusky-red"^^xsd:anyURI;
  rdfs:label "very dusky red"@en;
  skos:definition "The soil colour classifier of 'very-dusky-red' - a colour not recorded as hue, value or chroma as descibed in Chapter 8 Soil Profile, by R.C. McDonald and R.F. Isbell, in Australian soil and land survey field handbook (3rd edn) ISBN: 9780643097117."@en;
  skos:inScheme <http://anzoil.org/def/soil/au/edu/fed-uni>;
  skos:prefLabel "very dusky red"@en;
  skos:topConceptOf <http://anzoil.org/def/soil/au/edu/fed-uni> .

classifier:dusky-red a skos:Concept, sosa:Result;
  dct:description "The soil colour classifier of 'dusky-red' - a colour not recorded as hue, value or chroma as descibed in Chapter 8 Soil Profile, by R.C. McDonald and R.F. Isbell, in Australian soil and land survey field handbook (3rd edn) ISBN: 9780643097117."@en;
  dct:identifier "http://anzsoil.org/def/soil/au/edu/fed-uni/classifier/colour/dusky-red"^^xsd:anyURI;
  rdfs:label "dusky red"@en;
  skos:definition "The soil colour classifier of 'dusky-red' - a colour not recorded as hue, value or chroma as descibed in Chapter 8 Soil Profile, by R.C. McDonald and R.F. Isbell, in Australian soil and land survey field handbook (3rd edn) ISBN: 9780643097117."@en;
  skos:inScheme <http://anzoil.org/def/soil/au/edu/fed-uni>;
  skos:prefLabel "dusky red"@en;
  skos:topConceptOf <http://anzoil.org/def/soil/au/edu/fed-uni> .

classifier:olive-grey a skos:Concept, sosa:Result;
  dct:description "The soil colour classifier of 'olive-grey' - a colour not recorded as hue, value or chroma as descibed in Chapter 8 Soil Profile, by R.C. McDonald and R.F. Isbell, in Australian soil and land survey field handbook (3rd edn) ISBN: 9780643097117."@en;
  dct:identifier "http://anzsoil.org/def/soil/au/edu/fed-uni/classifier/colour/olive-grey"^^xsd:anyURI;
  rdfs:label "olive grey"@en;
  skos:definition "The soil colour classifier of 'olive-grey' - a colour not recorded as hue, value or chroma as descibed in Chapter 8 Soil Profile, by R.C. McDonald and R.F. Isbell, in Australian soil and land survey field handbook (3rd edn) ISBN: 9780643097117."@en;
  skos:inScheme <http://anzoil.org/def/soil/au/edu/fed-uni>;
  skos:prefLabel "olive grey"@en;
  skos:topConceptOf <http://anzoil.org/def/soil/au/edu/fed-uni> .

procedure:TC-KJE a skos:Concept, sosa:Procedure;
  dct:created "2021-12-23"@en;
  dct:description "A procedure for measuring Total Carbon by Kjeldahl method"@en;
  dct:identifier "http://registry.it.csiro.au/def/soil/au/edu/fed-uni/procedure/TC-KJE"^^xsd:anyURI;
  rdfs:label "TC-KJE"@en;
  skos:definition "A procedure for measuring Total Carbon by Kjeldahl method"@en;
  skos:inScheme <http://anzoil.org/def/soil/au/edu/fed-uni>;
  skos:notation "TC-KJE";
  skos:prefLabel "Total Carbon procedure - Kjeldahl method"@en;
  skos:topConceptOf <http://anzoil.org/def/soil/au/edu/fed-uni> .

procedure:CSBP-CA a skos:Concept, sosa:Procedure;
  dct:created "2021-12-23"@en;
  dct:description "Exchangeable Calcium - CSBP Soil and Plant Analysis Laboratory in house Lab procedure derived from 5A4 described in Soil Chemical Methods  Australasia 1. (2011), by George E Rayment and David J Lyons."@en;
  dct:identifier "http://registry.it.csiro.au/def/soil/au/edu/fed-uni/procedure/CSBP-CA"^^xsd:anyURI;
  rdfs:label "CSBP-CA"@en;
  skos:definition "Exchangeable Calcium - CSBP Soil and Plant Analysis Laboratory in house Lab procedure derived from 5A4 described in Soil Chemical Methods  Australasia 1. (2011), by George E Rayment and David J Lyons."@en;
  skos:inScheme <http://anzoil.org/def/soil/au/edu/fed-uni>;
  skos:notation "CSBP-CA";
  skos:prefLabel "Exchangeable Calcium - CSBP Procedure"@en;
  skos:topConceptOf <http://anzoil.org/def/soil/au/edu/fed-uni> .

procedure:CSBP-MG a skos:Concept, sosa:Procedure;
  dct:created "2021-12-23"@en;
  dct:description "Exchangeable Magnesium - CSBP Soil and Plant Analysis Laboratory in house Lab procedure derived from 5A4 described in Soil Chemical Methods Australasia 1. (2011), by George E Rayment and David J Lyons."@en;
  dct:identifier "http://registry.it.csiro.au/def/soil/au/edu/fed-uni/procedure/CSBP-MG"^^xsd:anyURI;
  rdfs:label "CSBP-MG"@en;
  skos:definition "Exchangeable Magnesium - CSBP Soil and Plant Analysis Laboratory in house Lab procedure derived from 5A4 described in Soil Chemical Methods Australasia 1. (2011), by George E Rayment and David J Lyons."@en;
  skos:inScheme <http://anzoil.org/def/soil/au/edu/fed-uni>;
  skos:notation "CSBP-MG";
  skos:prefLabel "Exchangeable Magnesium - CSBP Procedure"@en;
  skos:topConceptOf <http://anzoil.org/def/soil/au/edu/fed-uni> .

procedure:CSBP-K a skos:Concept, sosa:Procedure;
  dct:created "2021-12-23"@en;
  dct:description "Exchangeable Potassium - CSBP Soil and Plant Analysis Laboratory in house Lab procedure derived from 5A4 described in Soil Chemical Methods  Australasia 1. (2011), by George E Rayment and David J Lyons."@en;
  dct:identifier "http://registry.it.csiro.au/def/soil/au/edu/fed-uni/procedure/CSBP-K"^^xsd:anyURI;
  rdfs:label "CSBP-K"@en;
  skos:definition "Exchangeable Potassium - CSBP Soil and Plant Analysis Laboratory in house Lab procedure derived from 5A4 described in Soil Chemical Methods  Australasia 1. (2011), by George E Rayment and David J Lyons."@en;
  skos:inScheme <http://anzoil.org/def/soil/au/edu/fed-uni>;
  skos:notation "CSBP-K";
  skos:prefLabel "Exchangeable Potassium - CSBP Procedure"@en;
  skos:topConceptOf <http://anzoil.org/def/soil/au/edu/fed-uni> .

procedure:CSBP-NA a skos:Concept, sosa:Procedure;
  dct:created "2021-12-23"@en;
  dct:description "Exchangeable Sodium- CSBP Soil and Plant Analysis Laboratory in house Lab procedure derived from 5A4 described in Soil Chemical Methods  Australasia 1. (2011), by George E Rayment and David J Lyons."@en;
  dct:identifier "http://registry.it.csiro.au/def/soil/au/edu/fed-uni/procedure/CSBP-NA"^^xsd:anyURI;
  rdfs:label "CSBP-NA"@en;
  skos:definition "Exchangeable Sodium- CSBP Soil and Plant Analysis Laboratory in house Lab procedure derived from 5A4 described in Soil Chemical Methods  Australasia 1. (2011), by George E Rayment and David J Lyons."@en;
  skos:inScheme <http://anzoil.org/def/soil/au/edu/fed-uni>;
  skos:notation "CSBP-NA";
  skos:prefLabel "Exchangeable Sodium- CSBP Procedure"@en;
  skos:topConceptOf <http://anzoil.org/def/soil/au/edu/fed-uni> .

procedure:15G a skos:Concept, sosa:Procedure;
  dct:created "2021-12-23"@en;
  dct:description "Exchangable Acidity Procedure (15G)"@en;
  dct:identifier "http://registry.it.csiro.au/def/soil/au/edu/fed-uni/procedure/15G"^^xsd:anyURI;
  rdfs:label "15G"@en;
  skos:definition "Exchangable Acidity Procedure (15G)"@en;
  skos:inScheme <http://anzoil.org/def/soil/au/edu/fed-uni>;
  skos:notation "15G";
  skos:prefLabel "Acidity - Exchangeable Procedure"@en;
  skos:topConceptOf <http://anzoil.org/def/soil/au/edu/fed-uni> .

procedure:15G-AL a skos:Concept, sosa:Procedure;
  dct:created "2021-12-23"@en;
  dct:description "Exchangable Aluminium Procedure (15G)"@en;
  dct:identifier "http://registry.it.csiro.au/def/soil/au/edu/fed-uni/procedure/15G-AL"^^xsd:anyURI;
  rdfs:label "15G-AL"@en;
  skos:definition "Exchangable Aluminium Procedure (15G)"@en;
  skos:inScheme <http://anzoil.org/def/soil/au/edu/fed-uni>;
  skos:notation "15G-AL";
  skos:prefLabel "Aluminium - Exchangeable Procedure"@en;
  skos:topConceptOf <http://anzoil.org/def/soil/au/edu/fed-uni> .

procedure:15G-H a skos:Concept, sosa:Procedure;
  dct:created "2021-12-23"@en;
  dct:description "Exchangable Hydrogen Procedure (15G)"@en;
  dct:identifier "http://registry.it.csiro.au/def/soil/au/edu/fed-uni/procedure/15G-H"^^xsd:anyURI;
  rdfs:label "15G-H"@en;
  skos:definition "Exchangable Hydrogen Procedure (15G)"@en;
  skos:inScheme <http://anzoil.org/def/soil/au/edu/fed-uni>;
  skos:notation "15G-H";
  skos:prefLabel "Hydrogen - Exchangeable Procedure"@en;
  skos:topConceptOf <http://anzoil.org/def/soil/au/edu/fed-uni> .

procedure:15D-MG a skos:Concept, sosa:Procedure;
  dct:created "2021-12-23"@en;
  dct:description "Exchangeable Magnesium Procedure (15D) - Ammonium Acetate"@en;
  dct:identifier "http://registry.it.csiro.au/def/soil/au/edu/fed-uni/procedure/15D-MG"^^xsd:anyURI;
  rdfs:label "15D-MG"@en;
  skos:definition "Exchangeable Magnesium Procedure (15D) - Ammonium Acetate"@en;
  skos:inScheme <http://anzoil.org/def/soil/au/edu/fed-uni>;
  skos:notation "15D-MG";
  skos:prefLabel "Magnesium - Exchangeable Procedure"@en;
  skos:topConceptOf <http://anzoil.org/def/soil/au/edu/fed-uni> .

procedure:15D-K a skos:Concept, sosa:Procedure;
  dct:created "2021-12-23"@en;
  dct:description "Exchangeable Potassium Procedure (15D) - Ammonium Acetate"@en;
  dct:identifier "http://registry.it.csiro.au/def/soil/au/edu/fed-uni/procedure/15D-K"^^xsd:anyURI;
  rdfs:label "15D-K"@en;
  skos:definition "Exchangeable Potassium Procedure (15D) - Ammonium Acetate"@en;
  skos:inScheme <http://anzoil.org/def/soil/au/edu/fed-uni>;
  skos:notation "15D-K";
  skos:prefLabel "Potassium - Exchangeable Procedure"@en;
  skos:topConceptOf <http://anzoil.org/def/soil/au/edu/fed-uni> .

procedure:15D-NA a skos:Concept, sosa:Procedure;
  dct:created "2021-12-23"@en;
  dct:description "Exchangeable Sodium Procedure (15D) - Ammonium Acetate"@en;
  dct:identifier "http://registry.it.csiro.au/def/soil/au/edu/fed-uni/procedure/15D-NA"^^xsd:anyURI;
  rdfs:label "15D-NA"@en;
  skos:definition "Exchangeable Sodium Procedure (15D) - Ammonium Acetate"@en;
  skos:inScheme <http://anzoil.org/def/soil/au/edu/fed-uni>;
  skos:notation "15D-NA";
  skos:prefLabel "Sodium - Exchangeable Procedure"@en;
  skos:topConceptOf <http://anzoil.org/def/soil/au/edu/fed-uni> .

classifier:name a "reg:Register"@en, ldp:Container;
  dct:created "2022-02-07"@en;
  dct:description "Soil names outside of the Australian Soil Classification Editions."@en;
  dct:identifier "http://anzsoil.org/def/soil/au/edu/fed-uni/classifier/name"^^xsd:anyURI;
  rdfs:label "Soil name"@en;
  skos:definition "Soil names outside of the Australian Soil Classification Editions."@en;
  skos:member name:lismore-soil-series;
  skos:prefLabel "Soil name"@en .

name:lismore-soil-series a "reg:Register"@en, ldp:Container;
  dct:created "2022-02-07"@en;
  dct:description "Soil classification according to 'Soil Series Mapping of the Lismore Region, Victorian Volcanic Plains'. Thesis. Shari Linda McConachy, BAppSc(Hons)Geology, Department of Geology University of Ballarat, June 2009."@en;
  dct:identifier "http://anzsoil.org/def/soil/au/edu/fed-uni/classifier/name/lismore-soil-series"^^xsd:anyURI;
  rdfs:label "Lismore Soil Series"@en;
  skos:definition "Soil classification according to 'Soil Series Mapping of the Lismore Region, Victorian Volcanic Plains'. Thesis. Shari Linda McConachy, BAppSc(Hons)Geology, Department of Geology University of Ballarat, June 2009."@en;
  skos:member lismore-soil-series:buckshot-clays, lismore-soil-series:granitic-sandy-loam,
    lismore-soil-series:lismore-grey-clays, lismore-soil-series:lunette-clays, lismore-soil-series:mundy-gully-black-clays,
    lismore-soil-series:nowra-red-clays;
  skos:prefLabel "Lismore Soil Series"@en .

lismore-soil-series:mundy-gully-black-clays a skos:Concept, sosa:Result;
  dct:created "2022-02-07"@en;
  dct:description "Mundy Gully Black Clays. Following the Soil Series delineated by study 'Soil Series Mapping of the Lismore Region, Victorian Volcanic Plains'. Thesis. Shari Linda McConachy, BAppSc(Hons)Geology, Department of Geology University of Ballarat, June 2009."@en;
  dct:identifier "http://anzsoil.org/def/soil/au/edu/fed-uni/classifier/name/lismore-soil-series/mundy-gully-black-clays"^^xsd:anyURI;
  rdfs:label "Mundy Gully Black Clays"@en;
  skos:definition "Mundy Gully Black Clays. Following the Soil Series delineated by study 'Soil Series Mapping of the Lismore Region, Victorian Volcanic Plains'. Thesis. Shari Linda McConachy, BAppSc(Hons)Geology, Department of Geology University of Ballarat, June 2009."@en;
  skos:inScheme <http://anzoil.org/def/soil/au/edu/fed-uni>;
  skos:prefLabel "Mundy Gully Black Clays"@en;
  skos:topConceptOf <http://anzoil.org/def/soil/au/edu/fed-uni> .

lismore-soil-series:buckshot-clays a skos:Concept, sosa:Result;
  dct:created "2022-02-07"@en;
  dct:description "Buckshot Clays. Following the Soil Series delineated by study 'Soil Series Mapping of the Lismore Region, Victorian Volcanic Plains'. Thesis. Shari Linda McConachy, BAppSc(Hons)Geology, Department of Geology University of Ballarat, June 2009."@en;
  dct:identifier "http://anzsoil.org/def/soil/au/edu/fed-uni/classifier/name/lismore-soil-series/buckshot-clays"^^xsd:anyURI;
  rdfs:label "Buckshot clays"@en;
  skos:definition "Buckshot Clays. Following the Soil Series delineated by study 'Soil Series Mapping of the Lismore Region, Victorian Volcanic Plains'. Thesis. Shari Linda McConachy, BAppSc(Hons)Geology, Department of Geology University of Ballarat, June 2009."@en;
  skos:inScheme <http://anzoil.org/def/soil/au/edu/fed-uni>;
  skos:prefLabel "Buckshot clays"@en;
  skos:topConceptOf <http://anzoil.org/def/soil/au/edu/fed-uni> .

lismore-soil-series:lismore-grey-clays a skos:Concept, sosa:Result;
  dct:created "2022-02-07"@en;
  dct:description "Lismore Grey Clays. Following the Soil Series delineated by study 'Soil Series Mapping of the Lismore Region, Victorian Volcanic Plains'. Thesis. Shari Linda McConachy, BAppSc(Hons)Geology, Department of Geology University of Ballarat, June 2009."@en;
  dct:identifier "http://anzsoil.org/def/soil/au/edu/fed-uni/classifier/name/lismore-soil-series/lismore-grey-clays"^^xsd:anyURI;
  rdfs:label "Lismore Grey Clays"@en;
  skos:definition "Lismore Grey Clays. Following the Soil Series delineated by study 'Soil Series Mapping of the Lismore Region, Victorian Volcanic Plains'. Thesis. Shari Linda McConachy, BAppSc(Hons)Geology, Department of Geology University of Ballarat, June 2009."@en;
  skos:inScheme <http://anzoil.org/def/soil/au/edu/fed-uni>;
  skos:prefLabel "Lismore Grey Clays"@en;
  skos:topConceptOf <http://anzoil.org/def/soil/au/edu/fed-uni> .

lismore-soil-series:nowra-red-clays a skos:Concept, sosa:Result;
  dct:created "2022-02-07"@en;
  dct:description "Nowra Red Clays. Following the Soil Series delineated by study 'Soil Series Mapping of the Lismore Region, Victorian Volcanic Plains'. Thesis. Shari Linda McConachy, BAppSc(Hons)Geology, Department of Geology University of Ballarat, June 2009."@en;
  dct:identifier "http://anzsoil.org/def/soil/au/edu/fed-uni/classifier/name/lismore-soil-series/nowra-red-clays"^^xsd:anyURI;
  rdfs:label "Nowra Red Clays"@en;
  skos:definition "Nowra Red Clays. Following the Soil Series delineated by study 'Soil Series Mapping of the Lismore Region, Victorian Volcanic Plains'. Thesis. Shari Linda McConachy, BAppSc(Hons)Geology, Department of Geology University of Ballarat, June 2009."@en;
  skos:inScheme <http://anzoil.org/def/soil/au/edu/fed-uni>;
  skos:prefLabel "Nowra Red Clays"@en;
  skos:topConceptOf <http://anzoil.org/def/soil/au/edu/fed-uni> .

lismore-soil-series:lunette-clays a skos:Concept, sosa:Result;
  dct:created "2022-02-07"@en;
  dct:description "Lunette Clays. Following the Soil Series delineated by study 'Soil Series Mapping of the Lismore Region, Victorian Volcanic Plains'. Thesis. Shari Linda McConachy, BAppSc(Hons)Geology, Department of Geology University of Ballarat, June 2009."@en;
  dct:identifier "http://anzsoil.org/def/soil/au/edu/fed-uni/classifier/name/lismore-soil-series/lunette-clays"^^xsd:anyURI;
  rdfs:label "Lunette Clays"@en;
  skos:definition "Lunette Clays. Following the Soil Series delineated by study 'Soil Series Mapping of the Lismore Region, Victorian Volcanic Plains'. Thesis. Shari Linda McConachy, BAppSc(Hons)Geology, Department of Geology University of Ballarat, June 2009."@en;
  skos:inScheme <http://anzoil.org/def/soil/au/edu/fed-uni>;
  skos:prefLabel "Lunette Clays"@en;
  skos:topConceptOf <http://anzoil.org/def/soil/au/edu/fed-uni> .

lismore-soil-series:granitic-sandy-loam a skos:Concept, sosa:Result;
  dct:created "2022-02-07"@en;
  dct:description "Granitic Sandy Loam. Following the Soil Series delineated by study 'Soil Series Mapping of the Lismore Region, Victorian Volcanic Plains'. Thesis. Shari Linda McConachy, BAppSc(Hons)Geology, Department of Geology University of Ballarat, June 2009."@en;
  dct:identifier "http://anzsoil.org/def/soil/au/edu/fed-uni/classifier/name/lismore-soil-series/granitic-sandy-loam"^^xsd:anyURI;
  rdfs:label "Granitic Sandy Loam"@en;
  skos:definition "Granitic Sandy Loam. Following the Soil Series delineated by study 'Soil Series Mapping of the Lismore Region, Victorian Volcanic Plains'. Thesis. Shari Linda McConachy, BAppSc(Hons)Geology, Department of Geology University of Ballarat, June 2009."@en;
  skos:inScheme <http://anzoil.org/def/soil/au/edu/fed-uni>;
  skos:prefLabel "Granitic Sandy Loam"@en;
  skos:topConceptOf <http://anzoil.org/def/soil/au/edu/fed-uni> .

texture-grade:C a skos:Concept, sosa:Result;
  dct:created "2022-02-07"@en;
  dct:description "The texture grade of Clay"@en;
  dct:identifier "http://anzsoil.org/def/soil/au/edu/fed-uni/classifier/texture-grade/C"^^xsd:anyURI;
  rdfs:label "Clay"@en;
  skos:definition "The texture grade of Clay"@en;
  skos:inScheme <http://anzoil.org/def/soil/au/edu/fed-uni>;
  skos:prefLabel "Clay"@en;
  skos:topConceptOf <http://anzoil.org/def/soil/au/edu/fed-uni> .

texture-grade:CSBP-S a skos:Concept, sosa:Result;
  dct:created "2022-02-07"@en;
  dct:description "Sand - CSBP classification scheme 2012. An indication whether the soil type changed between samples, not an accurate measurement of the soil characteristics."@en;
  dct:identifier "http://anzsoil.org/def/soil/au/edu/fed-uni/classifier/texture-grade/CSBP-S"^^xsd:anyURI;
  rdfs:label "Sand - CSBP classification"@en;
  skos:definition "Sand - CSBP classification scheme 2012. An indication whether the soil type changed between samples, not an accurate measurement of the soil characteristics."@en;
  skos:inScheme <http://anzoil.org/def/soil/au/edu/fed-uni>;
  skos:prefLabel "Sand - CSBP classification"@en;
  skos:topConceptOf <http://anzoil.org/def/soil/au/edu/fed-uni> .

texture-grade:CSBP-LS a skos:Concept, sosa:Result;
  dct:created "2022-02-07"@en;
  dct:description "Loamy sand - CSBP classification scheme 2012. An indication whether the soil type changed between samples, not an accurate measurement of the soil characteristics."@en;
  dct:identifier "http://anzsoil.org/def/soil/au/edu/fed-uni/classifier/texture-grade/CSBP-LS"^^xsd:anyURI;
  rdfs:label "Loamy sand - CSBP classification"@en;
  skos:definition "Loamy sand - CSBP classification scheme 2012. An indication whether the soil type changed between samples, not an accurate measurement of the soil characteristics."@en;
  skos:inScheme <http://anzoil.org/def/soil/au/edu/fed-uni>;
  skos:prefLabel "Loamy sand - CSBP classification"@en;
  skos:topConceptOf <http://anzoil.org/def/soil/au/edu/fed-uni> .

texture-grade:CSBP-L a skos:Concept, sosa:Result;
  dct:created "2022-02-07"@en;
  dct:description "Loam - CSBP classification scheme 2012. An indication whether the soil type changed between samples, not an accurate measurement of the soil characteristics."@en;
  dct:identifier "http://anzsoil.org/def/soil/au/edu/fed-uni/classifier/texture-grade/CSBP-L"^^xsd:anyURI;
  rdfs:label "Loam - CSBP classification"@en;
  skos:definition "Loam - CSBP classification scheme 2012. An indication whether the soil type changed between samples, not an accurate measurement of the soil characteristics."@en;
  skos:inScheme <http://anzoil.org/def/soil/au/edu/fed-uni>;
  skos:prefLabel "Loam - CSBP classification"@en;
  skos:topConceptOf <http://anzoil.org/def/soil/au/edu/fed-uni> .

texture-grade:CSBP-CL a skos:Concept, sosa:Result;
  dct:created "2022-02-07"@en;
  dct:description "Clay loam - CSBP classification scheme 2012. An indication whether the soil type changed between samples, not an accurate measurement of the soil characteristics."@en;
  dct:identifier "http://anzsoil.org/def/soil/au/edu/fed-uni/classifier/texture-grade/CSBP-CL"^^xsd:anyURI;
  rdfs:label "Clay loam - CSBP classification"@en;
  skos:definition "Clay loam - CSBP classification scheme 2012. An indication whether the soil type changed between samples, not an accurate measurement of the soil characteristics."@en;
  skos:inScheme <http://anzoil.org/def/soil/au/edu/fed-uni>;
  skos:prefLabel "Clay loam - CSBP classification"@en;
  skos:topConceptOf <http://anzoil.org/def/soil/au/edu/fed-uni> .

texture-grade:CSBP-C a skos:Concept, sosa:Result;
  dct:created "2022-02-07"@en;
  dct:description "Clay - CSBP classification scheme 2012. An indication whether the soil type changed between samples, not an accurate measurement of the soil characteristics."@en;
  dct:identifier "http://anzsoil.org/def/soil/au/edu/fed-uni/classifier/texture-grade/CSBP-C"^^xsd:anyURI;
  rdfs:label "Clay - CSBP classification"@en;
  skos:definition "Clay - CSBP classification scheme 2012. An indication whether the soil type changed between samples, not an accurate measurement of the soil characteristics."@en;
  skos:inScheme <http://anzoil.org/def/soil/au/edu/fed-uni>;
  skos:prefLabel "Clay - CSBP classification"@en;
  skos:topConceptOf <http://anzoil.org/def/soil/au/edu/fed-uni> .

texture-grade:CSBP-HC a skos:Concept, sosa:Result;
  dct:created "2022-02-07"@en;
  dct:description "Heavy clay - CSBP classification scheme 2012. An indication whether the soil type changed between samples, not an accurate measurement of the soil characteristics."@en;
  dct:identifier "http://anzsoil.org/def/soil/au/edu/fed-uni/classifier/texture-grade/CSBP-HC"^^xsd:anyURI;
  rdfs:label "Heavy clay - CSBP classification"@en;
  skos:definition "Heavy clay - CSBP classification scheme 2012. An indication whether the soil type changed between samples, not an accurate measurement of the soil characteristics."@en;
  skos:inScheme <http://anzoil.org/def/soil/au/edu/fed-uni>;
  skos:prefLabel "Heavy clay - CSBP classification"@en;
  skos:topConceptOf <http://anzoil.org/def/soil/au/edu/fed-uni> .

texture-grade:L a skos:Concept, sosa:Result;
  dct:created "2022-02-07"@en;
  dct:description "The texture grade of Loam"@en;
  dct:identifier "http://anzsoil.org/def/soil/au/edu/fed-uni/classifier/texture-grade/L"^^xsd:anyURI;
  rdfs:label "Loam"@en;
  skos:definition "The texture grade of Loam"@en;
  skos:inScheme <http://anzoil.org/def/soil/au/edu/fed-uni>;
  skos:prefLabel "Loam"@en;
  skos:topConceptOf <http://anzoil.org/def/soil/au/edu/fed-uni> .

texture-grade:SL a skos:Concept, sosa:Result;
  dct:created "2022-02-07"@en;
  dct:description "The texture grade of Sandy Loam"@en;
  dct:identifier "http://anzsoil.org/def/soil/au/edu/fed-uni/classifier/texture-grade/SL"^^xsd:anyURI;
  rdfs:label "Sandy Loam"@en;
  skos:definition "The texture grade of Sandy Loam"@en;
  skos:inScheme <http://anzoil.org/def/soil/au/edu/fed-uni>;
  skos:prefLabel "Sandy Loam"@en;
  skos:topConceptOf <http://anzoil.org/def/soil/au/edu/fed-uni> .

texture-grade:CL a skos:Concept, sosa:Result;
  dct:created "2022-02-07"@en;
  dct:description "The texture grade of Clay Loam"@en;
  dct:identifier "http://anzsoil.org/def/soil/au/edu/fed-uni/classifier/texture-grade/CL"^^xsd:anyURI;
  rdfs:label "Clay Loam"@en;
  skos:definition "The texture grade of Clay Loam"@en;
  skos:inScheme <http://anzoil.org/def/soil/au/edu/fed-uni>;
  skos:prefLabel "Clay Loam"@en;
  skos:topConceptOf <http://anzoil.org/def/soil/au/edu/fed-uni> .

texture-grade:SCL a skos:Concept, sosa:Result;
  dct:created "2022-02-07"@en;
  dct:description "The texture grade of Sandy Clay Loam"@en;
  dct:identifier "http://anzsoil.org/def/soil/au/edu/fed-uni/classifier/texture-grade/SCL"^^xsd:anyURI;
  rdfs:label "Sandy Clay Loam"@en;
  skos:definition "The texture grade of Sandy Clay Loam"@en;
  skos:inScheme <http://anzoil.org/def/soil/au/edu/fed-uni>;
  skos:prefLabel "Sandy Clay Loam"@en;
  skos:topConceptOf <http://anzoil.org/def/soil/au/edu/fed-uni> .

texture-grade:SC a skos:Concept, sosa:Result;
  dct:created "2022-02-07"@en;
  dct:description "The texture grade of Sandy Clay"@en;
  dct:identifier "http://anzsoil.org/def/soil/au/edu/fed-uni/classifier/texture-grade/SC"^^xsd:anyURI;
  rdfs:label "Sandy Clay"@en;
  skos:definition "The texture grade of Sandy Clay"@en;
  skos:inScheme <http://anzoil.org/def/soil/au/edu/fed-uni>;
  skos:prefLabel "Sandy Clay"@en;
  skos:topConceptOf <http://anzoil.org/def/soil/au/edu/fed-uni> .

texture-grade:S a skos:Concept, sosa:Result;
  dct:created "2022-02-07"@en;
  dct:description "The texture grade of Sand"@en;
  dct:identifier "http://anzsoil.org/def/soil/au/edu/fed-uni/classifier/texture-grade/S"^^xsd:anyURI;
  rdfs:label "Sand"@en;
  skos:definition "The texture grade of Sand"@en;
  skos:inScheme <http://anzoil.org/def/soil/au/edu/fed-uni>;
  skos:prefLabel "Sand"@en;
  skos:topConceptOf <http://anzoil.org/def/soil/au/edu/fed-uni> .

texture-grade:LS a skos:Concept, sosa:Result;
  dct:created "2022-02-07"@en;
  dct:description "The texture grade of Loamy Sand"@en;
  dct:identifier "http://anzsoil.org/def/soil/au/edu/fed-uni/classifier/texture-grade/LS"^^xsd:anyURI;
  rdfs:label "Loamy Sand"@en;
  skos:definition "The texture grade of Loamy Sand"@en;
  skos:inScheme <http://anzoil.org/def/soil/au/edu/fed-uni>;
  skos:prefLabel "Loamy Sand"@en;
  skos:topConceptOf <http://anzoil.org/def/soil/au/edu/fed-uni> .

procedure:bouyoucos-1936 a skos:Concept, sosa:Procedure;
  dct:created "2022-02-07"@en;
  dct:description "Bouyoucos, G.J. (1936) Directions for making mechanical analysis of soils by the hydrometer method. Soil Science, 42, 225-230. doi:10.1097/00010694-193609000-00007"@en;
  dct:identifier "http://anzsoil.org/def/soil/au/edu/fed-uni/procedure/bouyoucos-1936"^^xsd:anyURI;
  rdfs:label "Hydrometer method (Bouyoucos 1936)"@en;
  skos:definition "Bouyoucos, G.J. (1936) Directions for making mechanical analysis of soils by the hydrometer method. Soil Science, 42, 225-230. doi:10.1097/00010694-193609000-00007"@en;
  skos:inScheme <http://anzoil.org/def/soil/au/edu/fed-uni>;
  skos:prefLabel "Hydrometer method (Bouyoucos 1936)"@en;
  skos:topConceptOf <http://anzoil.org/def/soil/au/edu/fed-uni> .

classifier:structure-pedality-type a "reg:Register"@en, ldp:Container;
  dct:created "2022-02-07"@en;
  dct:description "These Type of Pedality fall outside those described in Australian Soil and Land Survey Field Handbook (3rd edn). ISBN: 9780643093959"@en;
  dct:identifier "http://anzsoil.org/def/soil/au/edu/fed-uni/procedure/structure-pedality-type"^^xsd:anyURI;
  rdfs:label "Type of pedality"@en;
  skos:definition "These Type of Pedality fall outside those described in Australian Soil and Land Survey Field Handbook (3rd edn). ISBN: 9780643093959"@en;
  skos:member structure-pedality-type:B;
  skos:prefLabel "Type of pedality"@en .

structure-pedality-type:B a skos:Concept, sosa:Result;
  dct:created "2022-02-07"@en;
  dct:description "The Type of Pedality 'Blocky'. This Type of Pedality fall outside those described in Australian Soil and Land Survey Field Handbook (3rd edn). ISBN: 9780643093959"@en;
  dct:identifier "http://anzsoil.org/def/soil/au/edu/fed-uni/procedure/structure-pedality-type/B"^^xsd:anyURI;
  rdfs:label "Blocky"@en;
  skos:definition "The Type of Pedality 'Blocky'. This Type of Pedality fall outside those described in Australian Soil and Land Survey Field Handbook (3rd edn). ISBN: 9780643093959"@en;
  skos:inScheme <http://anzoil.org/def/soil/au/edu/fed-uni>;
  skos:prefLabel "Blocky"@en;
  skos:topConceptOf <http://anzoil.org/def/soil/au/edu/fed-uni> .
